{
    "@context": {
        "Fiware": "https://uri.fiware.org/ns/data-models#",
        "GTFS": "http://vocab.gtfs.org/gtfs.ttl#",
        "geojson": "https://purl.org/geojson/vocab#",
        "iudx": "https://voc.iudx.org.in/",
        "open311": "http://ontology.eil.utoronto.ca/open311.owl#",
        "owl": "http://www.w3.org/2002/07/owl#",
        "rdf": "http://www.w3.org/1999/02/22-rdf-syntax-ns#",
        "rdfs": "http://www.w3.org/2000/01/rdf-schema#",
        "schema": "http://schema.org/",
        "skos": "http://www.w3.org/2004/02/skos/core#"
    },
    "@graph": [
        {
            "@id": "https://voc.iudx.org.in/IssueReporting",
            "@type": "owl:Class",
            "rdfs:comment": "A Data Model for citizen issues, reports and feedbacks.",
            "rdfs:isDefinedBy": {
                "@id": "https://voc.iudx.org.in/"
            },
            "rdfs:label": "IssueReporting",
            "rdfs:subClassOf": {
                "@id": "https://voc.iudx.org.in/Civic"
            }
        },
        {
            "@id": "https://voc.iudx.org.in/PointOfInterest",
            "@type": "owl:Class",
            "rdfs:comment": "A Data Model for geographic description of a Point of Interest.",
            "rdfs:isDefinedBy": {
                "@id": "https://voc.iudx.org.in/"
            },
            "rdfs:label": "PointOfInterest",
            "rdfs:subClassOf": {
                "@id": "https://voc.iudx.org.in/Civic"
            }
        },
        {
            "@id": "https://voc.iudx.org.in/RevenueCollection",
            "@type": "owl:Class",
            "rdfs:comment": "A Data Model for city revenue collection operations.",
            "rdfs:isDefinedBy": {
                "@id": "https://voc.iudx.org.in/"
            },
            "rdfs:label": "RevenueCollection",
            "rdfs:subClassOf": {
                "@id": "https://voc.iudx.org.in/Civic"
            }
        },
        {
            "@id": "https://voc.iudx.org.in/SafetiPin",
            "@type": "owl:Class",
            "rdfs:comment": "A Data Model for information collected from a large group of people who submit their data via the My safetiPin app.",
            "rdfs:isDefinedBy": {
                "@id": "https://voc.iudx.org.in/"
            },
            "rdfs:label": "SafetiPin",
            "rdfs:subClassOf": {
                "@id": "https://voc.iudx.org.in/Civic"
            }
        },
        {
            "@id": "https://voc.iudx.org.in/WaterDistributionNetwork",
            "@type": "owl:Class",
            "rdfs:comment": "A Data Model for water supply network in a city.",
            "rdfs:isDefinedBy": {
                "@id": "https://voc.iudx.org.in/"
            },
            "rdfs:label": "WaterDistributionNetwork",
            "rdfs:subClassOf": {
                "@id": "https://voc.iudx.org.in/Civic"
            }
        },
        {
            "@id": "https://voc.iudx.org.in/Device",
            "@type": "owl:Class",
            "rdfs:comment": "Properties of the device that could have sensors or actuators which report measurements corresponding to this observation.",
            "rdfs:isDefinedBy": {
                "@id": "https://voc.iudx.org.in/"
            },
            "rdfs:label": "Device"
        },
        {
            "@id": "https://voc.iudx.org.in/EnvAQM",
            "@type": "owl:Class",
            "rdfs:comment": "Air Quality Monitoring (AQM) Data Model.",
            "rdfs:isDefinedBy": {
                "@id": "https://voc.iudx.org.in/"
            },
            "rdfs:label": "EnvAQM",
            "rdfs:subClassOf": {
                "@id": "https://voc.iudx.org.in/Environment"
            }
        },
        {
            "@id": "https://voc.iudx.org.in/EnvFlood",
            "@type": "owl:Class",
            "rdfs:comment": "Flood Sensor Data Model intended to represent the level of flooding w.r.t water flow/level at a certain water mass(river, lake,etc.).",
            "rdfs:isDefinedBy": {
                "@id": "https://voc.iudx.org.in/"
            },
            "rdfs:label": "EnvFlood",
            "rdfs:subClassOf": {
                "@id": "https://voc.iudx.org.in/Environment"
            }
        },
        {
            "@id": "https://voc.iudx.org.in/EnvWeather",
            "@type": "owl:Class",
            "rdfs:comment": "Data Model for weather conditions observed at a certain place and time.",
            "rdfs:isDefinedBy": {
                "@id": "https://voc.iudx.org.in/"
            },
            "rdfs:label": "EnvWeather",
            "rdfs:subClassOf": {
                "@id": "https://voc.iudx.org.in/Environment"
            }
        },
        {
            "@id": "https://voc.iudx.org.in/FeedEntity",
            "@type": "owl:Class",
            "rdfs:comment": "A definition (or update) of an entity in the transit feed. If the entity is not being deleted, exactly one of 'trip_update', 'vehicle' and 'alert' fields should be populated.",
            "rdfs:isDefinedBy": {
                "@id": "https://voc.iudx.org.in/"
            },
            "rdfs:label": "FeedEntity"
        },
        {
            "@id": "https://voc.iudx.org.in/Sequence",
            "@type": "owl:Class",
            "rdfs:comment": "A descriptor for the sequence of bus stops of a transit vehicle along a trip.",
            "rdfs:isDefinedBy": {
                "@id": "https://voc.iudx.org.in/"
            },
            "rdfs:label": "Sequence"
        },
        {
            "@id": "https://voc.iudx.org.in/StopTimeEvent",
            "@type": "owl:Class",
            "rdfs:comment": "Timing information for a single predicted event (either arrival or departure). Timing consists of delay and/or estimated time, and uncertainty.",
            "rdfs:isDefinedBy": {
                "@id": "https://voc.iudx.org.in/"
            },
            "rdfs:label": "StopTimeEvent"
        },
        {
            "@id": "https://voc.iudx.org.in/StopTimeUpdate",
            "@type": "owl:Class",
            "rdfs:comment": "A descriptor of realtime update for arrival and/or departure events for a given stop on a trip.",
            "rdfs:isDefinedBy": {
                "@id": "https://voc.iudx.org.in/"
            },
            "rdfs:label": "StopTimeUpdate"
        },
        {
            "@id": "https://voc.iudx.org.in/TripDescriptor",
            "@type": "owl:Class",
            "rdfs:comment": "A descriptor that identifies a single instance of a GTFS trip.",
            "rdfs:isDefinedBy": {
                "@id": "https://voc.iudx.org.in/"
            },
            "rdfs:label": "TripDescriptor"
        },
        {
            "@id": "https://voc.iudx.org.in/TripDetails",
            "@type": "owl:Class",
            "rdfs:comment": "A descriptor of realtime update on the schedule of a vehicle along a trip.",
            "rdfs:isDefinedBy": {
                "@id": "https://voc.iudx.org.in/"
            },
            "rdfs:label": "TripDetails"
        },
        {
            "@id": "https://voc.iudx.org.in/TripUpdate",
            "@type": "owl:Class",
            "rdfs:comment": "A descriptor of realtime update on the progress of a vehicle along a trip.",
            "rdfs:isDefinedBy": {
                "@id": "https://voc.iudx.org.in/"
            },
            "rdfs:label": "TripUpdate"
        },
        {
            "@id": "https://voc.iudx.org.in/VehicleDescriptor",
            "@type": "owl:Class",
            "rdfs:comment": "Identification information for the vehicle performing the trip.",
            "rdfs:isDefinedBy": {
                "@id": "https://voc.iudx.org.in/"
            },
            "rdfs:label": "VehicleDescriptor"
        },
        {
            "@id": "https://voc.iudx.org.in/VehiclePosition",
            "@type": "owl:Class",
            "rdfs:comment": "Realtime positioning information for a given vehicle.",
            "rdfs:isDefinedBy": {
                "@id": "https://voc.iudx.org.in/"
            },
            "rdfs:label": "VehiclePosition"
        },
        {
            "@id": "https://voc.iudx.org.in/MunicipalityDesc",
            "@type": "owl:Class",
            "rdfs:comment": "Municipality information corresponding to this observation.",
            "rdfs:isDefinedBy": {
                "@id": "https://voc.iudx.org.in/"
            },
            "rdfs:label": "MunicipalityDesc"
        },
        {
            "@id": "https://voc.iudx.org.in/Orientation",
            "@type": "owl:Class",
            "rdfs:comment": "Properties of the camera corresponding to this observation that indiactes its orientation.",
            "rdfs:isDefinedBy": {
                "@id": "https://voc.iudx.org.in/"
            },
            "rdfs:label": "Orientation"
        },
        {
            "@id": "https://voc.iudx.org.in/Streetlight",
            "@type": "owl:Class",
            "rdfs:comment": "A streetlight Data Model.",
            "rdfs:isDefinedBy": {
                "@id": "https://voc.iudx.org.in/"
            },
            "rdfs:label": "Streetlight",
            "rdfs:subClassOf": {
                "@id": "https://voc.iudx.org.in/StreetLight"
            }
        },
        {
            "@id": "https://voc.iudx.org.in/StreetLightFeeder",
            "@type": "owl:Class",
            "rdfs:comment": "A streetlight control panel Data Model.",
            "rdfs:isDefinedBy": {
                "@id": "https://voc.iudx.org.in/"
            },
            "rdfs:label": "StreetLightFeeder",
            "rdfs:subClassOf": {
                "@id": "https://voc.iudx.org.in/StreetLight"
            }
        },
        {
            "@id": "https://voc.iudx.org.in/BikeDockingStation",
            "@type": "owl:Class",
            "rdfs:comment": "A citizen bike hiring system Data Model.",
            "rdfs:isDefinedBy": {
                "@id": "https://voc.iudx.org.in/"
            },
            "rdfs:label": "BikeDockingStation",
            "rdfs:subClassOf": {
                "@id": "https://voc.iudx.org.in/UrbanMobility"
            }
        },
        {
            "@id": "https://voc.iudx.org.in/FareCollectionSystem",
            "@type": "owl:Class",
            "rdfs:comment": "A public transit fare collection system Data Model.",
            "rdfs:isDefinedBy": {
                "@id": "https://voc.iudx.org.in/"
            },
            "rdfs:label": "FareCollectionSystem",
            "rdfs:subClassOf": {
                "@id": "https://voc.iudx.org.in/UrbanMobility"
            }
        },
        {
            "@id": "https://voc.iudx.org.in/TrafficViolations",
            "@type": "owl:Class",
            "rdfs:comment": "A Data Model for Traffic Violations registered and E-Challans generated in Cities.",
            "rdfs:isDefinedBy": {
                "@id": "https://voc.iudx.org.in/"
            },
            "rdfs:label": "TrafficViolations",
            "rdfs:subClassOf": {
                "@id": "https://voc.iudx.org.in/UrbanMobility"
            }
        },
        {
            "@id": "https://voc.iudx.org.in/TransitManagement",
            "@type": "owl:Class",
            "rdfs:comment": "A public transit system Data Model.",
            "rdfs:isDefinedBy": {
                "@id": "https://voc.iudx.org.in/"
            },
            "rdfs:label": "TransitManagement",
            "rdfs:subClassOf": {
                "@id": "https://voc.iudx.org.in/UrbanMobility"
            }
        },
        {
            "@id": "https://voc.iudx.org.in/Version",
            "@type": "owl:Class",
            "rdfs:comment": "Version information associated with the observations.",
            "rdfs:isDefinedBy": {
                "@id": "https://voc.iudx.org.in/"
            },
            "rdfs:label": "Version"
        },
        {
            "@id": "https://voc.iudx.org.in/Camera",
            "@type": "owl:Class",
            "rdfs:comment": "A Data Model for camera installations in a city.",
            "rdfs:isDefinedBy": {
                "@id": "https://voc.iudx.org.in/"
            },
            "rdfs:label": "Camera",
            "rdfs:subClassOf": {
                "@id": "https://voc.iudx.org.in/VideoSystems"
            }
        },
        {
            "@id": "https://voc.iudx.org.in/WasteBinModel",
            "@type": "owl:Class",
            "rdfs:comment": "Properties of the waste bin that could have sensors which report measurements corresponding to this observation.",
            "rdfs:isDefinedBy": {
                "@id": "https://voc.iudx.org.in/"
            },
            "rdfs:label": "WasteBinModel"
        },
        {
            "@id": "https://voc.iudx.org.in/WasteWaterMgmt",
            "@type": "owl:Class",
            "rdfs:comment": "Data model for waste water treatment plant.",
            "rdfs:isDefinedBy": {
                "@id": "https://voc.iudx.org.in/"
            },
            "rdfs:label": "WasteWaterMgmt",
            "rdfs:subClassOf": {
                "@id": "https://voc.iudx.org.in/WasteManagement"
            }
        },
        {
            "@id": "https://voc.iudx.org.in/WmgmtBin",
            "@type": "owl:Class",
            "rdfs:comment": "Data model for solid waste management bins.",
            "rdfs:isDefinedBy": {
                "@id": "https://voc.iudx.org.in/"
            },
            "rdfs:label": "WmgmtBin",
            "rdfs:subClassOf": {
                "@id": "https://voc.iudx.org.in/WasteManagement"
            }
        },
        {
            "@id": "https://voc.iudx.org.in/WmgmtVehicle",
            "@type": "owl:Class",
            "rdfs:comment": "Data model for solid waste management vehicles.",
            "rdfs:isDefinedBy": {
                "@id": "https://voc.iudx.org.in/"
            },
            "rdfs:label": "WmgmtVehicle",
            "rdfs:subClassOf": {
                "@id": "https://voc.iudx.org.in/WasteManagement"
            }
        },
        {
            "@id": "https://voc.iudx.org.in/EmployeeDetails",
            "@type": "owl:Class",
            "rdfs:comment": "A Data Model for employee information in an organization.",
            "rdfs:isDefinedBy": {
                "@id": "https://voc.iudx.org.in/"
            },
            "rdfs:label": "EmployeeDetails",
            "rdfs:subClassOf": {
                "@id": "https://voc.iudx.org.in/WorkPlace"
            }
        },
        {
            "@id": "https://voc.iudx.org.in/AccessObjectInfoValue",
            "@type": "owl:Class",
            "rdfs:comment": "Describes information on accessing data from a given resource.",
            "rdfs:isDefinedBy": {
                "@id": "https://voc.iudx.org.in/"
            },
            "rdfs:label": "AccessObjectInfoValue",
            "rdfs:subClassOf": {
                "@id": "https://voc.iudx.org.in/StructuredValue"
            }
        },
        {
            "@id": "https://voc.iudx.org.in/AuthServerInfoValue",
            "@type": "owl:Class",
            "rdfs:comment": "Describes information about the IUDX Authorization Server for a given resource.",
            "rdfs:isDefinedBy": {
                "@id": "https://voc.iudx.org.in/"
            },
            "rdfs:label": "AuthServerInfoValue",
            "rdfs:subClassOf": {
                "@id": "https://voc.iudx.org.in/StructuredValue"
            }
        },
        {
            "@id": "https://voc.iudx.org.in/Class",
            "@type": "owl:Class",
            "rdfs:comment": "A class, also often called a 'Type'; equivalent to rdfs:Class.",
            "rdfs:isDefinedBy": {
                "@id": "https://voc.iudx.org.in/"
            },
            "rdfs:label": "Class",
            "rdfs:subClassOf": {
                "@id": "https://voc.iudx.org.in/Intangible"
            }
        },
        {
            "@id": "https://voc.iudx.org.in/DataDescriptor",
            "@type": "owl:Class",
            "rdfs:comment": "Describes the Data Descriptor Object embedded in another IUDX entity. It provides meta-information about various data fields associated with a resource.",
            "rdfs:isDefinedBy": {
                "@id": "https://voc.iudx.org.in/"
            },
            "rdfs:label": "DataDescriptor",
            "rdfs:subClassOf": {
                "@id": "https://voc.iudx.org.in/StructuredValue"
            }
        },
        {
            "@id": "https://voc.iudx.org.in/DataFieldListValue",
            "@type": "owl:Class",
            "rdfs:comment": "Lists various fields associated with the data available from a given group of resource items.",
            "rdfs:isDefinedBy": {
                "@id": "https://voc.iudx.org.in/"
            },
            "rdfs:label": "DataFieldListValue",
            "rdfs:subClassOf": {
                "@id": "https://voc.iudx.org.in/StructuredValue"
            }
        },
        {
            "@id": "https://voc.iudx.org.in/DataModel",
            "@type": "owl:Class",
            "rdfs:comment": "Class of all Data Models.",
            "rdfs:isDefinedBy": {
                "@id": "https://voc.iudx.org.in/"
            },
            "rdfs:label": "DataModel",
            "rdfs:subClassOf": {
                "@id": "https://voc.iudx.org.in/Thing"
            }
        },
        {
            "@id": "https://voc.iudx.org.in/Feature",
            "@type": "owl:Class",
            "rdfs:comment": "Describes the GeoJSON Feature",
            "rdfs:isDefinedBy": {
                "@id": "https://voc.iudx.org.in/"
            },
            "rdfs:label": "Feature",
            "rdfs:subClassOf": {
                "@id": "https://voc.iudx.org.in/GeoJSONGeometry"
            },
            "skos:exactMatch": {
                "@id": "https://purl.org/geojson/vocab#Feature"
            }
        },
        {
            "@id": "https://voc.iudx.org.in/FunctionDescription",
            "@type": "owl:Class",
            "rdfs:comment": "Description of a function associated in computation of a quanitative value.",
            "rdfs:isDefinedBy": {
                "@id": "https://voc.iudx.org.in/"
            },
            "rdfs:label": "FunctionDescription",
            "rdfs:subClassOf": {
                "@id": "https://voc.iudx.org.in/Intangible"
            }
        },
        {
            "@id": "https://voc.iudx.org.in/GeoCoordinates",
            "@type": "owl:Class",
            "rdfs:comment": "Geo coordinates in Latitude and Longitude for a given place. The Lat/Long values are in WGS84 notation",
            "rdfs:isDefinedBy": {
                "@id": "https://voc.iudx.org.in/"
            },
            "rdfs:label": "GeoCoordinates",
            "rdfs:subClassOf": {
                "@id": "https://voc.iudx.org.in/StructuredValue"
            },
            "skos:exactMatch": {
                "@id": "http://schema.org/GeoCoordinates"
            }
        },
        {
            "@id": "https://voc.iudx.org.in/GeoJSONGeometry",
            "@type": "owl:Class",
            "rdfs:comment": "Describes the GeoJSON object",
            "rdfs:isDefinedBy": {
                "@id": "https://voc.iudx.org.in/"
            },
            "rdfs:label": "GeoJSONGeometry",
            "rdfs:subClassOf": {
                "@id": "https://voc.iudx.org.in/StructuredValue"
            }
        },
        {
            "@id": "https://voc.iudx.org.in/GeoProperty",
            "@type": "owl:Class",
            "rdfs:comment": "Describes the class of all GeoProperties in IUDX. The range of a geo-property are objects describing geo-coordinates (e.g., latitude, longitude, GeoJSON objects etc.)",
            "rdfs:isDefinedBy": {
                "@id": "https://voc.iudx.org.in/"
            },
            "rdfs:label": "GeoProperty",
            "rdfs:subClassOf": {
                "@id": "https://voc.iudx.org.in/StructuredProperty"
            }
        },
        {
            "@id": "https://voc.iudx.org.in/Intangible",
            "@type": "owl:Class",
            "rdfs:comment": "Class of all intangible things like Structured valued objects etc.",
            "rdfs:isDefinedBy": {
                "@id": "https://voc.iudx.org.in/"
            },
            "rdfs:label": "Intangible",
            "rdfs:subClassOf": {
                "@id": "https://voc.iudx.org.in/Thing"
            }
        },
        {
            "@id": "https://voc.iudx.org.in/IUDXEntity",
            "@type": "owl:Class",
            "rdfs:comment": "Class of all IUDX Entities (Resource, ResourceGroup, ResourceServer, Provider etc.)",
            "rdfs:isDefinedBy": {
                "@id": "https://voc.iudx.org.in/"
            },
            "rdfs:label": "IUDXEntity",
            "rdfs:subClassOf": {
                "@id": "https://voc.iudx.org.in/Thing"
            }
        },
        {
            "@id": "https://voc.iudx.org.in/LineString",
            "@type": "owl:Class",
            "rdfs:comment": "Describes the GeoJSON LineString",
            "rdfs:isDefinedBy": {
                "@id": "https://voc.iudx.org.in/"
            },
            "rdfs:label": "LineString",
            "rdfs:subClassOf": {
                "@id": "https://voc.iudx.org.in/GeoJSONGeometry"
            },
            "skos:exactMatch": {
                "@id": "https://purl.org/geojson/vocab#LineString"
            }
        },
        {
            "@id": "https://voc.iudx.org.in/ModelInfo",
            "@type": "owl:Class",
            "rdfs:comment": "Describes the manufacture information of the device, sensor or system in consideration.",
            "rdfs:isDefinedBy": {
                "@id": "https://voc.iudx.org.in/"
            },
            "rdfs:label": "ModelInfo",
            "rdfs:subClassOf": {
                "@id": "https://voc.iudx.org.in/Thing"
            }
        },
        {
            "@id": "https://voc.iudx.org.in/Organization",
            "@type": "owl:Class",
            "rdfs:comment": "Information about a given organization (contact info, email, urls etc.)",
            "rdfs:isDefinedBy": {
                "@id": "https://voc.iudx.org.in/"
            },
            "rdfs:label": "Organization",
            "rdfs:subClassOf": {
                "@id": "https://voc.iudx.org.in/Thing"
            },
            "skos:exactMatch": {
                "@id": "http://schema.org/Organization"
            }
        },
        {
            "@id": "https://voc.iudx.org.in/Place",
            "@type": "owl:Class",
            "rdfs:comment": "Describes fixed location for various entities. The places can be described using geo-Coordinates (points, polgons, bboxes etc.) , structured form of addresses or simple address strings.",
            "rdfs:isDefinedBy": {
                "@id": "https://voc.iudx.org.in/"
            },
            "rdfs:label": "Place",
            "rdfs:subClassOf": {
                "@id": "https://voc.iudx.org.in/Thing"
            },
            "skos:closeMatch": {
                "@id": "http://schema.org/Place"
            }
        },
        {
            "@id": "https://voc.iudx.org.in/Point",
            "@type": "owl:Class",
            "rdfs:comment": "Describes the GeoJSON Point",
            "rdfs:isDefinedBy": {
                "@id": "https://voc.iudx.org.in/"
            },
            "rdfs:label": "Point",
            "rdfs:subClassOf": {
                "@id": "https://voc.iudx.org.in/GeoJSONGeometry"
            },
            "skos:exactMatch": {
                "@id": "https://purl.org/geojson/vocab#Point"
            }
        },
        {
            "@id": "https://voc.iudx.org.in/Polygon",
            "@type": "owl:Class",
            "rdfs:comment": "Describes the GeoJSON Polygon",
            "rdfs:isDefinedBy": {
                "@id": "https://voc.iudx.org.in/"
            },
            "rdfs:label": "Polygon",
            "rdfs:subClassOf": {
                "@id": "https://voc.iudx.org.in/GeoJSONGeometry"
            },
            "skos:exactMatch": {
                "@id": "https://purl.org/geojson/vocab#Polygon"
            }
        },
        {
            "@id": "https://voc.iudx.org.in/Provider",
            "@type": "owl:Class",
            "rdfs:comment": "Describes the Provider entity in the IUDX catalogue.",
            "rdfs:isDefinedBy": {
                "@id": "https://voc.iudx.org.in/"
            },
            "rdfs:label": "Provider",
            "rdfs:subClassOf": {
                "@id": "https://voc.iudx.org.in/IUDXEntity"
            }
        },
        {
            "@id": "https://voc.iudx.org.in/QuantitativeProperty",
            "@type": "owl:Class",
            "rdfs:comment": "Class of all Quantitative properties in IUDX. The range of Quantitative properties are objects describing the associated values as well as meta-information associated with the values. Typically, the value of quantiative property isa numeric value. However, in some cases, it may be a string that has to be interpreted as a number.",
            "rdfs:isDefinedBy": {
                "@id": "https://voc.iudx.org.in/"
            },
            "rdfs:label": "QuantitativeProperty",
            "rdfs:subClassOf": {
                "@id": "https://voc.iudx.org.in/StructuredProperty"
            }
        },
        {
            "@id": "https://voc.iudx.org.in/Relationship",
            "@type": "owl:Class",
            "rdfs:comment": "Class of all Relationships in IUDX. A relationship property relates a resource to another resource. The range of relationship property are objects describing the links (URIs etc.) to the related resource and may contain meta-information about the type of relationship.",
            "rdfs:isDefinedBy": {
                "@id": "https://voc.iudx.org.in/"
            },
            "rdfs:label": "Relationship",
            "rdfs:subClassOf": {
                "@id": "https://voc.iudx.org.in/Property"
            }
        },
        {
            "@id": "https://voc.iudx.org.in/RelationshipValue",
            "@type": "owl:Class",
            "rdfs:comment": "Describes the value of a Relationship Object.",
            "rdfs:isDefinedBy": {
                "@id": "https://voc.iudx.org.in/"
            },
            "rdfs:label": "RelationshipValue",
            "rdfs:subClassOf": {
                "@id": "https://voc.iudx.org.in/StructuredValue"
            }
        },
        {
            "@id": "https://voc.iudx.org.in/Resource",
            "@type": "owl:Class",
            "rdfs:comment": "Describes the Resource entity in the IUDX catalogue.",
            "rdfs:isDefinedBy": {
                "@id": "https://voc.iudx.org.in/"
            },
            "rdfs:label": "Resource",
            "rdfs:subClassOf": {
                "@id": "https://voc.iudx.org.in/IUDXEntity"
            }
        },
        {
            "@id": "https://voc.iudx.org.in/ResourceGroup",
            "@type": "owl:Class",
            "rdfs:comment": "Describes the Resource Group entity in the IUDX catalogue.",
            "rdfs:isDefinedBy": {
                "@id": "https://voc.iudx.org.in/"
            },
            "rdfs:label": "ResourceGroup",
            "rdfs:subClassOf": {
                "@id": "https://voc.iudx.org.in/IUDXEntity"
            }
        },
        {
            "@id": "https://voc.iudx.org.in/ResourceServer",
            "@type": "owl:Class",
            "rdfs:comment": "Describes the Resource Server entry in the IUDX catalogue.",
            "rdfs:isDefinedBy": {
                "@id": "https://voc.iudx.org.in/"
            },
            "rdfs:label": "ResourceServer",
            "rdfs:subClassOf": {
                "@id": "https://voc.iudx.org.in/IUDXEntity"
            }
        },
        {
            "@id": "https://voc.iudx.org.in/StructuredProperty",
            "@type": "owl:Class",
            "rdfs:comment": "Describes the class of all properties in IUDX that have a complex JSON structures and cannot be described using simple strings and native data types.",
            "rdfs:isDefinedBy": {
                "@id": "https://voc.iudx.org.in/"
            },
            "rdfs:label": "StructuredProperty",
            "rdfs:subClassOf": {
                "@id": "https://voc.iudx.org.in/Property"
            }
        },
        {
            "@id": "https://voc.iudx.org.in/StructuredValue",
            "@type": "owl:Class",
            "rdfs:comment": "Describes a generic nested JSON structured value",
            "rdfs:isDefinedBy": {
                "@id": "https://voc.iudx.org.in/"
            },
            "rdfs:label": "StructuredValue",
            "rdfs:subClassOf": {
                "@id": "https://voc.iudx.org.in/Intangible"
            }
        },
        {
            "@id": "https://voc.iudx.org.in/TextProperty",
            "@type": "owl:Class",
            "rdfs:comment": "Class of all Text Properties. The range of Text property contains text (multiple words).",
            "rdfs:isDefinedBy": {
                "@id": "https://voc.iudx.org.in/"
            },
            "rdfs:label": "TextProperty",
            "rdfs:subClassOf": {
                "@id": "https://voc.iudx.org.in/Property"
            }
        },
        {
            "@id": "https://voc.iudx.org.in/Thing",
            "@type": "owl:Class",
            "rdfs:comment": "Most generic IUDX object.",
            "rdfs:isDefinedBy": {
                "@id": "https://voc.iudx.org.in/"
            },
            "rdfs:label": "Thing",
            "skos:exactMatch": {
                "@id": "http://schema.org/Thing"
            }
        },
        {
            "@id": "https://voc.iudx.org.in/TimeProperty",
            "@type": "owl:Class",
            "rdfs:comment": "Class of all Time properties in IUDX. The range of time property is a time/date objects in standard formats.",
            "rdfs:isDefinedBy": {
                "@id": "https://voc.iudx.org.in/"
            },
            "rdfs:label": "TimeProperty",
            "rdfs:subClassOf": {
                "@id": "https://voc.iudx.org.in/rdf"
            }
        },
        {
            "@id": "https://voc.iudx.org.in/TimeSeriesAggregation",
            "@type": "owl:Class",
            "rdfs:comment": "This object describes various types of aggregated data associated with a time-seried data. For example, average over a certain duration in past, minimum value over a duration in past etc.",
            "rdfs:isDefinedBy": {
                "@id": "https://voc.iudx.org.in/"
            },
            "rdfs:label": "TimeSeriesAggregation",
            "rdfs:subClassOf": {
                "@id": "https://voc.iudx.org.in/Intangible"
            }
        },
        {
            "@id": "https://voc.iudx.org.in/ValueDescriptor",
            "@type": "owl:Class",
            "rdfs:comment": "Value descriptors are JSON objects that describes the value object for a given property.",
            "rdfs:isDefinedBy": {
                "@id": "https://voc.iudx.org.in/"
            },
            "rdfs:label": "ValueDescriptor",
            "rdfs:subClassOf": {
                "@id": "https://voc.iudx.org.in/Intangible"
            }
        },
        {
            "@id": "https://voc.iudx.org.in/Boolean",
            "@type": "owl:Class",
            "rdfs:comment": "Data type: True or False",
            "rdfs:isDefinedBy": {
                "@id": "https://voc.iudx.org.in/"
            },
            "rdfs:label": "Boolean",
            "skos:exactMatch": {
                "@id": "http://schema.org/Boolean"
            }
        },
        {
            "@id": "https://voc.iudx.org.in/DateTime",
            "@type": "owl:Class",
            "rdfs:comment": "Describes ISO Time in a DateTime format as specified in ISO 8601",
            "rdfs:isDefinedBy": {
                "@id": "https://voc.iudx.org.in/"
            },
            "rdfs:label": "DateTime",
            "skos:exactMatch": {
                "@id": "http://schema.org/DateTime"
            }
        },
        {
            "@id": "https://voc.iudx.org.in/Number",
            "@type": "owl:Class",
            "rdfs:comment": "Data type: Number for representing numeric values (Decimals, Integers, etc)",
            "rdfs:isDefinedBy": {
                "@id": "https://voc.iudx.org.in/"
            },
            "rdfs:label": "Number",
            "skos:exactMatch": {
                "@id": "http://schema.org/Number"
            }
        },
        {
            "@id": "https://voc.iudx.org.in/NumericArray",
            "@type": "owl:Class",
            "rdfs:comment": "Data type: Array of numbers, for representing numeric values (Decimals, Integers, etc)",
            "rdfs:isDefinedBy": {
                "@id": "https://voc.iudx.org.in/"
            },
            "rdfs:label": "NumericArray"
        },
        {
            "@id": "https://voc.iudx.org.in/Text",
            "@type": "owl:Class",
            "rdfs:comment": "Data type: Text for string values",
            "rdfs:isDefinedBy": {
                "@id": "https://voc.iudx.org.in/"
            },
            "rdfs:label": "Text",
            "skos:exactMatch": {
                "@id": "http://schema.org/Text"
            }
        },
        {
            "@id": "https://voc.iudx.org.in/Civic",
            "@type": "owl:Class",
            "rdfs:comment": "Data models that pertain to the citizen issues/civic domain",
            "rdfs:isDefinedBy": {
                "@id": "https://voc.iudx.org.in/"
            },
            "rdfs:label": "Civic",
            "rdfs:subClassOf": {
                "@id": "https://voc.iudx.org.in/DataModel"
            }
        },
        {
            "@id": "https://voc.iudx.org.in/Environment",
            "@type": "owl:Class",
            "rdfs:comment": "Data models that pertain to the environment domain",
            "rdfs:isDefinedBy": {
                "@id": "https://voc.iudx.org.in/"
            },
            "rdfs:label": "Environment",
            "rdfs:subClassOf": {
                "@id": "https://voc.iudx.org.in/DataModel"
            }
        },
        {
            "@id": "https://voc.iudx.org.in/StreetLight",
            "@type": "owl:Class",
            "rdfs:comment": "Data models that pertain to the streetlight domain",
            "rdfs:isDefinedBy": {
                "@id": "https://voc.iudx.org.in/"
            },
            "rdfs:label": "StreetLight",
            "rdfs:subClassOf": {
                "@id": "https://voc.iudx.org.in/DataModel"
            }
        },
        {
            "@id": "https://voc.iudx.org.in/UrbanMobility",
            "@type": "owl:Class",
            "rdfs:comment": "Data models that pertain to the urban mobility domain",
            "rdfs:isDefinedBy": {
                "@id": "https://voc.iudx.org.in/"
            },
            "rdfs:label": "UrbanMobility",
            "rdfs:subClassOf": {
                "@id": "https://voc.iudx.org.in/DataModel"
            }
        },
        {
            "@id": "https://voc.iudx.org.in/VideoSystems",
            "@type": "owl:Class",
            "rdfs:comment": "Data models that pertain to surveillance or traffic cameras",
            "rdfs:isDefinedBy": {
                "@id": "https://voc.iudx.org.in/"
            },
            "rdfs:label": "VideoSystems",
            "rdfs:subClassOf": {
                "@id": "https://voc.iudx.org.in/DataModel"
            }
        },
        {
            "@id": "https://voc.iudx.org.in/WasteManagement",
            "@type": "owl:Class",
            "rdfs:comment": "Data models that pertain to the waste management domain",
            "rdfs:isDefinedBy": {
                "@id": "https://voc.iudx.org.in/"
            },
            "rdfs:label": "WasteManagement",
            "rdfs:subClassOf": {
                "@id": "https://voc.iudx.org.in/DataModel"
            }
        },
        {
            "@id": "https://voc.iudx.org.in/WorkPlace",
            "@type": "owl:Class",
            "rdfs:comment": "Data models that pertain to organization domain",
            "rdfs:isDefinedBy": {
                "@id": "https://voc.iudx.org.in/"
            },
            "rdfs:label": "WorkPlace",
            "rdfs:subClassOf": {
                "@id": "https://voc.iudx.org.in/DataModel"
            }
        },
        {
            "@id": "https://voc.iudx.org.in/amountCollected",
            "@type": [
                "iudx:QuantitativeProperty"
            ],
            "iudx:domainIncludes": [
                {
                    "@id": "iudx:RevenueCollection"
                },
                {
                    "@id": "iudx:TrafficViolations"
                }
            ],
            "iudx:rangeIncludes": [
                {
                    "@id": "iudx:Number"
                },
                {
                    "@id": "iudx:ValueDescriptor"
                }
            ],
            "rdfs:comment": "Amount collected towards the service corresponding to this observation.",
            "rdfs:isDefinedBy": {
                "@id": "https://voc.iudx.org.in/"
            },
            "rdfs:label": "amountCollected"
        },
        {
            "@id": "https://voc.iudx.org.in/category",
            "@type": [
                "iudx:TextProperty"
            ],
            "iudx:domainIncludes": [
                {
                    "@id": "iudx:IssueReporting"
                }
            ],
            "iudx:rangeIncludes": [
                {
                    "@id": "iudx:Text"
                },
                {
                    "@id": "iudx:ValueDescriptor"
                }
            ],
            "rdfs:comment": "The category name corresponding to the issue that has been reported.",
            "rdfs:isDefinedBy": {
                "@id": "https://voc.iudx.org.in/"
            },
            "rdfs:label": "category",
            "skos:exactMatch": {
                "@id": "http://ontology.eil.utoronto.ca/open311.owl#group"
            }
        },
        {
            "@id": "https://voc.iudx.org.in/categoryCode",
            "@type": [
                "iudx:TextProperty"
            ],
            "iudx:domainIncludes": [
                {
                    "@id": "iudx:IssueReporting"
                }
            ],
            "iudx:rangeIncludes": [
                {
                    "@id": "iudx:Text"
                },
                {
                    "@id": "iudx:ValueDescriptor"
                }
            ],
            "rdfs:comment": "Unique identifier for the category corresponding to the issue reported.",
            "rdfs:isDefinedBy": {
                "@id": "https://voc.iudx.org.in/"
            },
            "rdfs:label": "categoryCode"
        },
        {
            "@id": "https://voc.iudx.org.in/cl",
            "@type": [
                "iudx:QuantitativeProperty"
            ],
            "iudx:domainIncludes": [
                {
                    "@id": "iudx:WaterDistributionNetwork"
                }
            ],
            "iudx:rangeIncludes": [
                {
                    "@id": "iudx:TimeSeriesAggregation"
                },
                {
                    "@id": "iudx:ValueDescriptor"
                }
            ],
            "rdfs:comment": "Concentration of chlorides in the water.",
            "rdfs:isDefinedBy": {
                "@id": "https://voc.iudx.org.in/"
            },
            "rdfs:label": "cl",
            "skos:exactMatch": {
                "@id": "https://uri.fiware.org/ns/data-models#WaterQualityObserved.Cl"
            }
        },
        {
            "@id": "https://voc.iudx.org.in/department",
            "@type": [
                "iudx:TextProperty"
            ],
            "iudx:domainIncludes": [
                {
                    "@id": "iudx:IssueReporting"
                }
            ],
            "iudx:rangeIncludes": [
                {
                    "@id": "iudx:Text"
                },
                {
                    "@id": "iudx:ValueDescriptor"
                }
            ],
            "rdfs:comment": "The department which is associated with the service or the issue corresponding to this observation.",
            "rdfs:isDefinedBy": {
                "@id": "https://voc.iudx.org.in/"
            },
            "rdfs:label": "department"
        },
        {
            "@id": "https://voc.iudx.org.in/departmentID",
            "@type": [
                "iudx:TextProperty"
            ],
            "iudx:domainIncludes": [
                {
                    "@id": "iudx:IssueReporting"
                }
            ],
            "iudx:rangeIncludes": [
                {
                    "@id": "iudx:Text"
                },
                {
                    "@id": "iudx:ValueDescriptor"
                }
            ],
            "rdfs:comment": "Unique ID or code associated with the department which is associated with the service or the issue corresponding to this observation.",
            "rdfs:isDefinedBy": {
                "@id": "https://voc.iudx.org.in/"
            },
            "rdfs:label": "departmentID"
        },
        {
            "@id": "https://voc.iudx.org.in/ecRecoveryAmount",
            "@type": [
                "iudx:QuantitativeProperty"
            ],
            "iudx:domainIncludes": [
                {
                    "@id": "iudx:RevenueCollection"
                }
            ],
            "iudx:rangeIncludes": [
                {
                    "@id": "iudx:Number"
                },
                {
                    "@id": "iudx:ValueDescriptor"
                }
            ],
            "rdfs:comment": "Amount collected towards Enrollment Certificate from the establishment on annual basis.",
            "rdfs:isDefinedBy": {
                "@id": "https://voc.iudx.org.in/"
            },
            "rdfs:label": "ecRecoveryAmount"
        },
        {
            "@id": "https://voc.iudx.org.in/flowrate",
            "@type": [
                "iudx:QuantitativeProperty"
            ],
            "iudx:domainIncludes": [
                {
                    "@id": "iudx:WaterDistributionNetwork"
                }
            ],
            "iudx:rangeIncludes": [
                {
                    "@id": "iudx:Number"
                },
                {
                    "@id": "iudx:ValueDescriptor"
                }
            ],
            "rdfs:comment": "Volume of water flowing in/out of the water storage tank corresponding to this observation.",
            "rdfs:isDefinedBy": {
                "@id": "https://voc.iudx.org.in/"
            },
            "rdfs:label": "flowrate",
            "skos:exactMatch": {
                "@id": "https://uri.fiware.org/ns/data-models#WasteWaterJunction.flowrate"
            }
        },
        {
            "@id": "https://voc.iudx.org.in/pH",
            "@type": [
                "iudx:QuantitativeProperty"
            ],
            "iudx:domainIncludes": [
                {
                    "@id": "iudx:WaterDistributionNetwork"
                },
                {
                    "@id": "iudx:WasteWaterMgmt"
                }
            ],
            "iudx:rangeIncludes": [
                {
                    "@id": "iudx:TimeSeriesAggregation"
                },
                {
                    "@id": "iudx:ValueDescriptor"
                }
            ],
            "rdfs:comment": "Acidity level or basicity level obsevered in the water.",
            "rdfs:isDefinedBy": {
                "@id": "https://voc.iudx.org.in/"
            },
            "rdfs:label": "pH",
            "skos:exactMatch": {
                "@id": "https://uri.fiware.org/ns/data-models#WaterQualityObserved.pH"
            }
        },
        {
            "@id": "https://voc.iudx.org.in/rcRecoveryAmount",
            "@type": [
                "iudx:QuantitativeProperty"
            ],
            "iudx:domainIncludes": [
                {
                    "@id": "iudx:RevenueCollection"
                }
            ],
            "iudx:rangeIncludes": [
                {
                    "@id": "iudx:Number"
                },
                {
                    "@id": "iudx:ValueDescriptor"
                }
            ],
            "rdfs:comment": "Amount collected towards Registration Certificate on monthly basis from the establishment per emplyoee.",
            "rdfs:isDefinedBy": {
                "@id": "https://voc.iudx.org.in/"
            },
            "rdfs:label": "rcRecoveryAmount"
        },
        {
            "@id": "https://voc.iudx.org.in/reportID",
            "@type": [
                "iudx:TextProperty"
            ],
            "iudx:domainIncludes": [
                {
                    "@id": "iudx:IssueReporting"
                },
                {
                    "@id": "iudx:SafetiPin"
                },
                {
                    "@id": "iudx:TrafficViolations"
                },
                {
                    "@id": "iudx:WmgmtVehicle"
                }
            ],
            "iudx:rangeIncludes": [
                {
                    "@id": "iudx:Text"
                },
                {
                    "@id": "iudx:ValueDescriptor"
                }
            ],
            "rdfs:comment": "Unique ID assigned for the issue or report or feedback or transaction corresponding to this observation.",
            "rdfs:isDefinedBy": {
                "@id": "https://voc.iudx.org.in/"
            },
            "rdfs:label": "reportID",
            "skos:exactMatch": {
                "@id": "http://ontology.eil.utoronto.ca/open311.owl#servicecode"
            }
        },
        {
            "@id": "https://voc.iudx.org.in/resolutionStatus",
            "@type": [
                "iudx:TextProperty"
            ],
            "iudx:domainIncludes": [
                {
                    "@id": "iudx:IssueReporting"
                }
            ],
            "iudx:rangeIncludes": [
                {
                    "@id": "iudx:Text"
                },
                {
                    "@id": "iudx:ValueDescriptor"
                }
            ],
            "rdfs:comment": "Status of the issue that was reported in terms of resolution or the actions taken on it. Could be Open, Assigned, InProgress, Unassigned, Closed.",
            "rdfs:isDefinedBy": {
                "@id": "https://voc.iudx.org.in/"
            },
            "rdfs:label": "resolutionStatus"
        },
        {
            "@id": "https://voc.iudx.org.in/revenueCollectionType",
            "@type": [
                "iudx:TextProperty"
            ],
            "iudx:domainIncludes": [
                {
                    "@id": "iudx:RevenueCollection"
                }
            ],
            "iudx:rangeIncludes": [
                {
                    "@id": "iudx:Text"
                },
                {
                    "@id": "iudx:ValueDescriptor"
                }
            ],
            "rdfs:comment": "Type of source from which the city administration collects the revenue, could be property tax, vehicle registration, party hall booking, community hall booking, auditorium booking etc.",
            "rdfs:isDefinedBy": {
                "@id": "https://voc.iudx.org.in/"
            },
            "rdfs:label": "revenueCollectionType"
        },
        {
            "@id": "https://voc.iudx.org.in/safetiPinScore",
            "@type": [
                "iudx:QuantitativeProperty"
            ],
            "iudx:domainIncludes": [
                {
                    "@id": "iudx:SafetiPin"
                }
            ],
            "iudx:rangeIncludes": [
                {
                    "@id": "iudx:Number"
                },
                {
                    "@id": "iudx:ValueDescriptor"
                }
            ],
            "rdfs:comment": "Score given to the location corresponding to this observation. The score is on a scale of 5 if the SafetiPinType is 'Feeling' and on a scale of 10 if the SafetiPinType is 'Audit'",
            "rdfs:isDefinedBy": {
                "@id": "https://voc.iudx.org.in/"
            },
            "rdfs:label": "safetiPinScore"
        },
        {
            "@id": "https://voc.iudx.org.in/subCategory",
            "@type": [
                "iudx:TextProperty"
            ],
            "iudx:domainIncludes": [
                {
                    "@id": "iudx:IssueReporting"
                }
            ],
            "iudx:rangeIncludes": [
                {
                    "@id": "iudx:Text"
                },
                {
                    "@id": "iudx:ValueDescriptor"
                }
            ],
            "rdfs:comment": "The sub-category name corresponding to the issue that has been reported.",
            "rdfs:isDefinedBy": {
                "@id": "https://voc.iudx.org.in/"
            },
            "rdfs:label": "subCategory"
        },
        {
            "@id": "https://voc.iudx.org.in/subCategoryCode",
            "@type": [
                "iudx:TextProperty"
            ],
            "iudx:domainIncludes": [
                {
                    "@id": "iudx:IssueReporting"
                }
            ],
            "iudx:rangeIncludes": [
                {
                    "@id": "iudx:Text"
                },
                {
                    "@id": "iudx:ValueDescriptor"
                }
            ],
            "rdfs:comment": "Unique identifier for the sub-category corresponding to the issue reported.",
            "rdfs:isDefinedBy": {
                "@id": "https://voc.iudx.org.in/"
            },
            "rdfs:label": "subCategoryCode"
        },
        {
            "@id": "https://voc.iudx.org.in/tankBreadth",
            "@type": [
                "iudx:QuantitativeProperty"
            ],
            "iudx:domainIncludes": [
                {
                    "@id": "iudx:WaterDistributionNetwork"
                }
            ],
            "iudx:rangeIncludes": [
                {
                    "@id": "iudx:Number"
                },
                {
                    "@id": "iudx:ValueDescriptor"
                }
            ],
            "rdfs:comment": "Breadth of the Cuboid shaped water storage tank.",
            "rdfs:isDefinedBy": {
                "@id": "https://voc.iudx.org.in/"
            },
            "rdfs:label": "tankBreadth"
        },
        {
            "@id": "https://voc.iudx.org.in/tankCapacity",
            "@type": [
                "iudx:QuantitativeProperty"
            ],
            "iudx:domainIncludes": [
                {
                    "@id": "iudx:WaterDistributionNetwork"
                }
            ],
            "iudx:rangeIncludes": [
                {
                    "@id": "iudx:Number"
                },
                {
                    "@id": "iudx:ValueDescriptor"
                }
            ],
            "rdfs:comment": "Maximum amount of water the water storage tank corresponding to this observation can hold.",
            "rdfs:isDefinedBy": {
                "@id": "https://voc.iudx.org.in/"
            },
            "rdfs:label": "tankCapacity"
        },
        {
            "@id": "https://voc.iudx.org.in/tankDepth",
            "@type": [
                "iudx:QuantitativeProperty"
            ],
            "iudx:domainIncludes": [
                {
                    "@id": "iudx:WaterDistributionNetwork"
                }
            ],
            "iudx:rangeIncludes": [
                {
                    "@id": "iudx:Number"
                },
                {
                    "@id": "iudx:ValueDescriptor"
                }
            ],
            "rdfs:comment": "Depth of the water storage tank corresponding to this observation.",
            "rdfs:isDefinedBy": {
                "@id": "https://voc.iudx.org.in/"
            },
            "rdfs:label": "tankdepth"
        },
        {
            "@id": "https://voc.iudx.org.in/tankDiameter",
            "@type": [
                "iudx:QuantitativeProperty"
            ],
            "iudx:domainIncludes": [
                {
                    "@id": "iudx:WaterDistributionNetwork"
                }
            ],
            "iudx:rangeIncludes": [
                {
                    "@id": "iudx:Number"
                },
                {
                    "@id": "iudx:ValueDescriptor"
                }
            ],
            "rdfs:comment": "Diameter of Cylindrical or Spherical water storage tanks.",
            "rdfs:isDefinedBy": {
                "@id": "https://voc.iudx.org.in/"
            },
            "rdfs:label": "tankDiameter"
        },
        {
            "@id": "https://voc.iudx.org.in/tankLength",
            "@type": [
                "iudx:QuantitativeProperty"
            ],
            "iudx:domainIncludes": [
                {
                    "@id": "iudx:WaterDistributionNetwork"
                }
            ],
            "iudx:rangeIncludes": [
                {
                    "@id": "iudx:Number"
                },
                {
                    "@id": "iudx:ValueDescriptor"
                }
            ],
            "rdfs:comment": "Length of the Cuboid shaped water storage tank.",
            "rdfs:isDefinedBy": {
                "@id": "https://voc.iudx.org.in/"
            },
            "rdfs:label": "tankLength"
        },
        {
            "@id": "https://voc.iudx.org.in/tankName",
            "@type": [
                "iudx:TextProperty"
            ],
            "iudx:domainIncludes": [
                {
                    "@id": "iudx:WaterDistributionNetwork"
                }
            ],
            "iudx:rangeIncludes": [
                {
                    "@id": "iudx:Text"
                },
                {
                    "@id": "iudx:ValueDescriptor"
                }
            ],
            "rdfs:comment": "Name of the water storage tank corresponding to this observation.",
            "rdfs:isDefinedBy": {
                "@id": "https://voc.iudx.org.in/"
            },
            "rdfs:label": "tankName"
        },
        {
            "@id": "https://voc.iudx.org.in/tankShape",
            "@type": [
                "iudx:TextProperty"
            ],
            "iudx:domainIncludes": [
                {
                    "@id": "iudx:WaterDistributionNetwork"
                }
            ],
            "iudx:rangeIncludes": [
                {
                    "@id": "iudx:Text"
                },
                {
                    "@id": "iudx:ValueDescriptor"
                }
            ],
            "rdfs:comment": "Physical shape of the water storage tank corresponding to this observation. ENUM: [Cylindrical, Conical, Cuboid, Spherical]",
            "rdfs:isDefinedBy": {
                "@id": "https://voc.iudx.org.in/"
            },
            "rdfs:label": "tankShape"
        },
        {
            "@id": "https://voc.iudx.org.in/title",
            "@type": [
                "iudx:TextProperty"
            ],
            "iudx:domainIncludes": [
                {
                    "@id": "iudx:IssueReporting"
                }
            ],
            "iudx:rangeIncludes": [
                {
                    "@id": "iudx:Text"
                },
                {
                    "@id": "iudx:ValueDescriptor"
                }
            ],
            "rdfs:comment": "The title assigned to the issue, report or feedback corresponding to this observation.",
            "rdfs:isDefinedBy": {
                "@id": "https://voc.iudx.org.in/"
            },
            "rdfs:label": "title",
            "skos:exactMatch": {
                "@id": "http://ontology.eil.utoronto.ca/open311.owl#description"
            }
        },
        {
            "@id": "https://voc.iudx.org.in/titleCode",
            "@type": [
                "iudx:TextProperty"
            ],
            "iudx:domainIncludes": [
                {
                    "@id": "iudx:IssueReporting"
                },
                {
                    "@id": "iudx:TrafficViolations"
                }
            ],
            "iudx:rangeIncludes": [
                {
                    "@id": "iudx:Text"
                },
                {
                    "@id": "iudx:ValueDescriptor"
                }
            ],
            "rdfs:comment": "The code assigned to the title corresponding to this observation.",
            "rdfs:isDefinedBy": {
                "@id": "https://voc.iudx.org.in/"
            },
            "rdfs:label": "titleCode"
        },
        {
            "@id": "https://voc.iudx.org.in/totalCount",
            "@type": [
                "iudx:QuantitativeProperty"
            ],
            "iudx:domainIncludes": [
                {
                    "@id": "iudx:RevenueCollection"
                }
            ],
            "iudx:rangeIncludes": [
                {
                    "@id": "iudx:Number"
                },
                {
                    "@id": "iudx:ValueDescriptor"
                }
            ],
            "rdfs:comment": "Count of the revenue collection service corresponding to this observation.",
            "rdfs:isDefinedBy": {
                "@id": "https://voc.iudx.org.in/"
            },
            "rdfs:label": "totalCount"
        },
        {
            "@id": "https://voc.iudx.org.in/totalML",
            "@type": [
                "iudx:QuantitativeProperty"
            ],
            "iudx:domainIncludes": [
                {
                    "@id": "iudx:WaterDistributionNetwork"
                }
            ],
            "iudx:rangeIncludes": [
                {
                    "@id": "iudx:Number"
                },
                {
                    "@id": "iudx:ValueDescriptor"
                }
            ],
            "rdfs:comment": "Total MLDs of water discharged from the water storage tank corresponding to this observation.",
            "rdfs:isDefinedBy": {
                "@id": "https://voc.iudx.org.in/"
            },
            "rdfs:label": "totalML"
        },
        {
            "@id": "https://voc.iudx.org.in/turbidity",
            "@type": [
                "iudx:QuantitativeProperty"
            ],
            "iudx:domainIncludes": [
                {
                    "@id": "iudx:WaterDistributionNetwork"
                }
            ],
            "iudx:rangeIncludes": [
                {
                    "@id": "iudx:TimeSeriesAggregation"
                },
                {
                    "@id": "iudx:ValueDescriptor"
                }
            ],
            "rdfs:comment": "Measurement of the amount of light that is scattered by material in the water when a light is shined through the water.",
            "rdfs:isDefinedBy": {
                "@id": "https://voc.iudx.org.in/"
            },
            "rdfs:label": "turbidity",
            "skos:exactMatch": {
                "@id": "https://uri.fiware.org/ns/data-models#WaterQualityObserved.turbidity"
            }
        },
        {
            "@id": "https://voc.iudx.org.in/ulbName",
            "@type": [
                "iudx:TextProperty"
            ],
            "iudx:domainIncludes": [
                {
                    "@id": "iudx:IssueReporting"
                }
            ],
            "iudx:rangeIncludes": [
                {
                    "@id": "iudx:Text"
                },
                {
                    "@id": "iudx:ValueDescriptor"
                }
            ],
            "rdfs:comment": "Name of the Urban Local Body from which the issue, report or feedback corresponding to this observation was raised or submitted.",
            "rdfs:isDefinedBy": {
                "@id": "https://voc.iudx.org.in/"
            },
            "rdfs:label": "ulbName"
        },
        {
            "@id": "https://voc.iudx.org.in/vehicleTypeCode",
            "@type": [
                "iudx:TextProperty"
            ],
            "iudx:domainIncludes": [
                {
                    "@id": "iudx:RevenueCollection"
                }
            ],
            "iudx:rangeIncludes": [
                {
                    "@id": "iudx:Text"
                },
                {
                    "@id": "iudx:ValueDescriptor"
                }
            ],
            "rdfs:comment": "The code for vehicleType corresponding to this observation. For eg.- '1' - MOPED/SCOOTER, '2' - MOTOR CYCLE, '4' - PRIVATE MOTOR CAR/JEEP CAR, '21' - TEMPO, '26' - BUS, etc.",
            "rdfs:isDefinedBy": {
                "@id": "https://voc.iudx.org.in/"
            },
            "rdfs:label": "vehicleTypeCode"
        },
        {
            "@id": "https://voc.iudx.org.in/waterFlow",
            "@type": [
                "iudx:QuantitativeProperty"
            ],
            "iudx:domainIncludes": [
                {
                    "@id": "iudx:WaterDistributionNetwork"
                }
            ],
            "iudx:rangeIncludes": [
                {
                    "@id": "iudx:Number"
                },
                {
                    "@id": "iudx:ValueDescriptor"
                }
            ],
            "rdfs:comment": "Flow or current of water flowing from the water storage tank corresponding to this observation.",
            "rdfs:isDefinedBy": {
                "@id": "https://voc.iudx.org.in/"
            },
            "rdfs:label": "waterFlow"
        },
        {
            "@id": "https://voc.iudx.org.in/waterLevel",
            "@type": [
                "iudx:QuantitativeProperty"
            ],
            "iudx:domainIncludes": [
                {
                    "@id": "iudx:WaterDistributionNetwork"
                }
            ],
            "iudx:rangeIncludes": [
                {
                    "@id": "iudx:Number"
                },
                {
                    "@id": "iudx:ValueDescriptor"
                }
            ],
            "rdfs:comment": "Current water level in the water storage tank corresponding to this observation.",
            "rdfs:isDefinedBy": {
                "@id": "https://voc.iudx.org.in/"
            },
            "rdfs:label": "waterLevel"
        },
        {
            "@id": "https://voc.iudx.org.in/waterPressure",
            "@type": [
                "iudx:QuantitativeProperty"
            ],
            "iudx:domainIncludes": [
                {
                    "@id": "iudx:WaterDistributionNetwork"
                }
            ],
            "iudx:rangeIncludes": [
                {
                    "@id": "iudx:Number"
                },
                {
                    "@id": "iudx:ValueDescriptor"
                }
            ],
            "rdfs:comment": "Pressure of water flowing from the water storage tank corresponding to this observation.",
            "rdfs:isDefinedBy": {
                "@id": "https://voc.iudx.org.in/"
            },
            "rdfs:label": "waterPressure"
        },
        {
            "@id": "https://voc.iudx.org.in/waterTemperature",
            "@type": [
                "iudx:QuantitativeProperty"
            ],
            "iudx:domainIncludes": [
                {
                    "@id": "iudx:WaterDistributionNetwork"
                }
            ],
            "iudx:rangeIncludes": [
                {
                    "@id": "iudx:Number"
                },
                {
                    "@id": "iudx:ValueDescriptor"
                }
            ],
            "rdfs:comment": "Water temperature in the water storage tank corresponding to this observation.",
            "rdfs:isDefinedBy": {
                "@id": "https://voc.iudx.org.in/"
            },
            "rdfs:label": "waterTemperature"
        },
        {
            "@id": "https://voc.iudx.org.in/comments",
            "@type": [
                "iudx:TextProperty"
            ],
            "iudx:domainIncludes": [
                {
                    "@id": "iudx:SafetiPin"
                },
                {
                    "@id": "iudx:IssueReporting"
                },
                {
                    "@id": "iudx:Version"
                },
                {
                    "@id": "iudx:Orientation"
                }
            ],
            "iudx:rangeIncludes": [
                {
                    "@container": "@list",
                    "@id": "iudx:Text"
                },
                {
                    "@id": "iudx:Text"
                },
                {
                    "@id": "iudx:ValueDescriptor"
                }
            ],
            "rdfs:comment": "User comments corresponding to this observation.",
            "rdfs:isDefinedBy": {
                "@id": "https://voc.iudx.org.in/"
            },
            "rdfs:label": "comments"
        },
        {
            "@id": "https://voc.iudx.org.in/deviceInfo",
            "@type": [
                "iudx:StructuredProperty"
            ],
            "iudx:domainIncludes": [
                {
                    "@id": "iudx:EnvAQM"
                },
                {
                    "@id": "iudx:EnvFlood"
                },
                {
                    "@id": "iudx:TransitManagement"
                },
                {
                    "@id": "iudx:WiFiHostspot"
                },
                {
                    "@id": "iudx:StreetLightFeeder"
                },
                {
                    "@id": "iudx:Streetlight"
                },
                {
                    "@id": "iudx:WaterDistributionNetwork"
                }
            ],
            "iudx:rangeIncludes": [
                {
                    "@id": "iudx:Device"
                }
            ],
            "rdfs:comment": "Information about the device associated with the observations.",
            "rdfs:isDefinedBy": {
                "@id": "https://voc.iudx.org.in/"
            },
            "rdfs:label": "deviceInfo"
        },
        {
            "@id": "https://voc.iudx.org.in/deviceStatus",
            "@type": [
                "iudx:TextProperty"
            ],
            "iudx:domainIncludes": [
                {
                    "@id": "iudx:EnvAQM"
                },
                {
                    "@id": "iudx:EnvFlood"
                },
                {
                    "@id": "iudx:WiFiHostspot"
                }
            ],
            "iudx:rangeIncludes": [
                {
                    "@id": "iudx:Text"
                },
                {
                    "@id": "iudx:ValueDescriptor"
                }
            ],
            "rdfs:comment": "Indicates the status of physical device or devices.",
            "rdfs:isDefinedBy": {
                "@id": "https://voc.iudx.org.in/"
            },
            "rdfs:label": "deviceStatus"
        },
        {
            "@id": "https://voc.iudx.org.in/municipalityInfo",
            "@type": [
                "iudx:StructuredProperty"
            ],
            "iudx:domainIncludes": [
                {
                    "@id": "iudx:RevenueCollection"
                },
                {
                    "@id": "iudx:EmployeeDetails"
                },
                {
                    "@id": "iudx:Streetlight"
                },
                {
                    "@id": "iudx:WasteWaterMgmt"
                }
            ],
            "iudx:rangeIncludes": [
                {
                    "@id": "iudx:MunicipalityDesc"
                }
            ],
            "rdfs:comment": "Municipality information corresponding to this observation.",
            "rdfs:isDefinedBy": {
                "@id": "https://voc.iudx.org.in/"
            },
            "rdfs:label": "municipalityInfo"
        },
        {
            "@id": "https://voc.iudx.org.in/observationDateTime",
            "@type": [
                "iudx:TimeProperty"
            ],
            "iudx:domainIncludes": [
                {
                    "@id": "iudx:EnvAQM"
                },
                {
                    "@id": "iudx:EnvFlood"
                },
                {
                    "@id": "iudx:EnvWeather"
                },
                {
                    "@id": "iudx:TransitManagement"
                },
                {
                    "@id": "iudx:WiFiHostspot"
                },
                {
                    "@id": "iudx:StreetLightFeeder"
                },
                {
                    "@id": "iudx:WmgmtVehicle"
                },
                {
                    "@id": "iudx:SafetiPin"
                },
                {
                    "@id": "iudx:IssueReporting"
                },
                {
                    "@id": "iudx:FareCollectionSystem"
                },
                {
                    "@id": "iudx:EmployeeDetails"
                },
                {
                    "@id": "iudx:TrafficViolations"
                },
                {
                    "@id": "iudx:Streetlight"
                },
                {
                    "@id": "iudx:BikeDockingStation"
                },
                {
                    "@id": "iudx:WaterDistributionNetwork"
                },
                {
                    "@id": "iudx:WasteWaterMgmt"
                }
            ],
            "iudx:rangeIncludes": [
                {
                    "@id": "iudx:DateTime"
                },
                {
                    "@id": "iudx:ValueDescriptor"
                }
            ],
            "rdfs:comment": "Last reported time of observation.",
            "rdfs:isDefinedBy": {
                "@id": "https://voc.iudx.org.in/"
            },
            "rdfs:label": "observationDateTime"
        },
        {
            "@id": "https://voc.iudx.org.in/deviceBatteryStatus",
            "@type": [
                "iudx:TextProperty"
            ],
            "iudx:domainIncludes": [
                {
                    "@id": "iudx:Device"
                },
                {
                    "@id": "iudx:WmgmtVehicle"
                }
            ],
            "iudx:rangeIncludes": [
                {
                    "@id": "iudx:Text"
                },
                {
                    "@id": "iudx:ValueDescriptor"
                }
            ],
            "rdfs:comment": "Gives the Battery charging status of the reporting device(Connected, Disconnected).",
            "rdfs:isDefinedBy": {
                "@id": "https://voc.iudx.org.in/"
            },
            "rdfs:label": "deviceBatteryStatus"
        },
        {
            "@id": "https://voc.iudx.org.in/deviceID",
            "@type": [
                "iudx:TextProperty"
            ],
            "iudx:domainIncludes": [
                {
                    "@id": "iudx:Device"
                }
            ],
            "iudx:rangeIncludes": [
                {
                    "@id": "iudx:Text"
                },
                {
                    "@id": "iudx:ValueDescriptor"
                }
            ],
            "rdfs:comment": "Device ID of the physical sensor/ measurement station corresponding to this observation.",
            "rdfs:isDefinedBy": {
                "@id": "https://voc.iudx.org.in/"
            },
            "rdfs:label": "deviceID"
        },
        {
            "@id": "https://voc.iudx.org.in/deviceList",
            "@type": [
                "iudx:TextProperty"
            ],
            "iudx:domainIncludes": [
                {
                    "@id": "iudx:Device"
                }
            ],
            "iudx:rangeIncludes": [
                {
                    "@container": "@list",
                    "@id": "iudx:Text"
                }
            ],
            "rdfs:comment": "Information of device part number and sub devices corresponding to this observation.",
            "rdfs:isDefinedBy": {
                "@id": "https://voc.iudx.org.in/"
            },
            "rdfs:label": "deviceList"
        },
        {
            "@id": "https://voc.iudx.org.in/deviceModel",
            "@type": [
                "iudx:StructuredProperty"
            ],
            "iudx:domainIncludes": [
                {
                    "@id": "iudx:Device"
                }
            ],
            "iudx:rangeIncludes": [
                {
                    "@id": "iudx:ModelInfo"
                }
            ],
            "rdfs:comment": "Describes the information of the device, sensor or system in consideration.",
            "rdfs:isDefinedBy": {
                "@id": "https://voc.iudx.org.in/"
            },
            "rdfs:label": "deviceModel"
        },
        {
            "@id": "https://voc.iudx.org.in/deviceName",
            "@type": [
                "iudx:TextProperty"
            ],
            "iudx:domainIncludes": [
                {
                    "@id": "iudx:Device"
                }
            ],
            "iudx:rangeIncludes": [
                {
                    "@id": "iudx:Text"
                },
                {
                    "@id": "iudx:ValueDescriptor"
                }
            ],
            "rdfs:comment": "Device Name or Station name of the sensor device/station corresponding to this observation.",
            "rdfs:isDefinedBy": {
                "@id": "https://voc.iudx.org.in/"
            },
            "rdfs:label": "deviceName"
        },
        {
            "@id": "https://voc.iudx.org.in/deviceSimNumber",
            "@type": [
                "iudx:TextProperty"
            ],
            "iudx:domainIncludes": [
                {
                    "@id": "iudx:Device"
                },
                {
                    "@id": "iudx:WmgmtVehicle"
                }
            ],
            "iudx:rangeIncludes": [
                {
                    "@id": "iudx:Text"
                },
                {
                    "@id": "iudx:ValueDescriptor"
                }
            ],
            "rdfs:comment": "Gives the sim number of the device in the waste management vehicle.",
            "rdfs:isDefinedBy": {
                "@id": "https://voc.iudx.org.in/"
            },
            "rdfs:label": "deviceSimNumber"
        },
        {
            "@id": "https://voc.iudx.org.in/measurand",
            "@type": [
                "iudx:TextProperty"
            ],
            "iudx:domainIncludes": [
                {
                    "@id": "iudx:Device"
                }
            ],
            "iudx:rangeIncludes": [
                {
                    "@id": "iudx:Text"
                }
            ],
            "rdfs:comment": "Property/properties sensed/observed/measured by the device.",
            "rdfs:isDefinedBy": {
                "@id": "https://voc.iudx.org.in/"
            },
            "rdfs:label": "measurand"
        },
        {
            "@id": "https://voc.iudx.org.in/RFID",
            "@type": [
                "iudx:TextProperty"
            ],
            "iudx:domainIncludes": [
                {
                    "@id": "iudx:Device"
                },
                {
                    "@id": "iudx:WmgmtBin"
                }
            ],
            "iudx:rangeIncludes": [
                {
                    "@id": "iudx:Text"
                },
                {
                    "@id": "iudx:ValueDescriptor"
                }
            ],
            "rdfs:comment": "Gives the ID of the RFID reader.",
            "rdfs:isDefinedBy": {
                "@id": "https://voc.iudx.org.in/"
            },
            "rdfs:label": "RFID"
        },
        {
            "@id": "https://voc.iudx.org.in/airQualityIndex",
            "@type": [
                "iudx:QuantitativeProperty"
            ],
            "iudx:domainIncludes": [
                {
                    "@id": "iudx:EnvWeather"
                },
                {
                    "@id": "iudx:EnvAQM"
                }
            ],
            "iudx:rangeIncludes": [
                {
                    "@id": "iudx:Number"
                },
                {
                    "@id": "iudx:ValueDescriptor"
                }
            ],
            "rdfs:comment": "Overall Air Quality Index (AQI) for the observed air quality.",
            "rdfs:isDefinedBy": {
                "@id": "https://voc.iudx.org.in/"
            },
            "rdfs:label": "airQualityIndex"
        },
        {
            "@id": "https://voc.iudx.org.in/airQualityIndexForecast",
            "@type": [
                "iudx:QuantitativeProperty"
            ],
            "iudx:domainIncludes": [
                {
                    "@id": "iudx:EnvWeather"
                }
            ],
            "iudx:rangeIncludes": [
                {
                    "@id": "iudx:Number"
                },
                {
                    "@id": "iudx:ValueDescriptor"
                }
            ],
            "rdfs:comment": "Forecasted overall Air Quality Index (AQI) over a certain duration in future.",
            "rdfs:isDefinedBy": {
                "@id": "https://voc.iudx.org.in/"
            },
            "rdfs:label": "airQualityIndexForecast"
        },
        {
            "@id": "https://voc.iudx.org.in/airQualityLevel",
            "@type": [
                "iudx:TextProperty"
            ],
            "iudx:domainIncludes": [
                {
                    "@id": "iudx:EnvAQM"
                }
            ],
            "iudx:rangeIncludes": [
                {
                    "@id": "iudx:Text"
                },
                {
                    "@id": "iudx:ValueDescriptor"
                }
            ],
            "rdfs:comment": "Air Quality Category Indication. Qualitative level defined according to the local health agencies. For example, 'GOOD', 'MODERATE', 'POOR', 'UNHEALTHY', 'SEVERE', 'HAZARDOUS' etc.",
            "rdfs:isDefinedBy": {
                "@id": "https://voc.iudx.org.in/"
            },
            "rdfs:label": "airQualityLevel",
            "skos:exactMatch": {
                "@id": "https://uri.fiware.org/ns/data-models#airQualityLevel"
            }
        },
        {
            "@id": "https://voc.iudx.org.in/airTemperature",
            "@type": [
                "iudx:QuantitativeProperty"
            ],
            "iudx:domainIncludes": [
                {
                    "@id": "iudx:EnvWeather"
                },
                {
                    "@id": "iudx:EnvAQM"
                }
            ],
            "iudx:rangeIncludes": [
                {
                    "@id": "iudx:TimeSeriesAggregation"
                }
            ],
            "rdfs:comment": "Observed value of air temperature. Value is an object containing attributes representing statistical aggregates derived from past data.",
            "rdfs:isDefinedBy": {
                "@id": "https://voc.iudx.org.in/"
            },
            "rdfs:label": "airTemperature",
            "skos:exactMatch": {
                "@id": "https://uri.fiware.org/ns/data-models#temperature"
            }
        },
        {
            "@id": "https://voc.iudx.org.in/airTemperatureForecast",
            "@type": [
                "iudx:QuantitativeProperty"
            ],
            "iudx:domainIncludes": [
                {
                    "@id": "iudx:EnvWeather"
                }
            ],
            "iudx:rangeIncludes": [
                {
                    "@id": "iudx:Number"
                },
                {
                    "@id": "iudx:ValueDescriptor"
                }
            ],
            "rdfs:comment": "Forecasted value of air temperature over a certain duration in future.",
            "rdfs:isDefinedBy": {
                "@id": "https://voc.iudx.org.in/"
            },
            "rdfs:label": "airTemperatureForecast"
        },
        {
            "@id": "https://voc.iudx.org.in/alertLevel",
            "@type": [
                "iudx:QuantitativeProperty"
            ],
            "iudx:domainIncludes": [
                {
                    "@id": "iudx:EnvFlood"
                }
            ],
            "iudx:rangeIncludes": [
                {
                    "@id": "iudx:Number"
                },
                {
                    "@id": "iudx:ValueDescriptor"
                }
            ],
            "rdfs:comment": "Reference alert level threshold value set for the sensing station corresponding to this observation. An Alert signal is generated if the current level crosses the alert level threshold value.",
            "rdfs:isDefinedBy": {
                "@id": "https://voc.iudx.org.in/"
            },
            "rdfs:label": "alertLevel"
        },
        {
            "@id": "https://voc.iudx.org.in/ambientNoise",
            "@type": [
                "iudx:QuantitativeProperty"
            ],
            "iudx:domainIncludes": [
                {
                    "@id": "iudx:EnvAQM"
                }
            ],
            "iudx:rangeIncludes": [
                {
                    "@id": "iudx:TimeSeriesAggregation"
                }
            ],
            "rdfs:comment": "Observed value of ambient noise levels. Value is an object containing attributes representing statistical aggregates derived from past data.",
            "rdfs:isDefinedBy": {
                "@id": "https://voc.iudx.org.in/"
            },
            "rdfs:label": "ambientNoise"
        },
        {
            "@id": "https://voc.iudx.org.in/aqiMajorPollutant",
            "@type": [
                "iudx:TextProperty"
            ],
            "iudx:domainIncludes": [
                {
                    "@id": "iudx:EnvWeather"
                },
                {
                    "@id": "iudx:EnvAQM"
                }
            ],
            "iudx:rangeIncludes": [
                {
                    "@id": "iudx:Text"
                },
                {
                    "@id": "iudx:ValueDescriptor"
                }
            ],
            "rdfs:comment": "Major pollutant in the Air Quality Index (AQI).",
            "rdfs:isDefinedBy": {
                "@id": "https://voc.iudx.org.in/"
            },
            "rdfs:label": "aqiMajorPollutant"
        },
        {
            "@id": "https://voc.iudx.org.in/aqiMajorPollutantForecast",
            "@type": [
                "iudx:TextProperty"
            ],
            "iudx:domainIncludes": [
                {
                    "@id": "iudx:EnvWeather"
                }
            ],
            "iudx:rangeIncludes": [
                {
                    "@id": "iudx:Text"
                },
                {
                    "@id": "iudx:ValueDescriptor"
                }
            ],
            "rdfs:comment": "Forecasted major air pollutant in the Air Quality Index (AQI) over a certain duration in future.",
            "rdfs:isDefinedBy": {
                "@id": "https://voc.iudx.org.in/"
            },
            "rdfs:label": "aqiMajorPollutantForecast"
        },
        {
            "@id": "https://voc.iudx.org.in/arsenic",
            "@type": [
                "iudx:QuantitativeProperty"
            ],
            "iudx:domainIncludes": [
                {
                    "@id": "iudx:EnvAQM"
                }
            ],
            "iudx:rangeIncludes": [
                {
                    "@id": "iudx:TimeSeriesAggregation"
                }
            ],
            "rdfs:comment": "Observed value of environmental pollutant Arsenic (As). Value is an object containing attributes representing statistical aggregates derived from past data.",
            "rdfs:isDefinedBy": {
                "@id": "https://voc.iudx.org.in/"
            },
            "rdfs:label": "arsenic"
        },
        {
            "@id": "https://voc.iudx.org.in/atmosphericPressure",
            "@type": [
                "iudx:QuantitativeProperty"
            ],
            "iudx:domainIncludes": [
                {
                    "@id": "iudx:EnvWeather"
                },
                {
                    "@id": "iudx:EnvAQM"
                }
            ],
            "iudx:rangeIncludes": [
                {
                    "@id": "iudx:Number"
                },
                {
                    "@id": "iudx:ValueDescriptor"
                }
            ],
            "rdfs:comment": "Observed air (atmospheric or barometric) pressure.",
            "rdfs:isDefinedBy": {
                "@id": "https://voc.iudx.org.in/"
            },
            "rdfs:label": "atmosphericPressure",
            "skos:exactMatch": {
                "@id": "https://uri.fiware.org/ns/data-models#atmosphericPressure"
            }
        },
        {
            "@id": "https://voc.iudx.org.in/bap",
            "@type": [
                "iudx:QuantitativeProperty"
            ],
            "iudx:domainIncludes": [
                {
                    "@id": "iudx:EnvAQM"
                }
            ],
            "iudx:rangeIncludes": [
                {
                    "@id": "iudx:TimeSeriesAggregation"
                }
            ],
            "rdfs:comment": "Observed value of environmental pollutant Benzo[a]pyrene (BaP). Value is an object containing attributes representing statistical aggregates derived from past data.",
            "rdfs:isDefinedBy": {
                "@id": "https://voc.iudx.org.in/"
            },
            "rdfs:label": "bap"
        },
        {
            "@id": "https://voc.iudx.org.in/benzene",
            "@type": [
                "iudx:QuantitativeProperty"
            ],
            "iudx:domainIncludes": [
                {
                    "@id": "iudx:EnvAQM"
                }
            ],
            "iudx:rangeIncludes": [
                {
                    "@id": "iudx:TimeSeriesAggregation"
                }
            ],
            "rdfs:comment": "Observed value of environmental pollutant Benzene (C6H6). Value is an object containing attributes representing statistical aggregates derived from past data.",
            "rdfs:isDefinedBy": {
                "@id": "https://voc.iudx.org.in/"
            },
            "rdfs:label": "benzene"
        },
        {
            "@id": "https://voc.iudx.org.in/co",
            "@type": [
                "iudx:QuantitativeProperty"
            ],
            "iudx:domainIncludes": [
                {
                    "@id": "iudx:EnvAQM"
                }
            ],
            "iudx:rangeIncludes": [
                {
                    "@id": "iudx:TimeSeriesAggregation"
                }
            ],
            "rdfs:comment": "Observed value of environmental pollutant Carbon Monoxide (CO). Value is an object containing attributes representing statistical aggregates derived from past data.",
            "rdfs:isDefinedBy": {
                "@id": "https://voc.iudx.org.in/"
            },
            "rdfs:label": "co"
        },
        {
            "@id": "https://voc.iudx.org.in/co2",
            "@type": [
                "iudx:QuantitativeProperty"
            ],
            "iudx:domainIncludes": [
                {
                    "@id": "iudx:EnvAQM"
                }
            ],
            "iudx:rangeIncludes": [
                {
                    "@id": "iudx:TimeSeriesAggregation"
                }
            ],
            "rdfs:comment": "Observed value of environmental pollutant Carbon Dioxide (CO2). Value is an object containing attributes representing statistical aggregates derived from past data.",
            "rdfs:isDefinedBy": {
                "@id": "https://voc.iudx.org.in/"
            },
            "rdfs:label": "co2"
        },
        {
            "@id": "https://voc.iudx.org.in/currentLevel",
            "@type": [
                "iudx:QuantitativeProperty"
            ],
            "iudx:domainIncludes": [
                {
                    "@id": "iudx:EnvFlood"
                }
            ],
            "iudx:rangeIncludes": [
                {
                    "@id": "iudx:Number"
                },
                {
                    "@id": "iudx:ValueDescriptor"
                }
            ],
            "rdfs:comment": "Current flooding level indicated by the sensing station corresponding to this observation.",
            "rdfs:isDefinedBy": {
                "@id": "https://voc.iudx.org.in/"
            },
            "rdfs:label": "currentLevel"
        },
        {
            "@id": "https://voc.iudx.org.in/dangerLevel",
            "@type": [
                "iudx:QuantitativeProperty"
            ],
            "iudx:domainIncludes": [
                {
                    "@id": "iudx:EnvFlood"
                }
            ],
            "iudx:rangeIncludes": [
                {
                    "@id": "iudx:Number"
                },
                {
                    "@id": "iudx:ValueDescriptor"
                }
            ],
            "rdfs:comment": "Reference danger level threshold value set for the sensing station corresponding to this observation. Flood level status is marked danger if the current level crosses the danger level threshold value.",
            "rdfs:isDefinedBy": {
                "@id": "https://voc.iudx.org.in/"
            },
            "rdfs:label": "dangerLevel"
        },
        {
            "@id": "https://voc.iudx.org.in/dewPoint",
            "@type": [
                "iudx:QuantitativeProperty"
            ],
            "iudx:domainIncludes": [
                {
                    "@id": "iudx:EnvWeather"
                }
            ],
            "iudx:rangeIncludes": [
                {
                    "@id": "iudx:Number"
                },
                {
                    "@id": "iudx:ValueDescriptor"
                }
            ],
            "rdfs:comment": "Observed  temperature to which air must be cooled to become saturated with water vapor.",
            "rdfs:isDefinedBy": {
                "@id": "https://voc.iudx.org.in/"
            },
            "rdfs:label": "dewPoint",
            "skos:exactMatch": {
                "@id": "https://uri.fiware.org/ns/data-models#dewPoint"
            }
        },
        {
            "@id": "https://voc.iudx.org.in/floodLevelStatus",
            "@type": [
                "iudx:TextProperty"
            ],
            "iudx:domainIncludes": [
                {
                    "@id": "iudx:EnvFlood"
                }
            ],
            "iudx:rangeIncludes": [
                {
                    "@id": "iudx:Text"
                },
                {
                    "@id": "iudx:ValueDescriptor"
                }
            ],
            "rdfs:comment": "Flood level status indication given by the flood sensing device. The status is marked Danger if the current level is higher than the danger level threshold value.",
            "rdfs:isDefinedBy": {
                "@id": "https://voc.iudx.org.in/"
            },
            "rdfs:label": "floodLevelStatus"
        },
        {
            "@id": "https://voc.iudx.org.in/gustSpeed",
            "@type": [
                "iudx:QuantitativeProperty"
            ],
            "iudx:domainIncludes": [
                {
                    "@id": "iudx:EnvWeather"
                }
            ],
            "iudx:rangeIncludes": [
                {
                    "@id": "iudx:Number"
                },
                {
                    "@id": "iudx:ValueDescriptor"
                }
            ],
            "rdfs:comment": "A sudden burst of high-speed wind over the observed average wind speed lasting  only for a few seconds.",
            "rdfs:isDefinedBy": {
                "@id": "https://voc.iudx.org.in/"
            },
            "rdfs:label": "gustSpeed"
        },
        {
            "@id": "https://voc.iudx.org.in/illuminance",
            "@type": [
                "iudx:QuantitativeProperty"
            ],
            "iudx:domainIncludes": [
                {
                    "@id": "iudx:EnvWeather"
                },
                {
                    "@id": "iudx:EnvAQM"
                }
            ],
            "iudx:rangeIncludes": [
                {
                    "@id": "iudx:Number"
                },
                {
                    "@id": "iudx:ValueDescriptor"
                }
            ],
            "rdfs:comment": "Observed instantaneous ambient light intensity.",
            "rdfs:isDefinedBy": {
                "@id": "https://voc.iudx.org.in/"
            },
            "rdfs:label": "illuminance",
            "skos:exactMatch": {
                "@id": "https://uri.fiware.org/ns/data-models#illuminance"
            }
        },
        {
            "@id": "https://voc.iudx.org.in/measuredDistance",
            "@type": [
                "iudx:QuantitativeProperty"
            ],
            "iudx:domainIncludes": [
                {
                    "@id": "iudx:EnvFlood"
                }
            ],
            "iudx:rangeIncludes": [
                {
                    "@id": "iudx:Number"
                },
                {
                    "@id": "iudx:ValueDescriptor"
                }
            ],
            "rdfs:comment": "Describes the distance measured by the sensor, from the sensor tip to the upper surface of water.",
            "rdfs:isDefinedBy": {
                "@id": "https://voc.iudx.org.in/"
            },
            "rdfs:label": "measuredDistance"
        },
        {
            "@id": "https://voc.iudx.org.in/nh3",
            "@type": [
                "iudx:QuantitativeProperty"
            ],
            "iudx:domainIncludes": [
                {
                    "@id": "iudx:EnvAQM"
                }
            ],
            "iudx:rangeIncludes": [
                {
                    "@id": "iudx:TimeSeriesAggregation"
                }
            ],
            "rdfs:comment": "Observed value of environmental pollutant Ammonia (NH3). Value is an object containing attributes representing statistical aggregates derived from past data.",
            "rdfs:isDefinedBy": {
                "@id": "https://voc.iudx.org.in/"
            },
            "rdfs:label": "nh3"
        },
        {
            "@id": "https://voc.iudx.org.in/nickel",
            "@type": [
                "iudx:QuantitativeProperty"
            ],
            "iudx:domainIncludes": [
                {
                    "@id": "iudx:EnvAQM"
                }
            ],
            "iudx:rangeIncludes": [
                {
                    "@id": "iudx:TimeSeriesAggregation"
                }
            ],
            "rdfs:comment": "Observed value of environmental pollutant Nickel (Ni). Value is an object containing attributes representing statistical aggregates derived from past data.",
            "rdfs:isDefinedBy": {
                "@id": "https://voc.iudx.org.in/"
            },
            "rdfs:label": "nickel"
        },
        {
            "@id": "https://voc.iudx.org.in/no",
            "@type": [
                "iudx:QuantitativeProperty"
            ],
            "iudx:domainIncludes": [
                {
                    "@id": "iudx:EnvAQM"
                }
            ],
            "iudx:rangeIncludes": [
                {
                    "@id": "iudx:TimeSeriesAggregation"
                }
            ],
            "rdfs:comment": "Observed value of environmental pollutant Nitrogen Monoxide (NO). Value is an object containing attributes representing statistical aggregates derived from past data.",
            "rdfs:isDefinedBy": {
                "@id": "https://voc.iudx.org.in/"
            },
            "rdfs:label": "no"
        },
        {
            "@id": "https://voc.iudx.org.in/no2",
            "@type": [
                "iudx:QuantitativeProperty"
            ],
            "iudx:domainIncludes": [
                {
                    "@id": "iudx:EnvAQM"
                }
            ],
            "iudx:rangeIncludes": [
                {
                    "@id": "iudx:TimeSeriesAggregation"
                }
            ],
            "rdfs:comment": "Observed value of environmental pollutant Nitrogen Dioxide (NO2). Value is an object containing attributes representing statistical aggregates derived from past data.",
            "rdfs:isDefinedBy": {
                "@id": "https://voc.iudx.org.in/"
            },
            "rdfs:label": "no2"
        },
        {
            "@id": "https://voc.iudx.org.in/o2",
            "@type": [
                "iudx:QuantitativeProperty"
            ],
            "iudx:domainIncludes": [
                {
                    "@id": "iudx:EnvAQM"
                }
            ],
            "iudx:rangeIncludes": [
                {
                    "@id": "iudx:TimeSeriesAggregation"
                }
            ],
            "rdfs:comment": "Observed value of Oxygen (O2). Value is an object containing attributes representing statistical aggregates derived from past data.",
            "rdfs:isDefinedBy": {
                "@id": "https://voc.iudx.org.in/"
            },
            "rdfs:label": "o2"
        },
        {
            "@id": "https://voc.iudx.org.in/o3",
            "@type": [
                "iudx:QuantitativeProperty"
            ],
            "iudx:domainIncludes": [
                {
                    "@id": "iudx:EnvAQM"
                }
            ],
            "iudx:rangeIncludes": [
                {
                    "@id": "iudx:TimeSeriesAggregation"
                }
            ],
            "rdfs:comment": "Observed value of environmental pollutant Ozone (O3). Value is an object containing attributes representing statistical aggregates derived from past data.",
            "rdfs:isDefinedBy": {
                "@id": "https://voc.iudx.org.in/"
            },
            "rdfs:label": "o3"
        },
        {
            "@id": "https://voc.iudx.org.in/pb",
            "@type": [
                "iudx:QuantitativeProperty"
            ],
            "iudx:domainIncludes": [
                {
                    "@id": "iudx:EnvAQM"
                }
            ],
            "iudx:rangeIncludes": [
                {
                    "@id": "iudx:TimeSeriesAggregation"
                }
            ],
            "rdfs:comment": "Observed value of environmental pollutant Lead (Pb). Value is an object containing attributes representing statistical aggregates derived from past data.",
            "rdfs:isDefinedBy": {
                "@id": "https://voc.iudx.org.in/"
            },
            "rdfs:label": "pb"
        },
        {
            "@id": "https://voc.iudx.org.in/pm10",
            "@type": [
                "iudx:QuantitativeProperty"
            ],
            "iudx:domainIncludes": [
                {
                    "@id": "iudx:EnvAQM"
                }
            ],
            "iudx:rangeIncludes": [
                {
                    "@id": "iudx:TimeSeriesAggregation"
                }
            ],
            "rdfs:comment": "Observed value of environmental pollutant  Particulate Matter 10 (PM10). Value is an object containing attributes representing statistical aggregates derived from past data.",
            "rdfs:isDefinedBy": {
                "@id": "https://voc.iudx.org.in/"
            },
            "rdfs:label": "pm10"
        },
        {
            "@id": "https://voc.iudx.org.in/pm2p5",
            "@type": [
                "iudx:QuantitativeProperty"
            ],
            "iudx:domainIncludes": [
                {
                    "@id": "iudx:EnvAQM"
                }
            ],
            "iudx:rangeIncludes": [
                {
                    "@id": "iudx:TimeSeriesAggregation"
                }
            ],
            "rdfs:comment": "Observed value of environmental pollutant Particulate Matter 2.5 (PM2.5). Value is an object containing attributes representing statistical aggregates derived from past data.",
            "rdfs:isDefinedBy": {
                "@id": "https://voc.iudx.org.in/"
            },
            "rdfs:label": "pm2p5"
        },
        {
            "@id": "https://voc.iudx.org.in/precipitation",
            "@type": [
                "iudx:QuantitativeProperty"
            ],
            "iudx:domainIncludes": [
                {
                    "@id": "iudx:EnvWeather"
                },
                {
                    "@id": "iudx:EnvAQM"
                }
            ],
            "iudx:rangeIncludes": [
                {
                    "@id": "iudx:Number"
                },
                {
                    "@id": "iudx:ValueDescriptor"
                }
            ],
            "rdfs:comment": "Observed precipitation/rainfall level over a given duration.",
            "rdfs:isDefinedBy": {
                "@id": "https://voc.iudx.org.in/"
            },
            "rdfs:label": "precipitation",
            "skos:exactMatch": {
                "@id": "https://uri.fiware.org/ns/data-models#precipitation"
            }
        },
        {
            "@id": "https://voc.iudx.org.in/precipitationForecast",
            "@type": [
                "iudx:QuantitativeProperty"
            ],
            "iudx:domainIncludes": [
                {
                    "@id": "iudx:EnvWeather"
                }
            ],
            "iudx:rangeIncludes": [
                {
                    "@id": "iudx:Number"
                },
                {
                    "@id": "iudx:ValueDescriptor"
                }
            ],
            "rdfs:comment": "Forecasted rainfall over a certain duration in future.",
            "rdfs:isDefinedBy": {
                "@id": "https://voc.iudx.org.in/"
            },
            "rdfs:label": "precipitationForecast"
        },
        {
            "@id": "https://voc.iudx.org.in/referenceLevel",
            "@type": [
                "iudx:QuantitativeProperty"
            ],
            "iudx:domainIncludes": [
                {
                    "@id": "iudx:EnvFlood"
                }
            ],
            "iudx:rangeIncludes": [
                {
                    "@id": "iudx:Number"
                },
                {
                    "@id": "iudx:ValueDescriptor"
                }
            ],
            "rdfs:comment": "Reference setting used to compute the currentLevel.",
            "rdfs:isDefinedBy": {
                "@id": "https://voc.iudx.org.in/"
            },
            "rdfs:label": "referenceLevel"
        },
        {
            "@id": "https://voc.iudx.org.in/relativeHumidity",
            "@type": [
                "iudx:QuantitativeProperty"
            ],
            "iudx:domainIncludes": [
                {
                    "@id": "iudx:EnvWeather"
                },
                {
                    "@id": "iudx:EnvAQM"
                }
            ],
            "iudx:rangeIncludes": [
                {
                    "@id": "iudx:TimeSeriesAggregation"
                }
            ],
            "rdfs:comment": "Observed instantaneous relative humidity (water vapour in air).",
            "rdfs:isDefinedBy": {
                "@id": "https://voc.iudx.org.in/"
            },
            "rdfs:label": "relativeHumidity",
            "skos:exactMatch": {
                "@id": "https://uri.fiware.org/ns/data-models#relativeHumidity"
            }
        },
        {
            "@id": "https://voc.iudx.org.in/relativeHumidityForecast",
            "@type": [
                "iudx:QuantitativeProperty"
            ],
            "iudx:domainIncludes": [
                {
                    "@id": "iudx:EnvWeather"
                }
            ],
            "iudx:rangeIncludes": [
                {
                    "@id": "iudx:Number"
                },
                {
                    "@id": "iudx:ValueDescriptor"
                }
            ],
            "rdfs:comment": "Forecasted relative humidity (water vapour in air) over a certain duration in future.",
            "rdfs:isDefinedBy": {
                "@id": "https://voc.iudx.org.in/"
            },
            "rdfs:label": "relativeHumidityForecast"
        },
        {
            "@id": "https://voc.iudx.org.in/so2",
            "@type": [
                "iudx:QuantitativeProperty"
            ],
            "iudx:domainIncludes": [
                {
                    "@id": "iudx:EnvAQM"
                }
            ],
            "iudx:rangeIncludes": [
                {
                    "@id": "iudx:TimeSeriesAggregation"
                }
            ],
            "rdfs:comment": "Observed value of environmental pollutant Sulphur Dioxide (SO2). Value is an object containing attributes representing statistical aggregates derived from past data.",
            "rdfs:isDefinedBy": {
                "@id": "https://voc.iudx.org.in/"
            },
            "rdfs:label": "so2"
        },
        {
            "@id": "https://voc.iudx.org.in/solarRadiation",
            "@type": [
                "iudx:QuantitativeProperty"
            ],
            "iudx:domainIncludes": [
                {
                    "@id": "iudx:EnvWeather"
                },
                {
                    "@id": "iudx:EnvAQM"
                }
            ],
            "iudx:rangeIncludes": [
                {
                    "@id": "iudx:Number"
                },
                {
                    "@id": "iudx:ValueDescriptor"
                }
            ],
            "rdfs:comment": "Observed solar radiation.",
            "rdfs:isDefinedBy": {
                "@id": "https://voc.iudx.org.in/"
            },
            "rdfs:label": "solarRadiation",
            "skos:exactMatch": {
                "@id": "https://uri.fiware.org/ns/data-models#solarRadiation"
            }
        },
        {
            "@id": "https://voc.iudx.org.in/uv",
            "@type": [
                "iudx:QuantitativeProperty"
            ],
            "iudx:domainIncludes": [
                {
                    "@id": "iudx:EnvWeather"
                },
                {
                    "@id": "iudx:EnvAQM"
                }
            ],
            "iudx:rangeIncludes": [
                {
                    "@id": "iudx:TimeSeriesAggregation"
                }
            ],
            "rdfs:comment": "Observed levels of UV radiation. Value is an object containing attributes representing statistical aggregates derived from past data.",
            "rdfs:isDefinedBy": {
                "@id": "https://voc.iudx.org.in/"
            },
            "rdfs:label": "uv"
        },
        {
            "@id": "https://voc.iudx.org.in/versionInfo",
            "@type": [
                "iudx:StructuredProperty"
            ],
            "iudx:domainIncludes": [
                {
                    "@id": "iudx:EnvAQM"
                }
            ],
            "iudx:rangeIncludes": [
                {
                    "@id": "iudx:Version"
                },
                {
                    "@container": "@list",
                    "@id": "iudx:Version"
                }
            ],
            "rdfs:comment": "Version information corresponding to this observation.",
            "rdfs:isDefinedBy": {
                "@id": "https://voc.iudx.org.in/"
            },
            "rdfs:label": "versionInfo"
        },
        {
            "@id": "https://voc.iudx.org.in/weatherType",
            "@type": [
                "iudx:TextProperty"
            ],
            "iudx:domainIncludes": [
                {
                    "@id": "iudx:EnvWeather"
                }
            ],
            "iudx:rangeIncludes": [
                {
                    "@id": "iudx:Text"
                },
                {
                    "@id": "iudx:ValueDescriptor"
                }
            ],
            "rdfs:comment": "Observed weather type or status. Represented by a comma separated list of weather types, e.g., cloudy, sunny etc.",
            "rdfs:isDefinedBy": {
                "@id": "https://voc.iudx.org.in/"
            },
            "rdfs:label": "weatherType",
            "skos:exactMatch": {
                "@id": "https://uri.fiware.org/ns/data-models#weatherType"
            }
        },
        {
            "@id": "https://voc.iudx.org.in/windDirection",
            "@type": [
                "iudx:QuantitativeProperty"
            ],
            "iudx:domainIncludes": [
                {
                    "@id": "iudx:EnvWeather"
                }
            ],
            "iudx:rangeIncludes": [
                {
                    "@id": "iudx:Number"
                },
                {
                    "@id": "iudx:ValueDescriptor"
                }
            ],
            "rdfs:comment": "Observed wind directiont. Measured in degrees clockwise from due north.",
            "rdfs:isDefinedBy": {
                "@id": "https://voc.iudx.org.in/"
            },
            "rdfs:label": "windDirection",
            "skos:exactMatch": {
                "@id": "https://uri.fiware.org/ns/data-models#windDirection"
            }
        },
        {
            "@id": "https://voc.iudx.org.in/windSpeed",
            "@type": [
                "iudx:QuantitativeProperty"
            ],
            "iudx:domainIncludes": [
                {
                    "@id": "iudx:EnvWeather"
                }
            ],
            "iudx:rangeIncludes": [
                {
                    "@id": "iudx:Number"
                },
                {
                    "@id": "iudx:ValueDescriptor"
                }
            ],
            "rdfs:comment": "Observed wind speed.",
            "rdfs:isDefinedBy": {
                "@id": "https://voc.iudx.org.in/"
            },
            "rdfs:label": "windSpeed",
            "skos:exactMatch": {
                "@id": "https://uri.fiware.org/ns/data-models#windSpeed"
            }
        },
        {
            "@id": "https://voc.iudx.org.in/actual_trip_end_time",
            "@type": [
                "iudx:TimeProperty"
            ],
            "iudx:domainIncludes": [
                {
                    "@id": "iudx:TransitManagement"
                }
            ],
            "iudx:rangeIncludes": [
                {
                    "@id": "iudx:DateTime"
                }
            ],
            "rdfs:comment": "This field specifies the time at which service or trip corresponding to this observation is scheduled to end.",
            "rdfs:isDefinedBy": {
                "@id": "https://voc.iudx.org.in/"
            },
            "rdfs:label": "actual_trip_end_time"
        },
        {
            "@id": "https://voc.iudx.org.in/actual_trip_start_time",
            "@type": [
                "iudx:TimeProperty"
            ],
            "iudx:domainIncludes": [
                {
                    "@id": "iudx:TransitManagement"
                }
            ],
            "iudx:rangeIncludes": [
                {
                    "@id": "iudx:DateTime"
                }
            ],
            "rdfs:comment": "This field specifies the time at which service actually began.  This is SameAs: absolute 'time'(StopTimeEvent) in the 'arrival' field of the stop_time_update (StopTimeUpdate) message of the GTFS Realtime message-TripUpdate (https://developers.google.com/transit/gtfs-realtime/reference#message-tripupdate)",
            "rdfs:isDefinedBy": {
                "@id": "https://voc.iudx.org.in/"
            },
            "rdfs:label": "actual_trip_start_time"
        },
        {
            "@id": "https://voc.iudx.org.in/ac_available",
            "@type": [
                "iudx:TextProperty"
            ],
            "iudx:domainIncludes": [
                {
                    "@id": "iudx:TransitManagement"
                }
            ],
            "iudx:rangeIncludes": [
                {
                    "@id": "iudx:Text"
                },
                {
                    "@id": "iudx:ValueDescriptor"
                }
            ],
            "rdfs:comment": "Describes the presence of air conditioning option in the vehicle corresponding to this observation.",
            "rdfs:isDefinedBy": {
                "@id": "https://voc.iudx.org.in/"
            },
            "rdfs:label": "ac_available"
        },
        {
            "@id": "https://voc.iudx.org.in/agency_fare_url",
            "@type": [
                "iudx:TextProperty"
            ],
            "iudx:domainIncludes": [
                {
                    "@id": "iudx:TransitManagement"
                },
                {
                    "@id": "iudx:BikeDockingStation"
                }
            ],
            "iudx:rangeIncludes": [
                {
                    "@id": "iudx:Text"
                },
                {
                    "@id": "iudx:ValueDescriptor"
                }
            ],
            "rdfs:comment": "URL of a web page that contains the details of the fares and also could allow to purchase tickets for that agency online. SameAs: 'agency_fare_url' field from GTFS Static Field Definition - agency.txt (https://developers.google.com/transit/gtfs/reference#agencytxt)",
            "rdfs:isDefinedBy": {
                "@id": "https://voc.iudx.org.in/"
            },
            "rdfs:label": "agency_fare_url",
            "skos:exactMatch": {
                "@id": "http://vocab.gtfs.org/gtfs.ttl#agency_fare_url"
            }
        },
        {
            "@id": "https://voc.iudx.org.in/agency_id",
            "@type": [
                "iudx:TextProperty"
            ],
            "iudx:domainIncludes": [
                {
                    "@id": "iudx:TransitManagement"
                }
            ],
            "iudx:rangeIncludes": [
                {
                    "@id": "iudx:Text"
                },
                {
                    "@id": "iudx:ValueDescriptor"
                }
            ],
            "rdfs:comment": "ID that uniquely identifies a transit agency. A transit feed may represent data from more than one agency. The agency_id is dataset unique. This field is optional for transit feeds that only contain data for a single agency. SameAs: 'agency_id' field from GTFS Static Field Definition - agency.txt (https://developers.google.com/transit/gtfs/reference#agencytxt)",
            "rdfs:isDefinedBy": {
                "@id": "https://voc.iudx.org.in/"
            },
            "rdfs:label": "agency_id",
            "skos:exactMatch": {
                "@id": "http://vocab.gtfs.org/gtfs.ttl#agency_id"
            }
        },
        {
            "@id": "https://voc.iudx.org.in/agency_lang",
            "@type": [
                "iudx:TextProperty"
            ],
            "iudx:domainIncludes": [
                {
                    "@id": "iudx:TransitManagement"
                }
            ],
            "iudx:rangeIncludes": [
                {
                    "@id": "iudx:Text"
                },
                {
                    "@id": "iudx:ValueDescriptor"
                }
            ],
            "rdfs:comment": "Contains a two-letter ISO 639-1 code for the primary language used by this transit agency. The language code is case-insensitive (both en and EN are accepted). SameAs: 'agency_lang' field from GTFS Static Field Definition - agency.txt (https://developers.google.com/transit/gtfs/reference#agencytxt)",
            "rdfs:isDefinedBy": {
                "@id": "https://voc.iudx.org.in/"
            },
            "rdfs:label": "agency_lang",
            "skos:exactMatch": {
                "@id": "http://vocab.gtfs.org/gtfs.ttl#agency_lang"
            }
        },
        {
            "@id": "https://voc.iudx.org.in/agency_name",
            "@type": [
                "iudx:TextProperty"
            ],
            "iudx:domainIncludes": [
                {
                    "@id": "iudx:TransitManagement"
                },
                {
                    "@id": "iudx:BikeDockingStation"
                }
            ],
            "iudx:rangeIncludes": [
                {
                    "@id": "iudx:Text"
                },
                {
                    "@id": "iudx:ValueDescriptor"
                }
            ],
            "rdfs:comment": "The agency_name field contains the full name of the transit agency. SameAs: 'agency_name' field from GTFS Static Field Definition - agency.txt (https://developers.google.com/transit/gtfs/reference#agencytxt)",
            "rdfs:isDefinedBy": {
                "@id": "https://voc.iudx.org.in/"
            },
            "rdfs:label": "agency_name",
            "skos:exactMatch": {
                "@id": "http://vocab.gtfs.org/gtfs.ttl#agency_name"
            }
        },
        {
            "@id": "https://voc.iudx.org.in/agency_timezone",
            "@type": [
                "iudx:TextProperty"
            ],
            "iudx:domainIncludes": [
                {
                    "@id": "iudx:TransitManagement"
                }
            ],
            "iudx:rangeIncludes": [
                {
                    "@id": "iudx:Text"
                },
                {
                    "@id": "iudx:ValueDescriptor"
                }
            ],
            "rdfs:comment": "Timezone field contains the timezone where the transit agency is located. SameAs: 'agency_timezone' field from GTFS Static Field Definition - agency.txt (https://developers.google.com/transit/gtfs/reference#agencytxt)",
            "rdfs:isDefinedBy": {
                "@id": "https://voc.iudx.org.in/"
            },
            "rdfs:label": "agency_timezone",
            "skos:exactMatch": {
                "@id": "http://vocab.gtfs.org/gtfs.ttl#agency_timezone"
            }
        },
        {
            "@id": "https://voc.iudx.org.in/agency_url",
            "@type": [
                "iudx:TextProperty"
            ],
            "iudx:domainIncludes": [
                {
                    "@id": "iudx:TransitManagement"
                },
                {
                    "@id": "iudx:BikeDockingStation"
                }
            ],
            "iudx:rangeIncludes": [
                {
                    "@id": "iudx:Text"
                },
                {
                    "@id": "iudx:ValueDescriptor"
                }
            ],
            "rdfs:comment": "The agency_url field contains the URL of the transit agency. SameAs: 'agency_url' field from GTFS Static Field Definition - agency.txt (https://developers.google.com/transit/gtfs/reference#agencytxt)",
            "rdfs:isDefinedBy": {
                "@id": "https://voc.iudx.org.in/"
            },
            "rdfs:label": "agency_url",
            "skos:exactMatch": {
                "@id": "http://vocab.gtfs.org/gtfs.ttl#agency_url"
            }
        },
        {
            "@id": "https://voc.iudx.org.in/arrival",
            "@type": [
                "iudx:StructuredProperty"
            ],
            "iudx:domainIncludes": [
                {
                    "@id": "iudx:TransitManagement"
                },
                {
                    "@id": "iudx:StopTimeUpdate"
                }
            ],
            "iudx:rangeIncludes": [
                {
                    "@id": "iudx:StopTimeEvent"
                }
            ],
            "rdfs:comment": "If schedule_relationship is empty or SCHEDULED, either arrival or departure must be provided within a StopTimeUpdate. SameAs: 'arrival' field from GTFS Realtime message-StopTimeUpdate (https://developers.google.com/transit/gtfs-realtime/reference#message-stoptimeupdate)",
            "rdfs:isDefinedBy": {
                "@id": "https://voc.iudx.org.in/"
            },
            "rdfs:label": "arrival"
        },
        {
            "@id": "https://voc.iudx.org.in/arrival_time",
            "@type": [
                "iudx:TimeProperty"
            ],
            "iudx:domainIncludes": [
                {
                    "@id": "iudx:TripDetails"
                },
                {
                    "@id": "iudx:TransitManagement"
                }
            ],
            "iudx:rangeIncludes": [
                {
                    "@id": "iudx:Text"
                },
                {
                    "@id": "iudx:ValueDescriptor"
                }
            ],
            "rdfs:comment": "Specifies the arrival time at a specific stop for a specific trip on a route. Times must be eight digits in HH:MM:SS format (HH:MM:SS is also accepted, if the hour begins with 0). \nNote: Trips that span multiple dates will have stop times greater than 24:00:00. For example, if a trip begins at 10:30:00 p.m. and ends at 2:15:00 a.m. on the following day, the stop times would be 22:30:00 and 26:15:00. Entering those stop times as 22:30:00 and 02:15:00 would not produce the desired results. SameAs: 'arrival_time' field from GTFS Static Field definitions-stop_times.txt (https://developers.google.com/transit/gtfs/reference#stop_timestxt)",
            "rdfs:isDefinedBy": {
                "@id": "https://voc.iudx.org.in/"
            },
            "rdfs:label": "arrival_time",
            "skos:exactMatch": {
                "@id": "http://vocab.gtfs.org/gtfs.ttl#arrival_time"
            }
        },
        {
            "@id": "https://voc.iudx.org.in/bearing",
            "@type": [
                "iudx:QuantitativeProperty"
            ],
            "iudx:domainIncludes": [
                {
                    "@id": "iudx:TransitManagement"
                },
                {
                    "@id": "iudx:WmgmtVehicle"
                }
            ],
            "iudx:rangeIncludes": [
                {
                    "@id": "iudx:Number"
                },
                {
                    "@id": "iudx:ValueDescriptor"
                }
            ],
            "rdfs:comment": "Gives the vehicle GPS angle measured in a clockwise direction from the True North. SameAs 'bearing' field from GTFS Realtime message-Position(https://developers.google.com/transit/gtfs-realtime/reference#message-position)",
            "rdfs:isDefinedBy": {
                "@id": "https://voc.iudx.org.in/"
            },
            "rdfs:label": "bearing",
            "skos:exactMatch": {
                "@id": "http://vocab.gtfs.org/gtfs.ttl#bearing"
            }
        },
        {
            "@id": "https://voc.iudx.org.in/current_status",
            "@type": [
                "iudx:TextProperty"
            ],
            "iudx:domainIncludes": [
                {
                    "@id": "iudx:TransitManagement"
                },
                {
                    "@id": "iudx:VehiclePosition"
                }
            ],
            "iudx:rangeIncludes": [
                {
                    "@id": "iudx:Text"
                },
                {
                    "@id": "iudx:ValueDescriptor"
                }
            ],
            "rdfs:comment": "Describes the status of the vehicle w.r.t the stop corresponding to this observation ENUM: [INCOMING_AT, STOPPED_AT, IN_TRANSIT_TO]. SameAs:'current_status' field from GTFS Realtime message-VehiclePosition(https://developers.google.com/transit/gtfs-realtime/reference#message-vehicleposition)",
            "rdfs:isDefinedBy": {
                "@id": "https://voc.iudx.org.in/"
            },
            "rdfs:label": "current_status"
        },
        {
            "@id": "https://voc.iudx.org.in/current_stop_sequence",
            "@type": [
                "iudx:QuantitativeProperty"
            ],
            "iudx:domainIncludes": [
                {
                    "@id": "iudx:TransitManagement"
                },
                {
                    "@id": "iudx:VehiclePosition"
                }
            ],
            "iudx:rangeIncludes": [
                {
                    "@id": "iudx:Number"
                },
                {
                    "@id": "iudx:ValueDescriptor"
                }
            ],
            "rdfs:comment": "Gives the stop sequence index of the current stop. This is determined by considering current_status, if current_status is missing IN_TRANSIT_TO is assumed. SameAs:'current_stop_sequence' field from GTFS Realtime message-VehiclePosition(https://developers.google.com/transit/gtfs-realtime/reference#message-vehicleposition)",
            "rdfs:isDefinedBy": {
                "@id": "https://voc.iudx.org.in/"
            },
            "rdfs:label": "current_stop_sequence"
        },
        {
            "@id": "https://voc.iudx.org.in/departure",
            "@type": [
                "iudx:StructuredProperty"
            ],
            "iudx:domainIncludes": [
                {
                    "@id": "iudx:TransitManagement"
                },
                {
                    "@id": "iudx:StopTimeUpdate"
                }
            ],
            "iudx:rangeIncludes": [
                {
                    "@id": "iudx:StopTimeEvent"
                }
            ],
            "rdfs:comment": "If schedule_relationship is empty or SCHEDULED, either arrival or departure must be provided within a StopTimeUpdate. SameAs: 'departure' field from GTFS Realtime message-StopTimeUpdate (https://developers.google.com/transit/gtfs-realtime/reference#message-stoptimeupdate)",
            "rdfs:isDefinedBy": {
                "@id": "https://voc.iudx.org.in/"
            },
            "rdfs:label": "departure"
        },
        {
            "@id": "https://voc.iudx.org.in/departure_time",
            "@type": [
                "iudx:TimeProperty"
            ],
            "iudx:domainIncludes": [
                {
                    "@id": "iudx:TripDetails"
                },
                {
                    "@id": "iudx:TransitManagement"
                }
            ],
            "iudx:rangeIncludes": [
                {
                    "@id": "iudx:Text"
                },
                {
                    "@id": "iudx:ValueDescriptor"
                }
            ],
            "rdfs:comment": "Specifies the departure time from a specific stop for a specific trip on a route. Times must be eight digits in HH:MM:SS format (HH:MM:SS is also accepted, if the hour begins with 0). \nNote: Trips that span multiple dates will have stop times greater than 24:00:00. For example, if a trip begins at 10:30:00 p.m. and ends at 2:15:00 a.m. on the following day, the stop times would be 22:30:00 and 26:15:00. Entering those stop times as 22:30:00 and 02:15:00 would not produce the desired results. SameAs: 'departure_time' field from GTFS Static Field definitions-stop_times.txt (https://developers.google.com/transit/gtfs/reference#stop_timestxt)",
            "rdfs:isDefinedBy": {
                "@id": "https://voc.iudx.org.in/"
            },
            "rdfs:label": "departure_time",
            "skos:exactMatch": {
                "@id": "http://vocab.gtfs.org/gtfs.ttl#departure_time"
            }
        },
        {
            "@id": "https://voc.iudx.org.in/depot_id",
            "@type": [
                "iudx:TextProperty"
            ],
            "iudx:domainIncludes": [
                {
                    "@id": "iudx:TransitManagement"
                }
            ],
            "iudx:rangeIncludes": [
                {
                    "@id": "iudx:Text"
                },
                {
                    "@id": "iudx:ValueDescriptor"
                }
            ],
            "rdfs:comment": "Describes the unique id of the bus depot corresponding to this observation.",
            "rdfs:isDefinedBy": {
                "@id": "https://voc.iudx.org.in/"
            },
            "rdfs:label": "depot_id"
        },
        {
            "@id": "https://voc.iudx.org.in/depot_name",
            "@type": [
                "iudx:TextProperty"
            ],
            "iudx:domainIncludes": [
                {
                    "@id": "iudx:TransitManagement"
                }
            ],
            "iudx:rangeIncludes": [
                {
                    "@id": "iudx:Text"
                },
                {
                    "@id": "iudx:ValueDescriptor"
                }
            ],
            "rdfs:comment": "Describes the depot name of the bus depot corresponding to this observation.",
            "rdfs:isDefinedBy": {
                "@id": "https://voc.iudx.org.in/"
            },
            "rdfs:label": "depot_name"
        },
        {
            "@id": "https://voc.iudx.org.in/direction_id",
            "@type": [
                "iudx:QuantitativeProperty"
            ],
            "iudx:domainIncludes": [
                {
                    "@id": "iudx:TransitManagement"
                },
                {
                    "@id": "iudx:TripDescriptor"
                },
                {
                    "@id": "iudx:FareCollectionSystem"
                }
            ],
            "iudx:rangeIncludes": [
                {
                    "@id": "iudx:Number"
                },
                {
                    "@id": "iudx:ValueDescriptor"
                }
            ],
            "rdfs:comment": "Indicates the direction of travel of the vehicle corresponding to this observation, can be referenced from the GTFS static feed trips.txt. SameAs: 'direction_id' field from GTFS Realtime message-TripDescriptor (https://developers.google.com/transit/gtfs-realtime/reference#message-tripdescriptor)",
            "rdfs:isDefinedBy": {
                "@id": "https://voc.iudx.org.in/"
            },
            "rdfs:label": "direction_id"
        },
        {
            "@id": "https://voc.iudx.org.in/entity_id",
            "@type": [
                "iudx:TextProperty"
            ],
            "iudx:domainIncludes": [
                {
                    "@id": "iudx:TransitManagement"
                },
                {
                    "@id": "iudx:FeedEntity"
                }
            ],
            "iudx:rangeIncludes": [
                {
                    "@id": "iudx:Text"
                },
                {
                    "@id": "iudx:ValueDescriptor"
                }
            ],
            "rdfs:comment": "Feed unique ID for the entity coressponding to this observation.SameAs:'entity_id' field from GTFS Realtime message-FeedEntity(https://developers.google.com/transit/gtfs-realtime/reference#message-feedentity)",
            "rdfs:isDefinedBy": {
                "@id": "https://voc.iudx.org.in/"
            },
            "rdfs:label": "entity_id"
        },
        {
            "@id": "https://voc.iudx.org.in/last_stop_arrival_time",
            "@type": [
                "iudx:TimeProperty"
            ],
            "iudx:domainIncludes": [
                {
                    "@id": "iudx:TransitManagement"
                }
            ],
            "iudx:rangeIncludes": [
                {
                    "@id": "iudx:Text"
                },
                {
                    "@id": "iudx:ValueDescriptor"
                }
            ],
            "rdfs:comment": "Specifies the arrival time at the previous stop for a specific trip on a route. Times must be eight digits in HH:MM:SS format (H:MM:SS is also accepted, if the hour begins with 0). \nNote: Trips that span multiple dates will have stop times greater than 24:00:00. For example, if a trip begins at 10:30:00 p.m. and ends at 2:15:00 a.m. on the following day, the stop times would be 22:30:00 and 26:15:00. Entering those stop times as 22:30:00 and 02:15:00 would not produce the desired results. This is SameAs: absolute 'time'(StopTimeEvent) in the 'arrival' field of the stop_time_update (StopTimeUpdate) message of the GTFS Realtime message-TripUpdate (https://developers.google.com/transit/gtfs-realtime/reference#message-tripupdate)",
            "rdfs:isDefinedBy": {
                "@id": "https://voc.iudx.org.in/"
            },
            "rdfs:label": "last_stop_arrival_time",
            "skos:exactMatch": {
                "@id": "http://vocab.gtfs.org/gtfs.ttl#arrival_time"
            }
        },
        {
            "@id": "https://voc.iudx.org.in/last_stop_id",
            "@type": [
                "iudx:TextProperty"
            ],
            "iudx:domainIncludes": [
                {
                    "@id": "iudx:TransitManagement"
                }
            ],
            "iudx:rangeIncludes": [
                {
                    "@id": "iudx:Text"
                },
                {
                    "@id": "iudx:ValueDescriptor"
                }
            ],
            "rdfs:comment": "Stop ID/Stop name of the previous bus stop corresponding to the bus in this observation. SameAs: 'stop_id' field from GTFS Realtime message-VehiclePosition (https://developers.google.com/transit/gtfs-realtime/reference#message-vehicleposition)",
            "rdfs:isDefinedBy": {
                "@id": "https://voc.iudx.org.in/"
            },
            "rdfs:label": "last_stop_id"
        },
        {
            "@id": "https://voc.iudx.org.in/last_tracked_time",
            "@type": [
                "iudx:TimeProperty"
            ],
            "iudx:domainIncludes": [
                {
                    "@id": "iudx:TransitManagement"
                }
            ],
            "iudx:rangeIncludes": [
                {
                    "@id": "iudx:DateTime"
                }
            ],
            "rdfs:comment": "Gives the time at which the vehicle was last tracked.",
            "rdfs:isDefinedBy": {
                "@id": "https://voc.iudx.org.in/"
            },
            "rdfs:label": "last_tracked_time"
        },
        {
            "@id": "https://voc.iudx.org.in/license_plate",
            "@type": [
                "iudx:TextProperty"
            ],
            "iudx:domainIncludes": [
                {
                    "@id": "iudx:TransitManagement"
                },
                {
                    "@id": "iudx:WmgmtBin"
                },
                {
                    "@id": "iudx:WmgmtVehicle"
                },
                {
                    "@id": "iudx:VehicleDescriptor"
                }
            ],
            "iudx:rangeIncludes": [
                {
                    "@id": "iudx:Text"
                },
                {
                    "@id": "iudx:ValueDescriptor"
                }
            ],
            "rdfs:comment": "Gives the License Plate number of the vehice. SameAs: 'license_plate' field from GTFS Realtime message-VehicleDescriptor (https://developers.google.com/transit/gtfs-realtime/reference#message-vehicledescriptor)",
            "rdfs:isDefinedBy": {
                "@id": "https://voc.iudx.org.in/"
            },
            "rdfs:label": "license_plate"
        },
        {
            "@id": "https://voc.iudx.org.in/position",
            "@type": [
                "iudx:StructuredProperty"
            ],
            "iudx:domainIncludes": [
                {
                    "@id": "iudx:TransitManagement"
                },
                {
                    "@id": "iudx:VehiclePosition"
                }
            ],
            "iudx:rangeIncludes": [
                {
                    "@id": "iudx:GeoCoordinates"
                }
            ],
            "rdfs:comment": "Deccribes the current position of the vehicle corresponding to this observation. SameAs:'position' field from GTFS Realtime message-VehiclePosition(https://developers.google.com/transit/gtfs-realtime/reference#message-vehicleposition)",
            "rdfs:isDefinedBy": {
                "@id": "https://voc.iudx.org.in/"
            },
            "rdfs:label": "position"
        },
        {
            "@id": "https://voc.iudx.org.in/routeStopSequence",
            "@type": [
                "iudx:TextProperty"
            ],
            "iudx:domainIncludes": [
                {
                    "@id": "iudx:TransitManagement"
                }
            ],
            "iudx:rangeIncludes": [
                {
                    "@container": "@list",
                    "@id": "iudx:Text"
                },
                {
                    "@id": "iudx:ValueDescriptor"
                }
            ],
            "rdfs:comment": "Gives the stop IDs/stop codes or station IDs/station codes in the right sequence for the route or line corresponding to this observation.",
            "rdfs:isDefinedBy": {
                "@id": "https://voc.iudx.org.in/"
            },
            "rdfs:label": "routeStopSequence"
        },
        {
            "@id": "https://voc.iudx.org.in/route_color",
            "@type": [
                "iudx:TextProperty"
            ],
            "iudx:domainIncludes": [
                {
                    "@id": "iudx:TransitManagement"
                }
            ],
            "iudx:rangeIncludes": [
                {
                    "@id": "iudx:Text"
                },
                {
                    "@id": "iudx:ValueDescriptor"
                }
            ],
            "rdfs:comment": "If assigned, this field defines a color that corresponds to a route. The color must be provided as a six-character hexadecimal number, for example, 00FFFF. If no color is specified, the default route color is white (FFFFFF). SameAs: 'route_color' field from GTFS Static Field definitions-routes.txt (https://developers.google.com/transit/gtfs/reference#routestxt)",
            "rdfs:isDefinedBy": {
                "@id": "https://voc.iudx.org.in/"
            },
            "rdfs:label": "route_color",
            "skos:exactMatch": {
                "@id": "http://vocab.gtfs.org/gtfs.ttl#route_color"
            }
        },
        {
            "@id": "https://voc.iudx.org.in/route_desc",
            "@type": [
                "iudx:TextProperty"
            ],
            "iudx:domainIncludes": [
                {
                    "@id": "iudx:TransitManagement"
                }
            ],
            "iudx:rangeIncludes": [
                {
                    "@id": "iudx:Text"
                },
                {
                    "@id": "iudx:ValueDescriptor"
                }
            ],
            "rdfs:comment": "Description of the route. This can include the entire route details including to and from destination and timing information in a text description form. SameAs: 'route_desc' field from GTFS Static Field definitions-routes.txt (https://developers.google.com/transit/gtfs/reference#routestxt)",
            "rdfs:isDefinedBy": {
                "@id": "https://voc.iudx.org.in/"
            },
            "rdfs:label": "route_desc",
            "skos:exactMatch": {
                "@id": "http://vocab.gtfs.org/gtfs.ttl#route_desc"
            }
        },
        {
            "@id": "https://voc.iudx.org.in/route_id",
            "@type": [
                "iudx:TextProperty"
            ],
            "iudx:domainIncludes": [
                {
                    "@id": "iudx:TransitManagement"
                },
                {
                    "@id": "iudx:TripDescriptor"
                },
                {
                    "@id": "iudx:FareCollectionSystem"
                }
            ],
            "iudx:rangeIncludes": [
                {
                    "@id": "iudx:Text"
                },
                {
                    "@id": "iudx:ValueDescriptor"
                }
            ],
            "rdfs:comment": "Route ID assigned to the route on which the bus/vehicle corresponding to the bus in this observation is currently plying on. SameAs: 'route_id' field from GTFS Realtime message-TripDescriptor (https://developers.google.com/transit/gtfs-realtime/reference#message-tripdescriptor)",
            "rdfs:isDefinedBy": {
                "@id": "https://voc.iudx.org.in/"
            },
            "rdfs:label": "route_id"
        },
        {
            "@id": "https://voc.iudx.org.in/route_long_name",
            "@type": [
                "iudx:TextProperty"
            ],
            "iudx:domainIncludes": [
                {
                    "@id": "iudx:TransitManagement"
                }
            ],
            "iudx:rangeIncludes": [
                {
                    "@id": "iudx:Text"
                },
                {
                    "@id": "iudx:ValueDescriptor"
                }
            ],
            "rdfs:comment": "Full name of a route. This name is more descriptive than the routeShortName and often includes the route's destination or stop. This mostly includes the to and from destination names of the route. SameAs: 'route_long_name' field from GTFS Static Field definitions-routes.txt (https://developers.google.com/transit/gtfs/reference#routestxt)",
            "rdfs:isDefinedBy": {
                "@id": "https://voc.iudx.org.in/"
            },
            "rdfs:label": "route_long_name",
            "skos:exactMatch": {
                "@id": "http://vocab.gtfs.org/gtfs.ttl#route_long_name"
            }
        },
        {
            "@id": "https://voc.iudx.org.in/route_short_name",
            "@type": [
                "iudx:TextProperty"
            ],
            "iudx:domainIncludes": [
                {
                    "@id": "iudx:TransitManagement"
                }
            ],
            "iudx:rangeIncludes": [
                {
                    "@id": "iudx:Text"
                },
                {
                    "@id": "iudx:ValueDescriptor"
                }
            ],
            "rdfs:comment": "Short name of a route. This will often be the transit vehicle's board name like \"402D\",  or \"Green\" that riders use to identify a route. SameAs: 'route_short_name' field from GTFS Static Field definitions-routes.txt (https://developers.google.com/transit/gtfs/reference#routestxt)",
            "rdfs:isDefinedBy": {
                "@id": "https://voc.iudx.org.in/"
            },
            "rdfs:label": "route_short_name",
            "skos:exactMatch": {
                "@id": "http://vocab.gtfs.org/gtfs.ttl#route_short_name"
            }
        },
        {
            "@id": "https://voc.iudx.org.in/route_text_color",
            "@type": [
                "iudx:TextProperty"
            ],
            "iudx:domainIncludes": [
                {
                    "@id": "iudx:TransitManagement"
                }
            ],
            "iudx:rangeIncludes": [
                {
                    "@id": "iudx:Text"
                },
                {
                    "@id": "iudx:ValueDescriptor"
                }
            ],
            "rdfs:comment": "This field can be used to specify a legible color to use for text drawn against a background of route_color. The color must be provided as a six-character hexadecimal number, for example, FFD700. If no color is specified, the default text color is black (000000). SameAs: 'route_text_color' field from GTFS Static Field definitions-routes.txt (https://developers.google.com/transit/gtfs/reference#routestxt)",
            "rdfs:isDefinedBy": {
                "@id": "https://voc.iudx.org.in/"
            },
            "rdfs:label": "route_text_color",
            "skos:exactMatch": {
                "@id": "http://vocab.gtfs.org/gtfs.ttl#route_text_color"
            }
        },
        {
            "@id": "https://voc.iudx.org.in/route_type",
            "@type": [
                "iudx:TextProperty"
            ],
            "iudx:domainIncludes": [
                {
                    "@id": "iudx:TransitManagement"
                }
            ],
            "iudx:rangeIncludes": [
                {
                    "@id": "iudx:Text"
                },
                {
                    "@id": "iudx:Number"
                },
                {
                    "@id": "iudx:ValueDescriptor"
                }
            ],
            "rdfs:comment": "Number indicating the type of transport-\n1 - Subway, Metro. Any underground rail system within a metropolitan area.\n2 - Rail. Used for intercity or long-distance travel.\n3 - Bus. Used for short- and long-distance bus routes. \nSameAs: 'route_type' field from GTFS Static Field definitions-routes.txt (https://developers.google.com/transit/gtfs/reference#routestxt)",
            "rdfs:isDefinedBy": {
                "@id": "https://voc.iudx.org.in/"
            },
            "rdfs:label": "route_type",
            "skos:exactMatch": {
                "@id": "http://vocab.gtfs.org/gtfs.ttl#route_type"
            }
        },
        {
            "@id": "https://voc.iudx.org.in/route_url",
            "@type": [
                "iudx:TextProperty"
            ],
            "iudx:domainIncludes": [
                {
                    "@id": "iudx:TransitManagement"
                }
            ],
            "iudx:rangeIncludes": [
                {
                    "@id": "iudx:Text"
                },
                {
                    "@id": "iudx:ValueDescriptor"
                }
            ],
            "rdfs:comment": "Contains the URL of a web page about that particular route and is different from the agency_url. SameAs: 'route_url' field from GTFS Static Field definitions-routes.txt (https://developers.google.com/transit/gtfs/reference#routestxt)",
            "rdfs:isDefinedBy": {
                "@id": "https://voc.iudx.org.in/"
            },
            "rdfs:label": "route_url",
            "skos:exactMatch": {
                "@id": "http://vocab.gtfs.org/gtfs.ttl#route_url"
            }
        },
        {
            "@id": "https://voc.iudx.org.in/schedule_relationship",
            "@type": [
                "iudx:TextProperty"
            ],
            "iudx:domainIncludes": [
                {
                    "@id": "iudx:TransitManagement"
                },
                {
                    "@id": "iudx:TripDescriptor"
                },
                {
                    "@id": "iudx:StopTimeUpdate"
                }
            ],
            "iudx:rangeIncludes": [
                {
                    "@id": "iudx:Text"
                },
                {
                    "@id": "iudx:ValueDescriptor"
                }
            ],
            "rdfs:comment": "Describes if the Route/Trip has been scheduled. SameAs: 'schedule_relationship' field from enumScheduleRelationship (https://developers.google.com/transit/gtfs-realtime/reference#enum-schedulerelationship-2)",
            "rdfs:isDefinedBy": {
                "@id": "https://voc.iudx.org.in/"
            },
            "rdfs:label": "schedule_relationship",
            "skos:exactMatch": {
                "@id": "http://vocab.gtfs.org/gtfs.ttl#schedule_relationship"
            }
        },
        {
            "@id": "https://voc.iudx.org.in/seating_capacity",
            "@type": [
                "iudx:QuantitativeProperty"
            ],
            "iudx:domainIncludes": [
                {
                    "@id": "iudx:TransitManagement"
                }
            ],
            "iudx:rangeIncludes": [
                {
                    "@id": "iudx:Number"
                },
                {
                    "@id": "iudx:ValueDescriptor"
                }
            ],
            "rdfs:comment": "Describes the passenger seating capacity of the vehicle corresponding to this observation.",
            "rdfs:isDefinedBy": {
                "@id": "https://voc.iudx.org.in/"
            },
            "rdfs:label": "seating_capacity"
        },
        {
            "@id": "https://voc.iudx.org.in/speed",
            "@type": [
                "iudx:QuantitativeProperty"
            ],
            "iudx:domainIncludes": [
                {
                    "@id": "iudx:TransitManagement"
                },
                {
                    "@id": "iudx:WmgmtVehicle"
                }
            ],
            "iudx:rangeIncludes": [
                {
                    "@id": "iudx:Number"
                },
                {
                    "@id": "iudx:ValueDescriptor"
                }
            ],
            "rdfs:comment": "Gives the Speed  of the vehicle.SameAs 'speed' field from GTFS Realtime message-Position(https://developers.google.com/transit/gtfs-realtime/reference#message-position)",
            "rdfs:isDefinedBy": {
                "@id": "https://voc.iudx.org.in/"
            },
            "rdfs:label": "speed",
            "skos:exactMatch": {
                "@id": "http://vocab.gtfs.org/gtfs.ttl#speed"
            }
        },
        {
            "@id": "https://voc.iudx.org.in/standing_capacity",
            "@type": [
                "iudx:QuantitativeProperty"
            ],
            "iudx:domainIncludes": [
                {
                    "@id": "iudx:TransitManagement"
                }
            ],
            "iudx:rangeIncludes": [
                {
                    "@id": "iudx:Number"
                },
                {
                    "@id": "iudx:ValueDescriptor"
                }
            ],
            "rdfs:comment": "Describes the passenger standing capacity of the vehicle corresponding to this observation.",
            "rdfs:isDefinedBy": {
                "@id": "https://voc.iudx.org.in/"
            },
            "rdfs:label": "standing_capacity"
        },
        {
            "@id": "https://voc.iudx.org.in/start_date",
            "@type": [
                "iudx:TextProperty"
            ],
            "iudx:domainIncludes": [
                {
                    "@id": "iudx:TransitManagement"
                },
                {
                    "@id": "iudx:TripDescriptor"
                }
            ],
            "iudx:rangeIncludes": [
                {
                    "@id": "iudx:Text"
                },
                {
                    "@id": "iudx:ValueDescriptor"
                }
            ],
            "rdfs:comment": "Describes the initial scheduled date of the trip corresponding to the vehicle this observation. An example format for this field - YYYYMMDD. SameAs: 'start_date' field from GTFS Realtime message-TripDescriptor (https://developers.google.com/transit/gtfs-realtime/reference#message-tripdescriptor)",
            "rdfs:isDefinedBy": {
                "@id": "https://voc.iudx.org.in/"
            },
            "rdfs:label": "start_date"
        },
        {
            "@id": "https://voc.iudx.org.in/start_time",
            "@type": [
                "iudx:TimeProperty"
            ],
            "iudx:domainIncludes": [
                {
                    "@id": "iudx:TransitManagement"
                },
                {
                    "@id": "iudx:TripDescriptor"
                }
            ],
            "iudx:rangeIncludes": [
                {
                    "@id": "iudx:Text"
                },
                {
                    "@id": "iudx:ValueDescriptor"
                }
            ],
            "rdfs:comment": "Describes the initial scheduled start time of the trip corresponding to the vehicle this observation. An example format for this field - 11:15:35 or 25:15:35. SameAs: 'start_time' field from GTFS Realtime message-TripDescriptor (https://developers.google.com/transit/gtfs-realtime/reference#message-tripdescriptor)",
            "rdfs:isDefinedBy": {
                "@id": "https://voc.iudx.org.in/"
            },
            "rdfs:label": "start_time"
        },
        {
            "@id": "https://voc.iudx.org.in/stop_code",
            "@type": [
                "iudx:TextProperty"
            ],
            "iudx:domainIncludes": [
                {
                    "@id": "iudx:TransitManagement"
                }
            ],
            "iudx:rangeIncludes": [
                {
                    "@id": "iudx:Text"
                },
                {
                    "@id": "iudx:ValueDescriptor"
                }
            ],
            "rdfs:comment": "This field contains short text or a number that uniquely identifies the stop for passengers. Can be same as stop_id if it is for public. SameAs: 'stop_code' field from GTFS Static Field definitions-stops.txt (https://developers.google.com/transit/gtfs/reference#stopstxt)",
            "rdfs:isDefinedBy": {
                "@id": "https://voc.iudx.org.in/"
            },
            "rdfs:label": "stop_code",
            "skos:exactMatch": {
                "@id": "http://vocab.gtfs.org/gtfs.ttl#stop_code"
            }
        },
        {
            "@id": "https://voc.iudx.org.in/stop_desc",
            "@type": [
                "iudx:TextProperty"
            ],
            "iudx:domainIncludes": [
                {
                    "@id": "iudx:TransitManagement"
                }
            ],
            "iudx:rangeIncludes": [
                {
                    "@id": "iudx:Text"
                },
                {
                    "@id": "iudx:ValueDescriptor"
                }
            ],
            "rdfs:comment": "This field contains a description of a stop. SameAs: 'stop_desc' field from GTFS Static Field definitions-stops.txt (https://developers.google.com/transit/gtfs/reference#stopstxt)",
            "rdfs:isDefinedBy": {
                "@id": "https://voc.iudx.org.in/"
            },
            "rdfs:label": "stop_desc",
            "skos:exactMatch": {
                "@id": "http://vocab.gtfs.org/gtfs.ttl#stop_desc"
            }
        },
        {
            "@id": "https://voc.iudx.org.in/stop_headsign",
            "@type": [
                "iudx:TextProperty"
            ],
            "iudx:domainIncludes": [
                {
                    "@id": "iudx:TripDetails"
                },
                {
                    "@id": "iudx:TransitManagement"
                }
            ],
            "iudx:rangeIncludes": [
                {
                    "@id": "iudx:Text"
                },
                {
                    "@id": "iudx:ValueDescriptor"
                }
            ],
            "rdfs:comment": "This field contains the text that appears on a sign that identifies the trip\u2019s destination to passengers. SameAs: 'stop_headsign' field from GTFS Static Field definitions-stop_times.txt (https://developers.google.com/transit/gtfs/reference#stop_timestxt)",
            "rdfs:isDefinedBy": {
                "@id": "https://voc.iudx.org.in/"
            },
            "rdfs:label": "stop_headsign",
            "skos:exactMatch": {
                "@id": "http://vocab.gtfs.org/gtfs.ttl#stop_headsign"
            }
        },
        {
            "@id": "https://voc.iudx.org.in/stop_id",
            "@type": [
                "iudx:TextProperty"
            ],
            "iudx:domainIncludes": [
                {
                    "@id": "iudx:TransitManagement"
                },
                {
                    "@id": "iudx:VehicePosition"
                },
                {
                    "@id": "iudx:StopTimeUpdate"
                },
                {
                    "@id": "iudx:TripDetails"
                },
                {
                    "@id": "iudx:Sequence"
                }
            ],
            "iudx:rangeIncludes": [
                {
                    "@id": "iudx:Text"
                },
                {
                    "@id": "iudx:ValueDescriptor"
                }
            ],
            "rdfs:comment": "Stop ID/Stop name of the bus stops corresponding to the bus in this observation. SameAs: 'stop_id' field from GTFS Realtime message-Vehicleposition (https://developers.google.com/transit/gtfs-realtime/reference#message-vehicleposition)",
            "rdfs:isDefinedBy": {
                "@id": "https://voc.iudx.org.in/"
            },
            "rdfs:label": "stop_id",
            "skos:exactMatch": {
                "@id": "http://vocab.gtfs.org/gtfs.ttl#stop_id"
            }
        },
        {
            "@id": "https://voc.iudx.org.in/stop_name",
            "@type": [
                "iudx:TextProperty"
            ],
            "iudx:domainIncludes": [
                {
                    "@id": "iudx:TransitManagement"
                }
            ],
            "iudx:rangeIncludes": [
                {
                    "@id": "iudx:Text"
                },
                {
                    "@id": "iudx:ValueDescriptor"
                }
            ],
            "rdfs:comment": "Describes the name of the Bus Stop. SameAs: 'stop_name' field from GTFS Static Field definitions-stops.txt (https://developers.google.com/transit/gtfs/reference#stopstxt)",
            "rdfs:isDefinedBy": {
                "@id": "https://voc.iudx.org.in/"
            },
            "rdfs:label": "stop_name",
            "skos:exactMatch": {
                "@id": "http://vocab.gtfs.org/gtfs.ttl#stop_name"
            }
        },
        {
            "@id": "https://voc.iudx.org.in/stop_sequence",
            "@type": [
                "iudx:QuantitativeProperty"
            ],
            "iudx:domainIncludes": [
                {
                    "@id": "iudx:TransitManagement"
                },
                {
                    "@id": "iudx:StopTimeUpdate"
                },
                {
                    "@id": "iudx:TripDetails"
                },
                {
                    "@id": "iudx:Sequence"
                }
            ],
            "iudx:rangeIncludes": [
                {
                    "@id": "iudx:Number"
                },
                {
                    "@id": "iudx:ValueDescriptor"
                }
            ],
            "rdfs:comment": "Indicates the stop sequencel of the vehicle corresponding to this observation, can be referenced from the GTFS static feed stop_times.txt. SameAs: 'stop_sequence' field from GTFS Realtime message-StopTimeUpdate (https://developers.google.com/transit/gtfs-realtime/reference#message-stoptimeupdate)",
            "rdfs:isDefinedBy": {
                "@id": "https://voc.iudx.org.in/"
            },
            "rdfs:label": "stop_sequence"
        },
        {
            "@id": "https://voc.iudx.org.in/stop_sequence_detail",
            "@type": [
                "iudx:StructuredProperty"
            ],
            "iudx:domainIncludes": [
                {
                    "@id": "iudx:TransitManagement"
                }
            ],
            "iudx:rangeIncludes": [
                {
                    "@id": "iudx:Sequence"
                }
            ],
            "rdfs:comment": "Describes the stop sequence for a trip in the designated route made by the public transit vehicle. SameAs: 'stop_sequence' field from GTFS Static Field definitions-stop_times.txt (https://developers.google.com/transit/gtfs/reference#stop_timestxt)",
            "rdfs:isDefinedBy": {
                "@id": "https://voc.iudx.org.in/"
            },
            "rdfs:label": "stop_sequence_detail",
            "skos:exactMatch": {
                "@id": "http://vocab.gtfs.org/gtfs.ttl#stop_sequence"
            }
        },
        {
            "@id": "https://voc.iudx.org.in/stop_time_update",
            "@type": [
                "iudx:StructuredProperty"
            ],
            "iudx:domainIncludes": [
                {
                    "@id": "iudx:TransitManagement"
                },
                {
                    "@id": "iudx:TripUpdate"
                }
            ],
            "iudx:rangeIncludes": [
                {
                    "@id": "iudx:StopTimeUpdate"
                }
            ],
            "rdfs:comment": "Updated sorted stop sequence for the trip made by the vehicle corresponding to this observation, not to be considered if schedule_realtionship is \"CANCELED\". SameAs: 'stop_time_update' field from GTFS Realtime message-TripUpdate (https://developers.google.com/transit/gtfs-realtime/reference#message-tripupdate)",
            "rdfs:isDefinedBy": {
                "@id": "https://voc.iudx.org.in/"
            },
            "rdfs:label": "stop_time_update"
        },
        {
            "@id": "https://voc.iudx.org.in/stop_url",
            "@type": [
                "iudx:TextProperty"
            ],
            "iudx:domainIncludes": [
                {
                    "@id": "iudx:TransitManagement"
                }
            ],
            "iudx:rangeIncludes": [
                {
                    "@id": "iudx:Text"
                },
                {
                    "@id": "iudx:ValueDescriptor"
                }
            ],
            "rdfs:comment": "This field contains the URL of a web page about a particular stop and is different from the agency_url and the route_url fields. SameAs: 'stop_url' field from GTFS Static Field definitions-stops.txt (https://developers.google.com/transit/gtfs/reference#stopstxt)",
            "rdfs:isDefinedBy": {
                "@id": "https://voc.iudx.org.in/"
            },
            "rdfs:label": "stop_url",
            "skos:exactMatch": {
                "@id": "http://vocab.gtfs.org/gtfs.ttl#stop_url"
            }
        },
        {
            "@id": "https://voc.iudx.org.in/timestamp",
            "@type": [
                "iudx:TimeProperty"
            ],
            "iudx:domainIncludes": [
                {
                    "@id": "iudx:TransitManagement"
                },
                {
                    "@id": "iudx:VehiclePosition"
                },
                {
                    "@id": "iudx:TripUpdate"
                }
            ],
            "iudx:rangeIncludes": [
                {
                    "@id": "iudx:DateTime"
                },
                {
                    "@id": "iudx:ValueDescriptor"
                }
            ],
            "rdfs:comment": "Last reported time of observation from the vehicle. SameAs: 'timestamp' field from GTFS Realtime message-Vehicleposition (https://developers.google.com/transit/gtfs-realtime/reference#message-vehicleposition)",
            "rdfs:isDefinedBy": {
                "@id": "https://voc.iudx.org.in/"
            },
            "rdfs:label": "timestamp",
            "skos:exactMatch": {
                "@id": "http://vocab.gtfs.org/gtfs.ttl#timestamp"
            }
        },
        {
            "@id": "https://voc.iudx.org.in/travelDistance",
            "@type": [
                "iudx:QuantitativeProperty"
            ],
            "iudx:domainIncludes": [
                {
                    "@id": "iudx:TransitManagement"
                },
                {
                    "@id": "iudx:FareCollectionSystem"
                }
            ],
            "iudx:rangeIncludes": [
                {
                    "@id": "iudx:Number"
                },
                {
                    "@id": "iudx:ValueDescriptor"
                }
            ],
            "rdfs:comment": "The distance between the orgin bus stop and the destination bus stop corresponding to this observation.",
            "rdfs:isDefinedBy": {
                "@id": "https://voc.iudx.org.in/"
            },
            "rdfs:label": "travelDistance"
        },
        {
            "@id": "https://voc.iudx.org.in/travelTime",
            "@type": [
                "iudx:TimeProperty"
            ],
            "iudx:domainIncludes": [
                {
                    "@id": "iudx:TransitManagement"
                }
            ],
            "iudx:rangeIncludes": [
                {
                    "@id": "iudx:Text"
                },
                {
                    "@id": "iudx:ValueDescriptor"
                }
            ],
            "rdfs:comment": "The time taken to travel between the orgin bus stop and the destination bus stop corresponding to this observation in HH:MM:SS format(HH:MM:SS is also accepted, if the hour begins with 0).",
            "rdfs:isDefinedBy": {
                "@id": "https://voc.iudx.org.in/"
            },
            "rdfs:label": "travelTime"
        },
        {
            "@id": "https://voc.iudx.org.in/trip",
            "@type": [
                "iudx:StructuredProperty"
            ],
            "iudx:domainIncludes": [
                {
                    "@id": "iudx:TransitManagement"
                },
                {
                    "@id": "iudx:VehiclePosition"
                },
                {
                    "@id": "iudx:TripUpdate"
                }
            ],
            "iudx:rangeIncludes": [
                {
                    "@id": "iudx:TripDescriptor"
                }
            ],
            "rdfs:comment": "Describes the trip the vehicle corresponding to this observation is making. SameAs:'trip' field from GTFS Realtime message-VehiclePosition(https://developers.google.com/transit/gtfs-realtime/reference#message-vehicleposition)(https://developers.google.com/transit/gtfs-realtime/reference#message-tripupdate)",
            "rdfs:isDefinedBy": {
                "@id": "https://voc.iudx.org.in/"
            },
            "rdfs:label": "trip",
            "skos:exactMatch": {
                "@id": "http://vocab.gtfs.org/gtfs.ttl#trip"
            }
        },
        {
            "@id": "https://voc.iudx.org.in/tripDetails",
            "@type": [
                "iudx:StructuredProperty"
            ],
            "iudx:domainIncludes": [
                {
                    "@id": "iudx:TransitManagement"
                }
            ],
            "iudx:rangeIncludes": [
                {
                    "@id": "iudx:TripDetails"
                }
            ],
            "rdfs:comment": "A descriptor of realtime update on the schedule of a vehicle along a trip.",
            "rdfs:isDefinedBy": {
                "@id": "https://voc.iudx.org.in/"
            },
            "rdfs:label": "tripDetails"
        },
        {
            "@id": "https://voc.iudx.org.in/tripDirection",
            "@type": [
                "iudx:TextProperty"
            ],
            "iudx:domainIncludes": [
                {
                    "@id": "iudx:TransitManagement"
                }
            ],
            "iudx:rangeIncludes": [
                {
                    "@id": "iudx:Text"
                },
                {
                    "@id": "iudx:ValueDescriptor"
                }
            ],
            "rdfs:comment": "Gives the direction in which the vehicle is travelling in ENUM[UP,DN]",
            "rdfs:isDefinedBy": {
                "@id": "https://voc.iudx.org.in/"
            },
            "rdfs:label": "tripDirection"
        },
        {
            "@id": "https://voc.iudx.org.in/trip_delay",
            "@type": [
                "iudx:QuantitativeProperty"
            ],
            "iudx:domainIncludes": [
                {
                    "@id": "iudx:TransitManagement"
                }
            ],
            "iudx:rangeIncludes": [
                {
                    "@id": "iudx:Number"
                },
                {
                    "@id": "iudx:ValueDescriptor"
                }
            ],
            "rdfs:comment": "This can be positive and negative in seconds and shows how much the vehicle deviates from the planned one. SameAs: 'delay' field from GTFS Realtime message-StopTimeEvent (https://developers.google.com/transit/gtfs-realtime/reference#message-stoptimeevent)",
            "rdfs:isDefinedBy": {
                "@id": "https://voc.iudx.org.in/"
            },
            "rdfs:label": "trip_delay",
            "skos:exactMatch": {
                "@id": "http://vocab.gtfs.org/gtfs.ttl#delay"
            }
        },
        {
            "@id": "https://voc.iudx.org.in/trip_details",
            "@type": [
                "iudx:StructuredProperty"
            ],
            "iudx:domainIncludes": [
                {
                    "@id": "iudx:TransitManagement"
                }
            ],
            "iudx:rangeIncludes": [
                {
                    "@id": "iudx:TripDetails"
                }
            ],
            "rdfs:comment": "A descriptor of realtime update on the schedule of a vehicle along a trip.",
            "rdfs:isDefinedBy": {
                "@id": "https://voc.iudx.org.in/"
            },
            "rdfs:label": "trip_details"
        },
        {
            "@id": "https://voc.iudx.org.in/trip_direction",
            "@type": [
                "iudx:TextProperty"
            ],
            "iudx:domainIncludes": [
                {
                    "@id": "iudx:TransitManagement"
                }
            ],
            "iudx:rangeIncludes": [
                {
                    "@id": "iudx:Text"
                },
                {
                    "@id": "iudx:ValueDescriptor"
                }
            ],
            "rdfs:comment": "Gives the direction in which the vehicle is travelling. SameAs: 'direction_id' field from GTFS Realtime message-TripDescriptor but is represented in the form of an ENUM[UP,DN] in place of [0,1] as seen in 'direction_id' (https://developers.google.com/transit/gtfs-realtime/reference#message-tripdescriptor).",
            "rdfs:isDefinedBy": {
                "@id": "https://voc.iudx.org.in/"
            },
            "rdfs:label": "trip_direction",
            "skos:exactMatch": {
                "@id": "http://vocab.gtfs.org/gtfs.ttl#direction_id"
            }
        },
        {
            "@id": "https://voc.iudx.org.in/trip_id",
            "@type": [
                "iudx:TextProperty"
            ],
            "iudx:domainIncludes": [
                {
                    "@id": "iudx:TransitManagement"
                },
                {
                    "@id": "iudx:TripDescriptor"
                },
                {
                    "@id": "iudx:FareCollectionSystem"
                }
            ],
            "iudx:rangeIncludes": [
                {
                    "@id": "iudx:Text"
                },
                {
                    "@id": "iudx:ValueDescriptor"
                }
            ],
            "rdfs:comment": "Trip ID/Trip name alloted to the bus corresponding to this observation, in consideration to the time of the day and the direction of the trip on the given routeId. SameAs: 'trip_id' field from GTFS Realtime message-TripDescriptor (https://developers.google.com/transit/gtfs-realtime/reference#message-tripdescriptor)",
            "rdfs:isDefinedBy": {
                "@id": "https://voc.iudx.org.in/"
            },
            "rdfs:label": "trip_id"
        },
        {
            "@id": "https://voc.iudx.org.in/trip_update",
            "@type": [
                "iudx:StructuredProperty"
            ],
            "iudx:domainIncludes": [
                {
                    "@id": "iudx:TransitManagement"
                },
                {
                    "@id": "iudx:FeedEntity"
                }
            ],
            "iudx:rangeIncludes": [
                {
                    "@id": "iudx:TripUpdate"
                }
            ],
            "rdfs:comment": "Describes the trip information like delay, departures, etc., for a trip made by the vehicle corresponding to this observation.SameAs:'trip_update' field from GTFS Realtime message-FeedEntity(https://developers.google.com/transit/gtfs-realtime/reference#message-feedentity)",
            "rdfs:isDefinedBy": {
                "@id": "https://voc.iudx.org.in/"
            },
            "rdfs:label": "trip_update"
        },
        {
            "@id": "https://voc.iudx.org.in/uncertainity",
            "@type": [
                "iudx:QuantitativeProperty"
            ],
            "iudx:domainIncludes": [
                {
                    "@id": "iudx:TransitManagement"
                },
                {
                    "@id": "iudx:StopTimeEvent"
                }
            ],
            "iudx:rangeIncludes": [
                {
                    "@id": "iudx:Number"
                },
                {
                    "@id": "iudx:ValueDescriptor"
                }
            ],
            "rdfs:comment": "If uncertainty is omitted, it is interpreted as unknown. To specify a completely certain prediction, set its uncertainty to 0.SameAs: 'uncertainity' field from GTFS Realtime message-StopTimeEvent (https://developers.google.com/transit/gtfs-realtime/reference#message-stoptimeevent)",
            "rdfs:isDefinedBy": {
                "@id": "https://voc.iudx.org.in/"
            },
            "rdfs:label": "uncertainity"
        },
        {
            "@id": "https://voc.iudx.org.in/vehicleDesc",
            "@type": [
                "iudx:StructuredProperty"
            ],
            "iudx:domainIncludes": [
                {
                    "@id": "iudx:TransitManagement"
                },
                {
                    "@id": "iudx:VehiclePosition"
                },
                {
                    "@id": "iudx:TripUpdate"
                }
            ],
            "iudx:rangeIncludes": [
                {
                    "@id": "iudx:VehicleDescriptor"
                }
            ],
            "rdfs:comment": "Describes the additional information of the vehicle corresponding to this observation. SameAs:'vehicle' field from GTFS Realtime message-VehiclePosition(https://developers.google.com/transit/gtfs-realtime/reference#message-vehicleposition)/(https://developers.google.com/transit/gtfs-realtime/reference#message-tripupdate)",
            "rdfs:isDefinedBy": {
                "@id": "https://voc.iudx.org.in/"
            },
            "rdfs:label": "vehicleDesc",
            "skos:exactMatch": {
                "@id": "http://vocab.gtfs.org/gtfs.ttl#vehicle"
            }
        },
        {
            "@id": "https://voc.iudx.org.in/vehicle_id",
            "@type": [
                "iudx:TextProperty"
            ],
            "iudx:domainIncludes": [
                {
                    "@id": "iudx:TransitManagement"
                },
                {
                    "@id": "iudx:VehicleDescriptor"
                }
            ],
            "iudx:rangeIncludes": [
                {
                    "@id": "iudx:Text"
                },
                {
                    "@id": "iudx:ValueDescriptor"
                }
            ],
            "rdfs:comment": "Unique ID assigned to the vehicle corresponding to this observation, used in internal system identification. SameAs: 'id' field from GTFS Realtime message-VehicleDescriptor (https://developers.google.com/transit/gtfs-realtime/reference#message-vehicledescriptor)",
            "rdfs:isDefinedBy": {
                "@id": "https://voc.iudx.org.in/"
            },
            "rdfs:label": "vehicle_id"
        },
        {
            "@id": "https://voc.iudx.org.in/vehicle_label",
            "@type": [
                "iudx:TextProperty"
            ],
            "iudx:domainIncludes": [
                {
                    "@id": "iudx:TransitManagement"
                },
                {
                    "@id": "iudx:VehicleDescriptor"
                },
                {
                    "@id": "iudx:FareCollectionSystem"
                }
            ],
            "iudx:rangeIncludes": [
                {
                    "@id": "iudx:Text"
                },
                {
                    "@id": "iudx:ValueDescriptor"
                }
            ],
            "rdfs:comment": "User visible label, i.e., something that must be shown to the passenger to help identify the correct vehicle. SameAs: 'label' field from GTFS Realtime message-VehicleDescriptor (https://developers.google.com/transit/gtfs-realtime/reference#message-vehicledescriptor)",
            "rdfs:isDefinedBy": {
                "@id": "https://voc.iudx.org.in/"
            },
            "rdfs:label": "vehicle_label"
        },
        {
            "@id": "https://voc.iudx.org.in/vehicle_position",
            "@type": [
                "iudx:StructuredProperty"
            ],
            "iudx:domainIncludes": [
                {
                    "@id": "iudx:TransitManagement"
                },
                {
                    "@id": "iudx:FeedEntity"
                }
            ],
            "iudx:rangeIncludes": [
                {
                    "@id": "iudx:VehiclePosition"
                }
            ],
            "rdfs:comment": "Describes the realtime position of the vehicle corresponding to this observation. SameAs:'vehicle' field from GTFS Realtime message-FeedEntity(https://developers.google.com/transit/gtfs-realtime/reference#message-feedentity)",
            "rdfs:isDefinedBy": {
                "@id": "https://voc.iudx.org.in/"
            },
            "rdfs:label": "vehicle_position"
        },
        {
            "@id": "https://voc.iudx.org.in/cityID",
            "@type": [
                "iudx:TextProperty"
            ],
            "iudx:domainIncludes": [
                {
                    "@id": "iudx:MunicipalityDesc"
                }
            ],
            "iudx:rangeIncludes": [
                {
                    "@id": "iudx:Text"
                },
                {
                    "@id": "iudx:ValueDescriptor"
                }
            ],
            "rdfs:comment": "City ID corresponding to this observation.",
            "rdfs:isDefinedBy": {
                "@id": "https://voc.iudx.org.in/"
            },
            "rdfs:label": "cityID"
        },
        {
            "@id": "https://voc.iudx.org.in/cityName",
            "@type": [
                "iudx:TextProperty"
            ],
            "iudx:domainIncludes": [
                {
                    "@id": "iudx:MunicipalityDesc"
                }
            ],
            "iudx:rangeIncludes": [
                {
                    "@id": "iudx:Text"
                },
                {
                    "@id": "iudx:ValueDescriptor"
                }
            ],
            "rdfs:comment": "City name corresponding to this observation.",
            "rdfs:isDefinedBy": {
                "@id": "https://voc.iudx.org.in/"
            },
            "rdfs:label": "cityName"
        },
        {
            "@id": "https://voc.iudx.org.in/district",
            "@type": [
                "iudx:TextProperty"
            ],
            "iudx:domainIncludes": [
                {
                    "@id": "iudx:MunicipalityDesc"
                }
            ],
            "iudx:rangeIncludes": [
                {
                    "@id": "iudx:Text"
                },
                {
                    "@id": "iudx:ValueDescriptor"
                }
            ],
            "rdfs:comment": "District name corresponding to this observation.",
            "rdfs:isDefinedBy": {
                "@id": "https://voc.iudx.org.in/"
            },
            "rdfs:label": "district"
        },
        {
            "@id": "https://voc.iudx.org.in/stateName",
            "@type": [
                "iudx:TextProperty"
            ],
            "iudx:domainIncludes": [
                {
                    "@id": "iudx:MunicipalityDesc"
                }
            ],
            "iudx:rangeIncludes": [
                {
                    "@id": "iudx:Text"
                },
                {
                    "@id": "iudx:ValueDescriptor"
                }
            ],
            "rdfs:comment": "Name of the state corresponding to this observation.",
            "rdfs:isDefinedBy": {
                "@id": "https://voc.iudx.org.in/"
            },
            "rdfs:label": "stateName"
        },
        {
            "@id": "https://voc.iudx.org.in/ulbName",
            "@type": [
                "iudx:TextProperty"
            ],
            "iudx:domainIncludes": [
                {
                    "@id": "iudx:MunicipalityDesc"
                }
            ],
            "iudx:rangeIncludes": [
                {
                    "@id": "iudx:Text"
                },
                {
                    "@id": "iudx:ValueDescriptor"
                }
            ],
            "rdfs:comment": "Name of the Urban Local Body corresponding to this observation.",
            "rdfs:isDefinedBy": {
                "@id": "https://voc.iudx.org.in/"
            },
            "rdfs:label": "ulbName"
        },
        {
            "@id": "https://voc.iudx.org.in/wardID",
            "@type": [
                "iudx:TextProperty"
            ],
            "iudx:domainIncludes": [
                {
                    "@id": "iudx:MunicipalityDesc"
                }
            ],
            "iudx:rangeIncludes": [
                {
                    "@id": "iudx:Text"
                },
                {
                    "@id": "iudx:ValueDescriptor"
                }
            ],
            "rdfs:comment": "Ward ID corresponding to this observation.",
            "rdfs:isDefinedBy": {
                "@id": "https://voc.iudx.org.in/"
            },
            "rdfs:label": "wardID"
        },
        {
            "@id": "https://voc.iudx.org.in/wardName",
            "@type": [
                "iudx:TextProperty"
            ],
            "iudx:domainIncludes": [
                {
                    "@id": "iudx:MunicipalityDesc"
                }
            ],
            "iudx:rangeIncludes": [
                {
                    "@id": "iudx:Text"
                },
                {
                    "@id": "iudx:ValueDescriptor"
                }
            ],
            "rdfs:comment": "Ward name corresponding to this observation.",
            "rdfs:isDefinedBy": {
                "@id": "https://voc.iudx.org.in/"
            },
            "rdfs:label": "wardName"
        },
        {
            "@id": "https://voc.iudx.org.in/wardNum",
            "@type": [
                "iudx:QuantitativeProperty"
            ],
            "iudx:domainIncludes": [
                {
                    "@id": "iudx:MunicipalityDesc"
                }
            ],
            "iudx:rangeIncludes": [
                {
                    "@id": "iudx:Number"
                },
                {
                    "@id": "iudx:ValueDescriptor"
                }
            ],
            "rdfs:comment": "Ward number corresponding to this observation.",
            "rdfs:isDefinedBy": {
                "@id": "https://voc.iudx.org.in/"
            },
            "rdfs:label": "wardNum"
        },
        {
            "@id": "https://voc.iudx.org.in/zoneID",
            "@type": [
                "iudx:TextProperty"
            ],
            "iudx:domainIncludes": [
                {
                    "@id": "iudx:MunicipalityDesc"
                }
            ],
            "iudx:rangeIncludes": [
                {
                    "@id": "iudx:Text"
                },
                {
                    "@id": "iudx:ValueDescriptor"
                }
            ],
            "rdfs:comment": "Zone ID corresponding to this observation.",
            "rdfs:isDefinedBy": {
                "@id": "https://voc.iudx.org.in/"
            },
            "rdfs:label": "zoneID"
        },
        {
            "@id": "https://voc.iudx.org.in/zoneName",
            "@type": [
                "iudx:TextProperty"
            ],
            "iudx:domainIncludes": [
                {
                    "@id": "iudx:MunicipalityDesc"
                }
            ],
            "iudx:rangeIncludes": [
                {
                    "@id": "iudx:Text"
                },
                {
                    "@id": "iudx:ValueDescriptor"
                }
            ],
            "rdfs:comment": "Zone name corresponding to this observation.",
            "rdfs:isDefinedBy": {
                "@id": "https://voc.iudx.org.in/"
            },
            "rdfs:label": "zoneName"
        },
        {
            "@id": "https://voc.iudx.org.in/annotatedMap",
            "@type": [
                "iudx:TextProperty"
            ],
            "iudx:domainIncludes": [
                {
                    "@id": "iudx:Orientation"
                }
            ],
            "iudx:rangeIncludes": [
                {
                    "@id": "iudx:Text"
                },
                {
                    "@id": "iudx:ValueDescriptor"
                }
            ],
            "rdfs:comment": "Annotated map view indicating the orientations for the camera corresponding to this observation",
            "rdfs:isDefinedBy": {
                "@id": "https://voc.iudx.org.in/"
            },
            "rdfs:label": "annotatedMap"
        },
        {
            "@id": "https://voc.iudx.org.in/activePower",
            "@type": [
                "iudx:QuantitativeProperty"
            ],
            "iudx:domainIncludes": [
                {
                    "@id": "iudx:StreetLightFeeder"
                }
            ],
            "iudx:rangeIncludes": [
                {
                    "@id": "iudx:NumericArray"
                },
                {
                    "@id": "iudx:ValueDescriptor"
                }
            ],
            "rdfs:comment": "Active power consumed per phase. Ordered triple comprising of active power from three phases in the following order: [R Y B]",
            "rdfs:isDefinedBy": {
                "@id": "https://voc.iudx.org.in/"
            },
            "rdfs:label": "activePower",
            "skos:exactMatch": {
                "@id": "https://uri.fiware.org/ns/data-models#activePower"
            }
        },
        {
            "@id": "https://voc.iudx.org.in/current",
            "@type": [
                "iudx:QuantitativeProperty"
            ],
            "iudx:domainIncludes": [
                {
                    "@id": "iudx:Streetlight"
                }
            ],
            "iudx:rangeIncludes": [
                {
                    "@id": "iudx:Number"
                },
                {
                    "@id": "iudx:ValueDescriptor"
                }
            ],
            "rdfs:comment": "Current value of the streetlight corresponding to this observation.",
            "rdfs:isDefinedBy": {
                "@id": "https://voc.iudx.org.in/"
            },
            "rdfs:label": "current"
        },
        {
            "@id": "https://voc.iudx.org.in/feederID",
            "@type": [
                "iudx:Relationship"
            ],
            "iudx:domainIncludes": [
                {
                    "@id": "iudx:Streetlight"
                }
            ],
            "iudx:rangeIncludes": [
                {
                    "@id": "iudx:Text"
                },
                {
                    "@id": "iudx:Text",
                    "@type": "@id"
                },
                {
                    "@id": "iudx:RelationshipValue"
                }
            ],
            "rdfs:comment": "Unique ID of the streetlight feeder panel associated with the streetlight corresponding to this observation.",
            "rdfs:isDefinedBy": {
                "@id": "https://voc.iudx.org.in/"
            },
            "rdfs:label": "feederID"
        },
        {
            "@id": "https://voc.iudx.org.in/feederPillarNum",
            "@type": [
                "iudx:TextProperty"
            ],
            "iudx:domainIncludes": [
                {
                    "@id": "iudx:Streetlight"
                }
            ],
            "iudx:rangeIncludes": [
                {
                    "@id": "iudx:Text"
                },
                {
                    "@id": "iudx:ValueDescriptor"
                }
            ],
            "rdfs:comment": "Streetlight feeder pillar information associated with the streetlight corresponding to this observation.",
            "rdfs:isDefinedBy": {
                "@id": "https://voc.iudx.org.in/"
            },
            "rdfs:label": "feederPillarNum"
        },
        {
            "@id": "https://voc.iudx.org.in/numStreetlight",
            "@type": [
                "iudx:QuantitativeProperty"
            ],
            "iudx:domainIncludes": [
                {
                    "@id": "iudx:StreetLightFeeder"
                }
            ],
            "iudx:rangeIncludes": [
                {
                    "@id": "iudx:Number"
                },
                {
                    "@id": "iudx:ValueDescriptor"
                }
            ],
            "rdfs:comment": "Describes the total number of streetlights connected to the feeder panel corresponding to this observation.",
            "rdfs:isDefinedBy": {
                "@id": "https://voc.iudx.org.in/"
            },
            "rdfs:label": "numStreetlight"
        },
        {
            "@id": "https://voc.iudx.org.in/phaseCurrent",
            "@type": [
                "iudx:QuantitativeProperty"
            ],
            "iudx:domainIncludes": [
                {
                    "@id": "iudx:StreetLightFeeder"
                }
            ],
            "iudx:rangeIncludes": [
                {
                    "@id": "iudx:NumericArray"
                },
                {
                    "@id": "iudx:ValueDescriptor"
                }
            ],
            "rdfs:comment": "Current per phase. Ordered triple comprising of active power from three phases in the following order: [R Y B]",
            "rdfs:isDefinedBy": {
                "@id": "https://voc.iudx.org.in/"
            },
            "rdfs:label": "phaseCurrent"
        },
        {
            "@id": "https://voc.iudx.org.in/phaseVoltage",
            "@type": [
                "iudx:QuantitativeProperty"
            ],
            "iudx:domainIncludes": [
                {
                    "@id": "iudx:StreetLightFeeder"
                }
            ],
            "iudx:rangeIncludes": [
                {
                    "@id": "iudx:NumericArray"
                },
                {
                    "@id": "iudx:ValueDescriptor"
                }
            ],
            "rdfs:comment": "Voltage per phase. Ordered triple comprising of active power from three phases in the following order: [R Y B]",
            "rdfs:isDefinedBy": {
                "@id": "https://voc.iudx.org.in/"
            },
            "rdfs:label": "phaseVoltage",
            "skos:exactMatch": {
                "@id": "https://uri.fiware.org/ns/data-models#voltage"
            }
        },
        {
            "@id": "https://voc.iudx.org.in/powerConsumption",
            "@type": [
                "iudx:QuantitativeProperty"
            ],
            "iudx:domainIncludes": [
                {
                    "@id": "iudx:Streetlight"
                }
            ],
            "iudx:rangeIncludes": [
                {
                    "@id": "iudx:Number"
                },
                {
                    "@id": "iudx:ValueDescriptor"
                }
            ],
            "rdfs:comment": "Power consumed by the LED or the streetlight bulb corresponding to this observation.",
            "rdfs:isDefinedBy": {
                "@id": "https://voc.iudx.org.in/"
            },
            "rdfs:label": "powerConsumption",
            "skos:exactMatch": {
                "@id": "https://uri.fiware.org/ns/data-models#powerConsumption"
            }
        },
        {
            "@id": "https://voc.iudx.org.in/powerFactor",
            "@type": [
                "iudx:QuantitativeProperty"
            ],
            "iudx:domainIncludes": [
                {
                    "@id": "iudx:Streetlight"
                }
            ],
            "iudx:rangeIncludes": [
                {
                    "@id": "iudx:Number"
                },
                {
                    "@id": "iudx:ValueDescriptor"
                }
            ],
            "rdfs:comment": "Power factor or the ratio of working power of the streetlight corresponding to this observation.",
            "rdfs:isDefinedBy": {
                "@id": "https://voc.iudx.org.in/"
            },
            "rdfs:label": "powerFactor",
            "skos:exactMatch": {
                "@id": "https://uri.fiware.org/ns/data-models#powerFactor"
            }
        },
        {
            "@id": "https://voc.iudx.org.in/powerRating",
            "@type": [
                "iudx:QuantitativeProperty"
            ],
            "iudx:domainIncludes": [
                {
                    "@id": "iudx:Streetlight"
                }
            ],
            "iudx:rangeIncludes": [
                {
                    "@id": "iudx:Number"
                },
                {
                    "@id": "iudx:ValueDescriptor"
                }
            ],
            "rdfs:comment": "Power rating of the LED or the streetlight bulb corresponding to this observation.",
            "rdfs:isDefinedBy": {
                "@id": "https://voc.iudx.org.in/"
            },
            "rdfs:label": "powerRating"
        },
        {
            "@id": "https://voc.iudx.org.in/powerState",
            "@type": [
                "iudx:TextProperty"
            ],
            "iudx:domainIncludes": [
                {
                    "@id": "iudx:StreetLightFeeder"
                },
                {
                    "@id": "iudx:Streetlight"
                }
            ],
            "iudx:rangeIncludes": [
                {
                    "@id": "iudx:Text"
                },
                {
                    "@id": "iudx:ValueDescriptor"
                }
            ],
            "rdfs:comment": "Indicates the current status of the streetlight feeder panel.",
            "rdfs:isDefinedBy": {
                "@id": "https://voc.iudx.org.in/"
            },
            "rdfs:label": "powerState",
            "skos:exactMatch": {
                "@id": "https://uri.fiware.org/ns/data-models#powerState"
            }
        },
        {
            "@id": "https://voc.iudx.org.in/reactivePower",
            "@type": [
                "iudx:QuantitativeProperty"
            ],
            "iudx:domainIncludes": [
                {
                    "@id": "iudx:StreetLightFeeder"
                }
            ],
            "iudx:rangeIncludes": [
                {
                    "@id": "iudx:NumericArray"
                },
                {
                    "@id": "iudx:ValueDescriptor"
                }
            ],
            "rdfs:comment": "Reactive power consumed per phase. Ordered triple comprising of active power from three phases in the following order: [R Y B]",
            "rdfs:isDefinedBy": {
                "@id": "https://voc.iudx.org.in/"
            },
            "rdfs:label": "reactivePower",
            "skos:exactMatch": {
                "@id": "https://uri.fiware.org/ns/data-models#reactivePower"
            }
        },
        {
            "@id": "https://voc.iudx.org.in/streetPoleNum",
            "@type": [
                "iudx:TextProperty"
            ],
            "iudx:domainIncludes": [
                {
                    "@id": "iudx:Streetlight"
                }
            ],
            "iudx:rangeIncludes": [
                {
                    "@id": "iudx:Text"
                },
                {
                    "@id": "iudx:ValueDescriptor"
                }
            ],
            "rdfs:comment": "Street pole information associated with the streetlight corresponding to this observation.",
            "rdfs:isDefinedBy": {
                "@id": "https://voc.iudx.org.in/"
            },
            "rdfs:label": "streetPoleNum"
        },
        {
            "@id": "https://voc.iudx.org.in/totalActivePower",
            "@type": [
                "iudx:QuantitativeProperty"
            ],
            "iudx:domainIncludes": [
                {
                    "@id": "iudx:StreetLightFeeder"
                }
            ],
            "iudx:rangeIncludes": [
                {
                    "@id": "iudx:Number"
                },
                {
                    "@id": "iudx:ValueDescriptor"
                }
            ],
            "rdfs:comment": "Total active power consumed by all phases",
            "rdfs:isDefinedBy": {
                "@id": "https://voc.iudx.org.in/"
            },
            "rdfs:label": "totalActivePower",
            "skos:exactMatch": {
                "@id": "https://uri.fiware.org/ns/data-models#totalActivePower"
            }
        },
        {
            "@id": "https://voc.iudx.org.in/totalReactivePower",
            "@type": [
                "iudx:QuantitativeProperty"
            ],
            "iudx:domainIncludes": [
                {
                    "@id": "iudx:StreetLightFeeder"
                }
            ],
            "iudx:rangeIncludes": [
                {
                    "@id": "iudx:Number"
                },
                {
                    "@id": "iudx:ValueDescriptor"
                }
            ],
            "rdfs:comment": "Total reactive power for all phases",
            "rdfs:isDefinedBy": {
                "@id": "https://voc.iudx.org.in/"
            },
            "rdfs:label": "totalReactivePower",
            "skos:exactMatch": {
                "@id": "https://uri.fiware.org/ns/data-models#totalReactivePower"
            }
        },
        {
            "@id": "https://voc.iudx.org.in/voltage",
            "@type": [
                "iudx:QuantitativeProperty"
            ],
            "iudx:domainIncludes": [
                {
                    "@id": "iudx:Streetlight"
                }
            ],
            "iudx:rangeIncludes": [
                {
                    "@id": "iudx:Number"
                },
                {
                    "@id": "iudx:ValueDescriptor"
                }
            ],
            "rdfs:comment": "Voltage value of the streetlight corresponding to this observation.",
            "rdfs:isDefinedBy": {
                "@id": "https://voc.iudx.org.in/"
            },
            "rdfs:label": "voltage"
        },
        {
            "@id": "https://voc.iudx.org.in/availableBikeNumber",
            "@type": [
                "iudx:QuantitativeProperty"
            ],
            "iudx:domainIncludes": [
                {
                    "@id": "iudx:BikeDockingStation"
                }
            ],
            "iudx:rangeIncludes": [
                {
                    "@id": "iudx:Number"
                },
                {
                    "@id": "iudx:ValueDescriptor"
                }
            ],
            "rdfs:comment": "The number of bikes available in the bike hire docking station to be hired by users.",
            "rdfs:isDefinedBy": {
                "@id": "https://voc.iudx.org.in/"
            },
            "rdfs:label": "availableBikeNumber",
            "skos:exactMatch": {
                "@id": "https://uri.fiware.org/ns/data-models#availableBikeNumber"
            }
        },
        {
            "@id": "https://voc.iudx.org.in/cardID",
            "@type": [
                "iudx:TextProperty"
            ],
            "iudx:domainIncludes": [
                {
                    "@id": "iudx:FareCollectionSystem"
                }
            ],
            "iudx:rangeIncludes": [
                {
                    "@id": "iudx:Text"
                },
                {
                    "@id": "iudx:ValueDescriptor"
                }
            ],
            "rdfs:comment": "Unique ticket ID of the transaction or ID of the smart card used in the transaction.",
            "rdfs:isDefinedBy": {
                "@id": "https://voc.iudx.org.in/"
            },
            "rdfs:label": "cardID"
        },
        {
            "@id": "https://voc.iudx.org.in/currentTripCount",
            "@type": [
                "iudx:QuantitativeProperty"
            ],
            "iudx:domainIncludes": [
                {
                    "@id": "iudx:FareCollectionSystem"
                },
                {
                    "@id": "iudx:WmgmtVehicle"
                }
            ],
            "iudx:rangeIncludes": [
                {
                    "@id": "iudx:Number"
                },
                {
                    "@id": "iudx:ValueDescriptor"
                }
            ],
            "rdfs:comment": "The current count of trips made by the vehicle corresponding to this obersvation on the given day of operation.",
            "rdfs:isDefinedBy": {
                "@id": "https://voc.iudx.org.in/"
            },
            "rdfs:label": "currentTripCount"
        },
        {
            "@id": "https://voc.iudx.org.in/destinationStopCategory",
            "@type": [
                "iudx:TextProperty"
            ],
            "iudx:domainIncludes": [
                {
                    "@id": "iudx:FareCollectionSystem"
                }
            ],
            "iudx:rangeIncludes": [
                {
                    "@id": "iudx:Text"
                },
                {
                    "@id": "iudx:ValueDescriptor"
                }
            ],
            "rdfs:comment": "Type of the destination bus stop corresponding to this observation.",
            "rdfs:isDefinedBy": {
                "@id": "https://voc.iudx.org.in/"
            },
            "rdfs:label": "destinationStopCategory"
        },
        {
            "@id": "https://voc.iudx.org.in/destinationStopID",
            "@type": [
                "iudx:TextProperty"
            ],
            "iudx:domainIncludes": [
                {
                    "@id": "iudx:FareCollectionSystem"
                }
            ],
            "iudx:rangeIncludes": [
                {
                    "@id": "iudx:Text"
                },
                {
                    "@id": "iudx:ValueDescriptor"
                }
            ],
            "rdfs:comment": "Unique ID of the bus stop at which the passenger deboards from the bus corresponding to this observation.",
            "rdfs:isDefinedBy": {
                "@id": "https://voc.iudx.org.in/"
            },
            "rdfs:label": "destinationStopID"
        },
        {
            "@id": "https://voc.iudx.org.in/destinationStopName",
            "@type": [
                "iudx:TextProperty"
            ],
            "iudx:domainIncludes": [
                {
                    "@id": "iudx:FareCollectionSystem"
                }
            ],
            "iudx:rangeIncludes": [
                {
                    "@id": "iudx:Text"
                },
                {
                    "@id": "iudx:ValueDescriptor"
                }
            ],
            "rdfs:comment": "The name of the destination bus stop corresponding to this observation.",
            "rdfs:isDefinedBy": {
                "@id": "https://voc.iudx.org.in/"
            },
            "rdfs:label": "destinationStopName"
        },
        {
            "@id": "https://voc.iudx.org.in/entryAreaCode",
            "@type": [
                "iudx:TextProperty"
            ],
            "iudx:domainIncludes": [
                {
                    "@id": "iudx:FareCollectionSystem"
                }
            ],
            "iudx:rangeIncludes": [
                {
                    "@id": "iudx:Text"
                },
                {
                    "@id": "iudx:ValueDescriptor"
                }
            ],
            "rdfs:comment": "Area code of the passenger boarding stop (used by the fare collection agency). For example, whether the stop is city-bus-service stop or brts stop or other service type stop etc.",
            "rdfs:isDefinedBy": {
                "@id": "https://voc.iudx.org.in/"
            },
            "rdfs:label": "entryAreaCode"
        },
        {
            "@id": "https://voc.iudx.org.in/equipmentCompanyCode",
            "@type": [
                "iudx:TextProperty"
            ],
            "iudx:domainIncludes": [
                {
                    "@id": "iudx:FareCollectionSystem"
                }
            ],
            "iudx:rangeIncludes": [
                {
                    "@id": "iudx:Text"
                },
                {
                    "@id": "iudx:ValueDescriptor"
                }
            ],
            "rdfs:comment": "Company/Agency code for the transaction equipment (used by fare collection agency). For example, 103 - CBS (city bus service),102 -  BRTS etc.",
            "rdfs:isDefinedBy": {
                "@id": "https://voc.iudx.org.in/"
            },
            "rdfs:label": "equipmentCompanyCode"
        },
        {
            "@id": "https://voc.iudx.org.in/equipmentID",
            "@type": [
                "iudx:TextProperty"
            ],
            "iudx:domainIncludes": [
                {
                    "@id": "iudx:FareCollectionSystem"
                },
                {
                    "@id": "iudx:TrafficViolations"
                }
            ],
            "iudx:rangeIncludes": [
                {
                    "@id": "iudx:Text"
                },
                {
                    "@id": "iudx:ValueDescriptor"
                }
            ],
            "rdfs:comment": "Unique ID of the equipment corresponding to this observation.",
            "rdfs:isDefinedBy": {
                "@id": "https://voc.iudx.org.in/"
            },
            "rdfs:label": "equipmentID"
        },
        {
            "@id": "https://voc.iudx.org.in/equipmentSequenceNumber",
            "@type": [
                "iudx:QuantitativeProperty"
            ],
            "iudx:domainIncludes": [
                {
                    "@id": "iudx:FareCollectionSystem"
                }
            ],
            "iudx:rangeIncludes": [
                {
                    "@id": "iudx:Number"
                },
                {
                    "@id": "iudx:ValueDescriptor"
                }
            ],
            "rdfs:comment": "Sequence number for the given equipment.",
            "rdfs:isDefinedBy": {
                "@id": "https://voc.iudx.org.in/"
            },
            "rdfs:label": "equipmentSequenceNumber"
        },
        {
            "@id": "https://voc.iudx.org.in/equipmentStopID",
            "@type": [
                "iudx:TextProperty"
            ],
            "iudx:domainIncludes": [
                {
                    "@id": "iudx:FareCollectionSystem"
                }
            ],
            "iudx:rangeIncludes": [
                {
                    "@id": "iudx:Text"
                },
                {
                    "@id": "iudx:ValueDescriptor"
                }
            ],
            "rdfs:comment": "Stop ID (BRTS) at which the equipment corresponding to this transaction is installed.",
            "rdfs:isDefinedBy": {
                "@id": "https://voc.iudx.org.in/"
            },
            "rdfs:label": "equipmentStopID"
        },
        {
            "@id": "https://voc.iudx.org.in/equipmentType",
            "@type": [
                "iudx:TextProperty"
            ],
            "iudx:domainIncludes": [
                {
                    "@id": "iudx:FareCollectionSystem"
                },
                {
                    "@id": "iudx:TrafficViolations"
                }
            ],
            "iudx:rangeIncludes": [
                {
                    "@id": "iudx:Text"
                },
                {
                    "@id": "iudx:ValueDescriptor"
                }
            ],
            "rdfs:comment": "Type of equipment or the name of the equipment corresponding to this observation.",
            "rdfs:isDefinedBy": {
                "@id": "https://voc.iudx.org.in/"
            },
            "rdfs:label": "equipmentType"
        },
        {
            "@id": "https://voc.iudx.org.in/equipmentTypeCode",
            "@type": [
                "iudx:TextProperty"
            ],
            "iudx:domainIncludes": [
                {
                    "@id": "iudx:FareCollectionSystem"
                }
            ],
            "iudx:rangeIncludes": [
                {
                    "@id": "iudx:Text"
                },
                {
                    "@id": "iudx:ValueDescriptor"
                }
            ],
            "rdfs:comment": "Unique code indicating the type of equipment used in the transaction (used by fare collection agency).ENUM [1B, 42, 02, 08, 41]\n1B - POS, 42 - HTT, 02- Mobile, 08- Fare Gate, 41- Pole Validator",
            "rdfs:isDefinedBy": {
                "@id": "https://voc.iudx.org.in/"
            },
            "rdfs:label": "equipmentTypeCode"
        },
        {
            "@id": "https://voc.iudx.org.in/exitAreaCode",
            "@type": [
                "iudx:TextProperty"
            ],
            "iudx:domainIncludes": [
                {
                    "@id": "iudx:FareCollectionSystem"
                }
            ],
            "iudx:rangeIncludes": [
                {
                    "@id": "iudx:Text"
                },
                {
                    "@id": "iudx:ValueDescriptor"
                }
            ],
            "rdfs:comment": "Area code of the passenger alighting stop (used by the fare collection agency). For example, whether the stop is city-bus-service stop or brts stop or other service type stop etc.",
            "rdfs:isDefinedBy": {
                "@id": "https://voc.iudx.org.in/"
            },
            "rdfs:label": "exitAreaCode"
        },
        {
            "@id": "https://voc.iudx.org.in/fareForAdult",
            "@type": [
                "iudx:QuantitativeProperty"
            ],
            "iudx:domainIncludes": [
                {
                    "@id": "iudx:FareCollectionSystem"
                }
            ],
            "iudx:rangeIncludes": [
                {
                    "@id": "iudx:Number"
                },
                {
                    "@id": "iudx:ValueDescriptor"
                }
            ],
            "rdfs:comment": "The fare for an adult in the journey corresponding to this observation.",
            "rdfs:isDefinedBy": {
                "@id": "https://voc.iudx.org.in/"
            },
            "rdfs:label": "fareForAdult"
        },
        {
            "@id": "https://voc.iudx.org.in/fareForChild",
            "@type": [
                "iudx:QuantitativeProperty"
            ],
            "iudx:domainIncludes": [
                {
                    "@id": "iudx:FareCollectionSystem"
                }
            ],
            "iudx:rangeIncludes": [
                {
                    "@id": "iudx:Number"
                },
                {
                    "@id": "iudx:ValueDescriptor"
                }
            ],
            "rdfs:comment": "The fare for a child in the journey corresponding to this observation.",
            "rdfs:isDefinedBy": {
                "@id": "https://voc.iudx.org.in/"
            },
            "rdfs:label": "fareForChild"
        },
        {
            "@id": "https://voc.iudx.org.in/freeSlotNumber",
            "@type": [
                "iudx:QuantitativeProperty"
            ],
            "iudx:domainIncludes": [
                {
                    "@id": "iudx:BikeDockingStation"
                }
            ],
            "iudx:rangeIncludes": [
                {
                    "@id": "iudx:Number"
                },
                {
                    "@id": "iudx:ValueDescriptor"
                }
            ],
            "rdfs:comment": "The number of bike racks or docking slots available for returning and parking bikes in the bike docking station corresponding to this observation.",
            "rdfs:isDefinedBy": {
                "@id": "https://voc.iudx.org.in/"
            },
            "rdfs:label": "freeSlotNumber",
            "skos:exactMatch": {
                "@id": "https://uri.fiware.org/ns/data-models#freeSlotNumber"
            }
        },
        {
            "@id": "https://voc.iudx.org.in/occupancyLevel",
            "@type": [
                "iudx:TextProperty"
            ],
            "iudx:domainIncludes": [
                {
                    "@id": "iudx:FareCollectionSystem"
                }
            ],
            "iudx:rangeIncludes": [
                {
                    "@id": "iudx:Text"
                },
                {
                    "@id": "iudx:ValueDescriptor"
                }
            ],
            "rdfs:comment": "Occupancy level in the public transit bus corresponding to this observation. 'Red' indicates the congestion level in the bus is HIGH, 'Yellow' indicates the congestion level in the bus is MODERATE and 'Green' indicates the congestion level in the bus is LOW.",
            "rdfs:isDefinedBy": {
                "@id": "https://voc.iudx.org.in/"
            },
            "rdfs:label": "occupancyLevel"
        },
        {
            "@id": "https://voc.iudx.org.in/originDestinationCode",
            "@type": [
                "iudx:TextProperty"
            ],
            "iudx:domainIncludes": [
                {
                    "@id": "iudx:FareCollectionSystem"
                }
            ],
            "iudx:rangeIncludes": [
                {
                    "@id": "iudx:Text"
                },
                {
                    "@id": "iudx:ValueDescriptor"
                }
            ],
            "rdfs:comment": "The code for the orgin and destination stops corresponding to this observation.",
            "rdfs:isDefinedBy": {
                "@id": "https://voc.iudx.org.in/"
            },
            "rdfs:label": "originDestinationCode"
        },
        {
            "@id": "https://voc.iudx.org.in/originStopCategory",
            "@type": [
                "iudx:TextProperty"
            ],
            "iudx:domainIncludes": [
                {
                    "@id": "iudx:FareCollectionSystem"
                }
            ],
            "iudx:rangeIncludes": [
                {
                    "@id": "iudx:Text"
                },
                {
                    "@id": "iudx:ValueDescriptor"
                }
            ],
            "rdfs:comment": "Type of the origin bus stop corresponding to this observation.",
            "rdfs:isDefinedBy": {
                "@id": "https://voc.iudx.org.in/"
            },
            "rdfs:label": "originStopCategory"
        },
        {
            "@id": "https://voc.iudx.org.in/originStopID",
            "@type": [
                "iudx:TextProperty"
            ],
            "iudx:domainIncludes": [
                {
                    "@id": "iudx:FareCollectionSystem"
                }
            ],
            "iudx:rangeIncludes": [
                {
                    "@id": "iudx:Text"
                },
                {
                    "@id": "iudx:ValueDescriptor"
                }
            ],
            "rdfs:comment": "Unique ID of the bus stop at which the passenger boards into the bus corresponding to this observation.",
            "rdfs:isDefinedBy": {
                "@id": "https://voc.iudx.org.in/"
            },
            "rdfs:label": "originStopID"
        },
        {
            "@id": "https://voc.iudx.org.in/originStopName",
            "@type": [
                "iudx:TextProperty"
            ],
            "iudx:domainIncludes": [
                {
                    "@id": "iudx:FareCollectionSystem"
                }
            ],
            "iudx:rangeIncludes": [
                {
                    "@id": "iudx:Text"
                },
                {
                    "@id": "iudx:ValueDescriptor"
                }
            ],
            "rdfs:comment": "The name of the origin bus stop corresponding to this observation.",
            "rdfs:isDefinedBy": {
                "@id": "https://voc.iudx.org.in/"
            },
            "rdfs:label": "originStopName"
        },
        {
            "@id": "https://voc.iudx.org.in/outOfServiceSlotNumber",
            "@type": [
                "iudx:QuantitativeProperty"
            ],
            "iudx:domainIncludes": [
                {
                    "@id": "iudx:BikeDockingStation"
                }
            ],
            "iudx:rangeIncludes": [
                {
                    "@id": "iudx:Number"
                },
                {
                    "@id": "iudx:ValueDescriptor"
                }
            ],
            "rdfs:comment": "The number of bike racks or docking slots that are out of order and cannot be used to hire or park a bike in the bike docking station corresponding to this observation.",
            "rdfs:isDefinedBy": {
                "@id": "https://voc.iudx.org.in/"
            },
            "rdfs:label": "outOfServiceSlotNumber",
            "skos:exactMatch": {
                "@id": "https://uri.fiware.org/ns/data-models#outOfServiceSlotNumber"
            }
        },
        {
            "@id": "https://voc.iudx.org.in/passengerCount",
            "@type": [
                "iudx:QuantitativeProperty"
            ],
            "iudx:domainIncludes": [
                {
                    "@id": "iudx:FareCollectionSystem"
                }
            ],
            "iudx:rangeIncludes": [
                {
                    "@id": "iudx:Number"
                },
                {
                    "@id": "iudx:ValueDescriptor"
                }
            ],
            "rdfs:comment": "Number of passengers travelling in the public transit bus corresponding to this observation. This count is computed based on the realtime ticketing transactions in the public transit bus.",
            "rdfs:isDefinedBy": {
                "@id": "https://voc.iudx.org.in/"
            },
            "rdfs:label": "passengerCount"
        },
        {
            "@id": "https://voc.iudx.org.in/paymentStatus",
            "@type": [
                "iudx:TextProperty"
            ],
            "iudx:domainIncludes": [
                {
                    "@id": "iudx:TrafficViolations"
                }
            ],
            "iudx:rangeIncludes": [
                {
                    "@id": "iudx:Text"
                },
                {
                    "@id": "iudx:ValueDescriptor"
                }
            ],
            "rdfs:comment": "The payment status of the fine or violation or challan corresponding to this observation. ENUM[\"Paid\", \"Unpaid\"].",
            "rdfs:isDefinedBy": {
                "@id": "https://voc.iudx.org.in/"
            },
            "rdfs:label": "paymentStatus"
        },
        {
            "@id": "https://voc.iudx.org.in/shiftOfOperation",
            "@type": [
                "iudx:TextProperty"
            ],
            "iudx:domainIncludes": [
                {
                    "@id": "iudx:FareCollectionSystem"
                },
                {
                    "@id": "iudx:EmployeeDetails"
                }
            ],
            "iudx:rangeIncludes": [
                {
                    "@id": "iudx:Text"
                },
                {
                    "@id": "iudx:ValueDescriptor"
                }
            ],
            "rdfs:comment": "Shift of operation of the public transit vehicle operated by the fare collection agency/ public transit agency or the employee corresponding to this observation. Indiacted as '1' when the vehicle operates in the first shift, '2' when the vehicle operates in the second shift and '3' when the vehilce operates in the third shift.",
            "rdfs:isDefinedBy": {
                "@id": "https://voc.iudx.org.in/"
            },
            "rdfs:label": "shiftOfOperation"
        },
        {
            "@id": "https://voc.iudx.org.in/stage",
            "@type": [
                "iudx:QuantitativeProperty"
            ],
            "iudx:domainIncludes": [
                {
                    "@id": "iudx:FareCollectionSystem"
                }
            ],
            "iudx:rangeIncludes": [
                {
                    "@id": "iudx:Number"
                },
                {
                    "@id": "iudx:ValueDescriptor"
                }
            ],
            "rdfs:comment": "Total number of stages from the origin bus stop to the destination bus stop.",
            "rdfs:isDefinedBy": {
                "@id": "https://voc.iudx.org.in/"
            },
            "rdfs:label": "stage"
        },
        {
            "@id": "https://voc.iudx.org.in/stationCode",
            "@type": [
                "iudx:TextProperty"
            ],
            "iudx:domainIncludes": [
                {
                    "@id": "iudx:BikeDockingStation"
                }
            ],
            "iudx:rangeIncludes": [
                {
                    "@id": "iudx:Text"
                },
                {
                    "@id": "iudx:ValueDescriptor"
                }
            ],
            "rdfs:comment": "The station number or station code of the bike hire docking station corresponding to the observation.",
            "rdfs:isDefinedBy": {
                "@id": "https://voc.iudx.org.in/"
            },
            "rdfs:label": "stationCode"
        },
        {
            "@id": "https://voc.iudx.org.in/stationName",
            "@type": [
                "iudx:TextProperty"
            ],
            "iudx:domainIncludes": [
                {
                    "@id": "iudx:BikeDockingStation"
                }
            ],
            "iudx:rangeIncludes": [
                {
                    "@id": "iudx:Text"
                },
                {
                    "@id": "iudx:ValueDescriptor"
                }
            ],
            "rdfs:comment": "The name of the bike hire docking station corresponding to this observation.",
            "rdfs:isDefinedBy": {
                "@id": "https://voc.iudx.org.in/"
            },
            "rdfs:label": "stationName"
        },
        {
            "@id": "https://voc.iudx.org.in/ticketTypeCode",
            "@type": [
                "iudx:TextProperty"
            ],
            "iudx:domainIncludes": [
                {
                    "@id": "iudx:FareCollectionSystem"
                }
            ],
            "iudx:rangeIncludes": [
                {
                    "@id": "iudx:Text"
                },
                {
                    "@id": "iudx:ValueDescriptor"
                }
            ],
            "rdfs:comment": "Unique ticket type code of the corresponding trip.",
            "rdfs:isDefinedBy": {
                "@id": "https://voc.iudx.org.in/"
            },
            "rdfs:label": "ticketTypeCode"
        },
        {
            "@id": "https://voc.iudx.org.in/totalSlotNumber",
            "@type": [
                "iudx:QuantitativeProperty"
            ],
            "iudx:domainIncludes": [
                {
                    "@id": "iudx:BikeDockingStation"
                }
            ],
            "iudx:rangeIncludes": [
                {
                    "@id": "iudx:Number"
                },
                {
                    "@id": "iudx:ValueDescriptor"
                }
            ],
            "rdfs:comment": "The total number of bike racks or docking slots in bike docking station corresponding to this observation.",
            "rdfs:isDefinedBy": {
                "@id": "https://voc.iudx.org.in/"
            },
            "rdfs:label": "totalSlotNumber",
            "skos:exactMatch": {
                "@id": "https://uri.fiware.org/ns/data-models#totalSlotNumber"
            }
        },
        {
            "@id": "https://voc.iudx.org.in/transactionDateTime",
            "@type": [
                "iudx:TimeProperty"
            ],
            "iudx:domainIncludes": [
                {
                    "@id": "iudx:FareCollectionSystem"
                }
            ],
            "iudx:rangeIncludes": [
                {
                    "@id": "iudx:DateTime"
                },
                {
                    "@id": "iudx:ValueDescriptor"
                }
            ],
            "rdfs:comment": "Date-time of the transaction corresponding to this observation.",
            "rdfs:isDefinedBy": {
                "@id": "https://voc.iudx.org.in/"
            },
            "rdfs:label": "transactionDateTime"
        },
        {
            "@id": "https://voc.iudx.org.in/transactionType",
            "@type": [
                "iudx:TextProperty"
            ],
            "iudx:domainIncludes": [
                {
                    "@id": "iudx:FareCollectionSystem"
                }
            ],
            "iudx:rangeIncludes": [
                {
                    "@id": "iudx:Text"
                },
                {
                    "@id": "iudx:ValueDescriptor"
                }
            ],
            "rdfs:comment": "Type of the transaction corresponding to this observation. For Eg - Issue, ReIssue, Entry, Exit etc.",
            "rdfs:isDefinedBy": {
                "@id": "https://voc.iudx.org.in/"
            },
            "rdfs:label": "transactionType"
        },
        {
            "@id": "https://voc.iudx.org.in/transactionTypeDescription",
            "@type": [
                "iudx:TextProperty"
            ],
            "iudx:domainIncludes": [
                {
                    "@id": "iudx:FareCollectionSystem"
                }
            ],
            "iudx:rangeIncludes": [
                {
                    "@id": "iudx:Text"
                },
                {
                    "@id": "iudx:ValueDescriptor"
                }
            ],
            "rdfs:comment": "Description of the transaction type. Explanation of various transanctionTypeID codes used in the data.",
            "rdfs:isDefinedBy": {
                "@id": "https://voc.iudx.org.in/"
            },
            "rdfs:label": "transactionTypeDescription"
        },
        {
            "@id": "https://voc.iudx.org.in/transactionTypeID",
            "@type": [
                "iudx:TextProperty"
            ],
            "iudx:domainIncludes": [
                {
                    "@id": "iudx:FareCollectionSystem"
                }
            ],
            "iudx:rangeIncludes": [
                {
                    "@id": "iudx:Text"
                },
                {
                    "@id": "iudx:ValueDescriptor"
                }
            ],
            "rdfs:comment": "ID for the transactionType corresponding to this observation. 2401 - QR sale, C201- smart card entry , C202 - smart card exit etc.",
            "rdfs:isDefinedBy": {
                "@id": "https://voc.iudx.org.in/"
            },
            "rdfs:label": "transactionTypeID"
        },
        {
            "@id": "https://voc.iudx.org.in/transactionVehicleNum",
            "@type": [
                "iudx:QuantitativeProperty"
            ],
            "iudx:domainIncludes": [
                {
                    "@id": "iudx:FareCollectionSystem"
                }
            ],
            "iudx:rangeIncludes": [
                {
                    "@id": "iudx:Number"
                },
                {
                    "@id": "iudx:ValueDescriptor"
                }
            ],
            "rdfs:comment": "Code used by fare collection agency for the vehicle number corresponding to the transaction.",
            "rdfs:isDefinedBy": {
                "@id": "https://voc.iudx.org.in/"
            },
            "rdfs:label": "transactionVehicleNum"
        },
        {
            "@id": "https://voc.iudx.org.in/endDateTime",
            "@type": [
                "iudx:TimeProperty"
            ],
            "iudx:domainIncludes": [
                {
                    "@id": "iudx:Version"
                },
                {
                    "@id": "iudx:Camera"
                }
            ],
            "iudx:rangeIncludes": [
                {
                    "@id": "iudx:DateTime"
                },
                {
                    "@id": "iudx:ValueDescriptor"
                }
            ],
            "rdfs:comment": "Reported end time corresponding to this observation.",
            "rdfs:isDefinedBy": {
                "@id": "https://voc.iudx.org.in/"
            },
            "rdfs:label": "endDateTime"
        },
        {
            "@id": "https://voc.iudx.org.in/startDateTime",
            "@type": [
                "iudx:TimeProperty"
            ],
            "iudx:domainIncludes": [
                {
                    "@id": "iudx:Version"
                },
                {
                    "@id": "iudx:Camera"
                }
            ],
            "iudx:rangeIncludes": [
                {
                    "@id": "iudx:DateTime"
                },
                {
                    "@id": "iudx:ValueDescriptor"
                }
            ],
            "rdfs:comment": "Reported start time corresponding to this observation.",
            "rdfs:isDefinedBy": {
                "@id": "https://voc.iudx.org.in/"
            },
            "rdfs:label": "startDateTime"
        },
        {
            "@id": "https://voc.iudx.org.in/versionName",
            "@type": [
                "iudx:TextProperty"
            ],
            "iudx:domainIncludes": [
                {
                    "@id": "iudx:Version"
                }
            ],
            "iudx:rangeIncludes": [
                {
                    "@id": "iudx:Text"
                },
                {
                    "@id": "iudx:ValueDescriptor"
                }
            ],
            "rdfs:comment": "Version name corresponding to this observation",
            "rdfs:isDefinedBy": {
                "@id": "https://voc.iudx.org.in/"
            },
            "rdfs:label": "versionName"
        },
        {
            "@id": "https://voc.iudx.org.in/cameraName",
            "@type": [
                "iudx:TextProperty"
            ],
            "iudx:domainIncludes": [
                {
                    "@id": "iudx:Camera"
                }
            ],
            "iudx:rangeIncludes": [
                {
                    "@id": "iudx:Text"
                },
                {
                    "@id": "iudx:ValueDescriptor"
                }
            ],
            "rdfs:comment": "Name of the camera corresponding to this observation",
            "rdfs:isDefinedBy": {
                "@id": "https://voc.iudx.org.in/"
            },
            "rdfs:label": "cameraName"
        },
        {
            "@id": "https://voc.iudx.org.in/cameraNum",
            "@type": [
                "iudx:QuantitativeProperty"
            ],
            "iudx:domainIncludes": [
                {
                    "@id": "iudx:Camera"
                }
            ],
            "iudx:rangeIncludes": [
                {
                    "@id": "iudx:Number"
                },
                {
                    "@id": "iudx:ValueDescriptor"
                }
            ],
            "rdfs:comment": "Camera number corresponding to this observation",
            "rdfs:isDefinedBy": {
                "@id": "https://voc.iudx.org.in/"
            },
            "rdfs:label": "cameraNum"
        },
        {
            "@id": "https://voc.iudx.org.in/cameraOrientation",
            "@type": [
                "iudx:StructuredProperty"
            ],
            "iudx:domainIncludes": [
                {
                    "@id": "iudx:Camera"
                }
            ],
            "iudx:rangeIncludes": [
                {
                    "@id": "iudx:Orientation"
                }
            ],
            "rdfs:comment": "Orientation information for the camera corresponding to this observation",
            "rdfs:isDefinedBy": {
                "@id": "https://voc.iudx.org.in/"
            },
            "rdfs:label": "cameraOrientation"
        },
        {
            "@id": "https://voc.iudx.org.in/cameraType",
            "@type": [
                "iudx:TextProperty"
            ],
            "iudx:domainIncludes": [
                {
                    "@id": "iudx:Camera"
                }
            ],
            "iudx:rangeIncludes": [
                {
                    "@id": "iudx:Text"
                },
                {
                    "@id": "iudx:ValueDescriptor"
                }
            ],
            "rdfs:comment": "Type of the camera corresponding to this observation. ENUM: [FIXED, PTZ, DOME, DAY/NIGHT, C-MOUNT, BULLET].",
            "rdfs:isDefinedBy": {
                "@id": "https://voc.iudx.org.in/"
            },
            "rdfs:label": "cameraType"
        },
        {
            "@id": "https://voc.iudx.org.in/cameraUsage",
            "@type": [
                "iudx:TextProperty"
            ],
            "iudx:domainIncludes": [
                {
                    "@id": "iudx:Camera"
                }
            ],
            "iudx:rangeIncludes": [
                {
                    "@id": "iudx:Text"
                },
                {
                    "@id": "iudx:ValueDescriptor"
                }
            ],
            "rdfs:comment": "Purpose of the camera corresponding to this observation. ENUM: [SURVEILLANCE, RLVD, ANPR/LPR].",
            "rdfs:isDefinedBy": {
                "@id": "https://voc.iudx.org.in/"
            },
            "rdfs:label": "cameraUsage"
        },
        {
            "@id": "https://voc.iudx.org.in/imageSnapshot",
            "@type": [
                "iudx:TextProperty"
            ],
            "iudx:domainIncludes": [
                {
                    "@id": "iudx:Camera"
                }
            ],
            "iudx:rangeIncludes": [
                {
                    "@id": "iudx:Text"
                },
                {
                    "@id": "iudx:ValueDescriptor"
                }
            ],
            "rdfs:comment": "Camera feed snapshot download link for the camera corresponding to this observation",
            "rdfs:isDefinedBy": {
                "@id": "https://voc.iudx.org.in/"
            },
            "rdfs:label": "imageSnapshot"
        },
        {
            "@id": "https://voc.iudx.org.in/streamName",
            "@type": [
                "iudx:TextProperty"
            ],
            "iudx:domainIncludes": [
                {
                    "@id": "iudx:Camera"
                }
            ],
            "iudx:rangeIncludes": [
                {
                    "@id": "iudx:Text"
                },
                {
                    "@id": "iudx:ValueDescriptor"
                }
            ],
            "rdfs:comment": "Name of the video stream from the camera corresponding to this observation",
            "rdfs:isDefinedBy": {
                "@id": "https://voc.iudx.org.in/"
            },
            "rdfs:label": "streamName"
        },
        {
            "@id": "https://voc.iudx.org.in/streamURL",
            "@type": [
                "iudx:TextProperty"
            ],
            "iudx:domainIncludes": [
                {
                    "@id": "iudx:Camera"
                }
            ],
            "iudx:rangeIncludes": [
                {
                    "@id": "iudx:Text"
                },
                {
                    "@id": "iudx:ValueDescriptor"
                }
            ],
            "rdfs:comment": "URL providing video streaming information for the camera corresponding to this observation",
            "rdfs:isDefinedBy": {
                "@id": "https://voc.iudx.org.in/"
            },
            "rdfs:label": "streamURL"
        },
        {
            "@id": "https://voc.iudx.org.in/binCapacity",
            "@type": [
                "iudx:QuantitativeProperty"
            ],
            "iudx:domainIncludes": [
                {
                    "@id": "iudx:WmgmtBin"
                },
                {
                    "@id": "iudx:WasteBinModel"
                }
            ],
            "iudx:rangeIncludes": [
                {
                    "@id": "iudx:Number"
                },
                {
                    "@id": "iudx:ValueDescriptor"
                }
            ],
            "rdfs:comment": "Total capacity in terms of the volume of waste the bin can hold.",
            "rdfs:isDefinedBy": {
                "@id": "https://voc.iudx.org.in/"
            },
            "rdfs:label": "binCapacity",
            "skos:exactMatch": {
                "@id": "https://uri.fiware.org/ns/data-models#cargoVolume"
            }
        },
        {
            "@id": "https://voc.iudx.org.in/binCategory",
            "@type": [
                "iudx:TextProperty"
            ],
            "iudx:domainIncludes": [
                {
                    "@id": "iudx:WmgmtBin"
                },
                {
                    "@id": "iudx:WasteBinModel"
                }
            ],
            "iudx:rangeIncludes": [
                {
                    "@id": "iudx:Text"
                },
                {
                    "@id": "iudx:ValueDescriptor"
                }
            ],
            "rdfs:comment": "Category/type of the waste container bin. It can be a household bin or a dumpster or any other pre-defined category/type.",
            "rdfs:isDefinedBy": {
                "@id": "https://voc.iudx.org.in/"
            },
            "rdfs:label": "binCategory"
        },
        {
            "@id": "https://voc.iudx.org.in/binColor",
            "@type": [
                "iudx:TextProperty"
            ],
            "iudx:domainIncludes": [
                {
                    "@id": "iudx:WmgmtBin"
                },
                {
                    "@id": "iudx:WasteBinModel"
                }
            ],
            "iudx:rangeIncludes": [
                {
                    "@id": "iudx:Text"
                },
                {
                    "@id": "iudx:ValueDescriptor"
                }
            ],
            "rdfs:comment": "Color of the bin. Could be used for indicating the type of waste. The color coding should follow the conventions applicable to the geographical area the bins are located.",
            "rdfs:isDefinedBy": {
                "@id": "https://voc.iudx.org.in/"
            },
            "rdfs:label": "binColor",
            "skos:exactMatch": {
                "@id": "https://uri.fiware.org/ns/data-models#color"
            }
        },
        {
            "@id": "https://voc.iudx.org.in/binFullnessThreshold",
            "@type": [
                "iudx:QuantitativeProperty"
            ],
            "iudx:domainIncludes": [
                {
                    "@id": "iudx:WmgmtBin"
                },
                {
                    "@id": "iudx:WasteBinModel"
                }
            ],
            "iudx:rangeIncludes": [
                {
                    "@id": "iudx:Number"
                },
                {
                    "@id": "iudx:ValueDescriptor"
                }
            ],
            "rdfs:comment": "The fullness threshold level of the bin defined as the level (in terms of percentage) when the bin full alert or notification will be generated.",
            "rdfs:isDefinedBy": {
                "@id": "https://voc.iudx.org.in/"
            },
            "rdfs:label": "binFullnessThreshold",
            "skos:exactMatch": {
                "@id": "https://uri.fiware.org/ns/data-models#fullnessThreshold"
            }
        },
        {
            "@id": "https://voc.iudx.org.in/binMaxLoad",
            "@type": [
                "iudx:QuantitativeProperty"
            ],
            "iudx:domainIncludes": [
                {
                    "@id": "iudx:WmgmtBin"
                },
                {
                    "@id": "iudx:WasteBinModel"
                }
            ],
            "iudx:rangeIncludes": [
                {
                    "@id": "iudx:Number"
                },
                {
                    "@id": "iudx:ValueDescriptor"
                }
            ],
            "rdfs:comment": "Maximum load (weight) that the waste bin can hold.",
            "rdfs:isDefinedBy": {
                "@id": "https://voc.iudx.org.in/"
            },
            "rdfs:label": "binMaxLoad",
            "skos:exactMatch": {
                "@id": "https://uri.fiware.org/ns/data-models#maximumLoad"
            }
        },
        {
            "@id": "https://voc.iudx.org.in/binRecommendedLoad",
            "@type": [
                "iudx:QuantitativeProperty"
            ],
            "iudx:domainIncludes": [
                {
                    "@id": "iudx:WmgmtBin"
                },
                {
                    "@id": "iudx:WasteBinModel"
                }
            ],
            "iudx:rangeIncludes": [
                {
                    "@id": "iudx:Number"
                },
                {
                    "@id": "iudx:ValueDescriptor"
                }
            ],
            "rdfs:comment": "Recommended load (weight) that the waste bin corresponding to this observation can hold.",
            "rdfs:isDefinedBy": {
                "@id": "https://voc.iudx.org.in/"
            },
            "rdfs:label": "binRecommendedLoad",
            "skos:exactMatch": {
                "@id": "https://uri.fiware.org/ns/data-models#recommendedLoad"
            }
        },
        {
            "@id": "https://voc.iudx.org.in/binClearedTime",
            "@type": [
                "iudx:TimeProperty"
            ],
            "iudx:domainIncludes": [
                {
                    "@id": "iudx:WmgmtBin"
                }
            ],
            "iudx:rangeIncludes": [
                {
                    "@id": "iudx:DateTime"
                }
            ],
            "rdfs:comment": "Time when the bin was last cleared.",
            "rdfs:isDefinedBy": {
                "@id": "https://voc.iudx.org.in/"
            },
            "rdfs:label": "binClearedTime",
            "skos:exactMatch": {
                "@id": "https://uri.fiware.org/ns/data-models#dateLastEmptying"
            }
        },
        {
            "@id": "https://voc.iudx.org.in/binFillingLevel",
            "@type": [
                "iudx:QuantitativeProperty"
            ],
            "iudx:domainIncludes": [
                {
                    "@id": "iudx:WmgmtBin"
                }
            ],
            "iudx:rangeIncludes": [
                {
                    "@id": "iudx:Number"
                },
                {
                    "@id": "iudx:ValueDescriptor"
                }
            ],
            "rdfs:comment": "Current level of waste in the bin. Typically, the level is specified in terms of percentage volume filled.",
            "rdfs:isDefinedBy": {
                "@id": "https://voc.iudx.org.in/"
            },
            "rdfs:label": "binFillingLevel",
            "skos:exactMatch": {
                "@id": "https://uri.fiware.org/ns/data-models#fillingLevel"
            }
        },
        {
            "@id": "https://voc.iudx.org.in/binID",
            "@type": [
                "iudx:TextProperty"
            ],
            "iudx:domainIncludes": [
                {
                    "@id": "iudx:WmgmtBin"
                }
            ],
            "iudx:rangeIncludes": [
                {
                    "@id": "iudx:Text"
                },
                {
                    "@id": "iudx:ValueDescriptor"
                }
            ],
            "rdfs:comment": "ID of the waste carrying bin",
            "rdfs:isDefinedBy": {
                "@id": "https://voc.iudx.org.in/"
            },
            "rdfs:label": "binID"
        },
        {
            "@id": "https://voc.iudx.org.in/binLoggedTime",
            "@type": [
                "iudx:TimeProperty"
            ],
            "iudx:domainIncludes": [
                {
                    "@id": "iudx:WmgmtBin"
                }
            ],
            "iudx:rangeIncludes": [
                {
                    "@id": "iudx:DateTime"
                }
            ],
            "rdfs:comment": "Time when the bin's level was last logged.",
            "rdfs:isDefinedBy": {
                "@id": "https://voc.iudx.org.in/"
            },
            "rdfs:label": "binLoggedTime"
        },
        {
            "@id": "https://voc.iudx.org.in/bod",
            "@type": [
                "iudx:QuantitativeProperty"
            ],
            "iudx:domainIncludes": [
                {
                    "@id": "iudx:WasteWaterMgmt"
                }
            ],
            "iudx:rangeIncludes": [
                {
                    "@id": "iudx:Number"
                },
                {
                    "@id": "iudx:ValueDescriptor"
                }
            ],
            "rdfs:comment": "Biological Oxygen Demand concentration measured in the waste-water treatment plant corresponding to this observation.",
            "rdfs:isDefinedBy": {
                "@id": "https://voc.iudx.org.in/"
            },
            "rdfs:label": "bod",
            "skos:exactMatch": {
                "@id": "https://uri.fiware.org/ns/data-models#bod"
            }
        },
        {
            "@id": "https://voc.iudx.org.in/cod",
            "@type": [
                "iudx:QuantitativeProperty"
            ],
            "iudx:domainIncludes": [
                {
                    "@id": "iudx:WasteWaterMgmt"
                }
            ],
            "iudx:rangeIncludes": [
                {
                    "@id": "iudx:Number"
                },
                {
                    "@id": "iudx:ValueDescriptor"
                }
            ],
            "rdfs:comment": "Chemical Oxygen Demand concentration measured in the waste-water treatment plant corresponding to this observation.",
            "rdfs:isDefinedBy": {
                "@id": "https://voc.iudx.org.in/"
            },
            "rdfs:label": "cod",
            "skos:exactMatch": {
                "@id": "https://uri.fiware.org/ns/data-models#cod"
            }
        },
        {
            "@id": "https://voc.iudx.org.in/do",
            "@type": [
                "iudx:QuantitativeProperty"
            ],
            "iudx:domainIncludes": [
                {
                    "@id": "iudx:WasteWaterMgmt"
                }
            ],
            "iudx:rangeIncludes": [
                {
                    "@id": "iudx:Number"
                },
                {
                    "@id": "iudx:ValueDescriptor"
                }
            ],
            "rdfs:comment": "Dissolved oxygen measured in the waste-water treatment plant corresponding to this observation.",
            "rdfs:isDefinedBy": {
                "@id": "https://voc.iudx.org.in/"
            },
            "rdfs:label": "do",
            "skos:exactMatch": {
                "@id": "https://uri.fiware.org/ns/data-models#do"
            }
        },
        {
            "@id": "https://voc.iudx.org.in/fuelEfficiency",
            "@type": [
                "iudx:QuantitativeProperty"
            ],
            "iudx:domainIncludes": [
                {
                    "@id": "iudx:WmgmtVehicle"
                }
            ],
            "iudx:rangeIncludes": [
                {
                    "@id": "iudx:Number"
                },
                {
                    "@id": "iudx:ValueDescriptor"
                }
            ],
            "rdfs:comment": "The distance traveled per unit of fuel used, commonly in kilometers per liter (km/L).",
            "rdfs:isDefinedBy": {
                "@id": "https://voc.iudx.org.in/"
            },
            "rdfs:label": "fuelEfficiency",
            "skos:exactMatch": {
                "@id": "http://schema.org/fuelEfficiency"
            }
        },
        {
            "@id": "https://voc.iudx.org.in/fuelFilled",
            "@type": [
                "iudx:QuantitativeProperty"
            ],
            "iudx:domainIncludes": [
                {
                    "@id": "iudx:WmgmtVehicle"
                }
            ],
            "iudx:rangeIncludes": [
                {
                    "@id": "iudx:Number"
                },
                {
                    "@id": "iudx:ValueDescriptor"
                }
            ],
            "rdfs:comment": "Amount of fuel filled in liters to the vehicle corresponding to this observation.",
            "rdfs:isDefinedBy": {
                "@id": "https://voc.iudx.org.in/"
            },
            "rdfs:label": "fuelFilled"
        },
        {
            "@id": "https://voc.iudx.org.in/fuelType",
            "@type": [
                "iudx:TextProperty"
            ],
            "iudx:domainIncludes": [
                {
                    "@id": "iudx:WmgmtVehicle"
                }
            ],
            "iudx:rangeIncludes": [
                {
                    "@id": "iudx:Text"
                },
                {
                    "@id": "iudx:ValueDescriptor"
                }
            ],
            "rdfs:comment": "The type of fuel suitable for the engine or engines of the vehicle corresponding to this observation.",
            "rdfs:isDefinedBy": {
                "@id": "https://voc.iudx.org.in/"
            },
            "rdfs:label": "fuelType",
            "skos:exactMatch": {
                "@id": "http://schema.org/fuelType"
            }
        },
        {
            "@id": "https://voc.iudx.org.in/ignitionStatus",
            "@type": [
                "iudx:TextProperty"
            ],
            "iudx:domainIncludes": [
                {
                    "@id": "iudx:WmgmtVehicle"
                }
            ],
            "iudx:rangeIncludes": [
                {
                    "@id": "iudx:Text"
                },
                {
                    "@id": "iudx:ValueDescriptor"
                }
            ],
            "rdfs:comment": "Gives the ignition status of the vehicle.(Y, N)",
            "rdfs:isDefinedBy": {
                "@id": "https://voc.iudx.org.in/"
            },
            "rdfs:label": "ignitionStatus"
        },
        {
            "@id": "https://voc.iudx.org.in/inFlow",
            "@type": [
                "iudx:QuantitativeProperty"
            ],
            "iudx:domainIncludes": [
                {
                    "@id": "iudx:WasteWaterMgmt"
                }
            ],
            "iudx:rangeIncludes": [
                {
                    "@id": "iudx:Number"
                },
                {
                    "@id": "iudx:ValueDescriptor"
                }
            ],
            "rdfs:comment": "In-flow amount into the treatment plant/reservoir corresponding to this observation.",
            "rdfs:isDefinedBy": {
                "@id": "https://voc.iudx.org.in/"
            },
            "rdfs:label": "inFlow"
        },
        {
            "@id": "https://voc.iudx.org.in/nh4",
            "@type": [
                "iudx:QuantitativeProperty"
            ],
            "iudx:domainIncludes": [
                {
                    "@id": "iudx:WasteWaterMgmt"
                }
            ],
            "iudx:rangeIncludes": [
                {
                    "@id": "iudx:Number"
                },
                {
                    "@id": "iudx:ValueDescriptor"
                }
            ],
            "rdfs:comment": "Ammonium concentration measured in the waste-water treatment plant corresponding to this observation.",
            "rdfs:isDefinedBy": {
                "@id": "https://voc.iudx.org.in/"
            },
            "rdfs:label": "nh4",
            "skos:exactMatch": {
                "@id": "https://uri.fiware.org/ns/data-models#nh4"
            }
        },
        {
            "@id": "https://voc.iudx.org.in/no3",
            "@type": [
                "iudx:QuantitativeProperty"
            ],
            "iudx:domainIncludes": [
                {
                    "@id": "iudx:WasteWaterMgmt"
                }
            ],
            "iudx:rangeIncludes": [
                {
                    "@id": "iudx:Number"
                },
                {
                    "@id": "iudx:ValueDescriptor"
                }
            ],
            "rdfs:comment": "Nitrate concentration measured in waste-water treatment plant corresponding to this observation.",
            "rdfs:isDefinedBy": {
                "@id": "https://voc.iudx.org.in/"
            },
            "rdfs:label": "no3",
            "skos:exactMatch": {
                "@id": "https://uri.fiware.org/ns/data-models#no3"
            }
        },
        {
            "@id": "https://voc.iudx.org.in/outFlow",
            "@type": [
                "iudx:QuantitativeProperty"
            ],
            "iudx:domainIncludes": [
                {
                    "@id": "iudx:WasteWaterMgmt"
                }
            ],
            "iudx:rangeIncludes": [
                {
                    "@id": "iudx:Number"
                },
                {
                    "@id": "iudx:ValueDescriptor"
                }
            ],
            "rdfs:comment": "Out-flow amount into the treatment plant/reservoir corresponding to this observation.",
            "rdfs:isDefinedBy": {
                "@id": "https://voc.iudx.org.in/"
            },
            "rdfs:label": "outFlow"
        },
        {
            "@id": "https://voc.iudx.org.in/po4",
            "@type": [
                "iudx:QuantitativeProperty"
            ],
            "iudx:domainIncludes": [
                {
                    "@id": "iudx:WasteWaterMgmt"
                }
            ],
            "iudx:rangeIncludes": [
                {
                    "@id": "iudx:Number"
                },
                {
                    "@id": "iudx:ValueDescriptor"
                }
            ],
            "rdfs:comment": "Ortho-phosphate concentration measured in the waste-water treatment plant corresponding to this observation.",
            "rdfs:isDefinedBy": {
                "@id": "https://voc.iudx.org.in/"
            },
            "rdfs:label": "po4",
            "skos:exactMatch": {
                "@id": "https://uri.fiware.org/ns/data-models#po4"
            }
        },
        {
            "@id": "https://voc.iudx.org.in/redox",
            "@type": [
                "iudx:QuantitativeProperty"
            ],
            "iudx:domainIncludes": [
                {
                    "@id": "iudx:WasteWaterMgmt"
                }
            ],
            "iudx:rangeIncludes": [
                {
                    "@id": "iudx:Number"
                },
                {
                    "@id": "iudx:ValueDescriptor"
                }
            ],
            "rdfs:comment": "Reduction potential or oxidation measured in waste-water treatment plant corresponding to this observation.",
            "rdfs:isDefinedBy": {
                "@id": "https://voc.iudx.org.in/"
            },
            "rdfs:label": "redox",
            "skos:exactMatch": {
                "@id": "https://uri.fiware.org/ns/data-models#redox"
            }
        },
        {
            "@id": "https://voc.iudx.org.in/tic",
            "@type": [
                "iudx:QuantitativeProperty"
            ],
            "iudx:domainIncludes": [
                {
                    "@id": "iudx:WasteWaterMgmt"
                }
            ],
            "iudx:rangeIncludes": [
                {
                    "@id": "iudx:Number"
                },
                {
                    "@id": "iudx:ValueDescriptor"
                }
            ],
            "rdfs:comment": "Total Inorganic Carbon concentration measured in the waste-water treatment plant corresponding to this observation.",
            "rdfs:isDefinedBy": {
                "@id": "https://voc.iudx.org.in/"
            },
            "rdfs:label": "tic",
            "skos:exactMatch": {
                "@id": "https://uri.fiware.org/ns/data-models#tic"
            }
        },
        {
            "@id": "https://voc.iudx.org.in/tn",
            "@type": [
                "iudx:QuantitativeProperty"
            ],
            "iudx:domainIncludes": [
                {
                    "@id": "iudx:WasteWaterMgmt"
                }
            ],
            "iudx:rangeIncludes": [
                {
                    "@id": "iudx:Number"
                },
                {
                    "@id": "iudx:ValueDescriptor"
                }
            ],
            "rdfs:comment": "Total Nitrogen concentration measured in waste-water treatment plant corresponding to this observation.",
            "rdfs:isDefinedBy": {
                "@id": "https://voc.iudx.org.in/"
            },
            "rdfs:label": "tn",
            "skos:exactMatch": {
                "@id": "https://uri.fiware.org/ns/data-models#tn"
            }
        },
        {
            "@id": "https://voc.iudx.org.in/toc",
            "@type": [
                "iudx:QuantitativeProperty"
            ],
            "iudx:domainIncludes": [
                {
                    "@id": "iudx:WasteWaterMgmt"
                }
            ],
            "iudx:rangeIncludes": [
                {
                    "@id": "iudx:Number"
                },
                {
                    "@id": "iudx:ValueDescriptor"
                }
            ],
            "rdfs:comment": "Total Organic Carbon concentration measured in the waste-water treatment plant corresponding to this observation.",
            "rdfs:isDefinedBy": {
                "@id": "https://voc.iudx.org.in/"
            },
            "rdfs:label": "toc",
            "skos:exactMatch": {
                "@id": "https://uri.fiware.org/ns/data-models#toc"
            }
        },
        {
            "@id": "https://voc.iudx.org.in/treatmentPlantCapacity",
            "@type": [
                "iudx:QuantitativeProperty"
            ],
            "iudx:domainIncludes": [
                {
                    "@id": "iudx:WasteWaterMgmt"
                }
            ],
            "iudx:rangeIncludes": [
                {
                    "@id": "iudx:Number"
                },
                {
                    "@id": "iudx:ValueDescriptor"
                }
            ],
            "rdfs:comment": "Handling capacity of the waste-water treatment plant corresponding to this observation.",
            "rdfs:isDefinedBy": {
                "@id": "https://voc.iudx.org.in/"
            },
            "rdfs:label": "treatmentPlantCapacity"
        },
        {
            "@id": "https://voc.iudx.org.in/treatmentPlantCode",
            "@type": [
                "iudx:TextProperty"
            ],
            "iudx:domainIncludes": [
                {
                    "@id": "iudx:WasteWaterMgmt"
                }
            ],
            "iudx:rangeIncludes": [
                {
                    "@id": "iudx:Text"
                }
            ],
            "rdfs:comment": "Unique code for the waste-water treatment plant corresponding to this observation.",
            "rdfs:isDefinedBy": {
                "@id": "https://voc.iudx.org.in/"
            },
            "rdfs:label": "treatmentPlantCode"
        },
        {
            "@id": "https://voc.iudx.org.in/treatmentPlantID",
            "@type": [
                "iudx:QuantitativeProperty"
            ],
            "iudx:domainIncludes": [
                {
                    "@id": "iudx:WasteWaterMgmt"
                }
            ],
            "iudx:rangeIncludes": [
                {
                    "@id": "iudx:Number"
                },
                {
                    "@id": "iudx:ValueDescriptor"
                }
            ],
            "rdfs:comment": "Unique identification number for the waste-water treatment plant corresponding to this observation.",
            "rdfs:isDefinedBy": {
                "@id": "https://voc.iudx.org.in/"
            },
            "rdfs:label": "treatmentPlantID"
        },
        {
            "@id": "https://voc.iudx.org.in/treatmentPlantName",
            "@type": [
                "iudx:TextProperty"
            ],
            "iudx:domainIncludes": [
                {
                    "@id": "iudx:WasteWaterMgmt"
                }
            ],
            "iudx:rangeIncludes": [
                {
                    "@id": "iudx:Text"
                },
                {
                    "@id": "iudx:ValueDescriptor"
                }
            ],
            "rdfs:comment": "Name of the waste-water treatment plant corresponding to this observation.",
            "rdfs:isDefinedBy": {
                "@id": "https://voc.iudx.org.in/"
            },
            "rdfs:label": "treatmentPlantName"
        },
        {
            "@id": "https://voc.iudx.org.in/tripNetWeightCollected",
            "@type": [
                "iudx:QuantitativeProperty"
            ],
            "iudx:domainIncludes": [
                {
                    "@id": "iudx:WmgmtVehicle"
                }
            ],
            "iudx:rangeIncludes": [
                {
                    "@id": "iudx:Number"
                },
                {
                    "@id": "iudx:ValueDescriptor"
                }
            ],
            "rdfs:comment": "The net weight of garbage collected by the SWM vehicle corresponding to this observation at the end of the trip.",
            "rdfs:isDefinedBy": {
                "@id": "https://voc.iudx.org.in/"
            },
            "rdfs:label": "tripNetWeightCollected"
        },
        {
            "@id": "https://voc.iudx.org.in/tss",
            "@type": [
                "iudx:QuantitativeProperty"
            ],
            "iudx:domainIncludes": [
                {
                    "@id": "iudx:WasteWaterMgmt"
                }
            ],
            "iudx:rangeIncludes": [
                {
                    "@id": "iudx:Number"
                },
                {
                    "@id": "iudx:ValueDescriptor"
                }
            ],
            "rdfs:comment": "Total suspended solids concentration measured in a waste-water treatment plant corresponding to this observation.",
            "rdfs:isDefinedBy": {
                "@id": "https://voc.iudx.org.in/"
            },
            "rdfs:label": "tss",
            "skos:exactMatch": {
                "@id": "https://uri.fiware.org/ns/data-models#tss"
            }
        },
        {
            "@id": "https://voc.iudx.org.in/vehicleAltitude",
            "@type": [
                "iudx:QuantitativeProperty"
            ],
            "iudx:domainIncludes": [
                {
                    "@id": "iudx:WmgmtVehicle"
                }
            ],
            "iudx:rangeIncludes": [
                {
                    "@id": "iudx:Number"
                },
                {
                    "@id": "iudx:ValueDescriptor"
                }
            ],
            "rdfs:comment": "Gives the current altitude of the vehicle using GPS",
            "rdfs:isDefinedBy": {
                "@id": "https://voc.iudx.org.in/"
            },
            "rdfs:label": "vehicleAltitude"
        },
        {
            "@id": "https://voc.iudx.org.in/vehicleRunningStatus",
            "@type": [
                "iudx:TextProperty"
            ],
            "iudx:domainIncludes": [
                {
                    "@id": "iudx:WmgmtVehicle"
                }
            ],
            "iudx:rangeIncludes": [
                {
                    "@id": "iudx:Text"
                },
                {
                    "@id": "iudx:ValueDescriptor"
                }
            ],
            "rdfs:comment": "Moving status of the vehicle, one of running, waiting, stopped.",
            "rdfs:isDefinedBy": {
                "@id": "https://voc.iudx.org.in/"
            },
            "rdfs:label": "vehicleRunningStatus"
        },
        {
            "@id": "https://voc.iudx.org.in/vehicleTrackerDevice",
            "@type": [
                "iudx:TextProperty"
            ],
            "iudx:domainIncludes": [
                {
                    "@id": "iudx:WmgmtVehicle"
                }
            ],
            "iudx:rangeIncludes": [
                {
                    "@id": "iudx:Text"
                },
                {
                    "@id": "iudx:ValueDescriptor"
                }
            ],
            "rdfs:comment": "Installation status of the GPS device or the tracking device fitted to the vehicle corresponding to this observation.",
            "rdfs:isDefinedBy": {
                "@id": "https://voc.iudx.org.in/"
            },
            "rdfs:label": "vehicleTrackerDevice"
        },
        {
            "@id": "https://voc.iudx.org.in/vehicleType",
            "@type": [
                "iudx:TextProperty"
            ],
            "iudx:domainIncludes": [
                {
                    "@id": "iudx:WmgmtVehicle"
                },
                {
                    "@id": "iudx:TransitManagement"
                },
                {
                    "@id": "iudx:RevenueCollection"
                }
            ],
            "iudx:rangeIncludes": [
                {
                    "@id": "iudx:Text"
                },
                {
                    "@id": "iudx:ValueDescriptor"
                }
            ],
            "rdfs:comment": "Describes the type of vehicle corresponding to this observation, could be hopper, compactor, tipper, dumper in case of solid waste management vehicles, BRT mini bus, BRT bus, city bus in case of ITMS vehicles and Moped/Scooter, Motor Cycle,  Autorickshaw, Private car/ Jeep car, Tempo, Bus, E-Moped/E-Scooter/E-Motor Cycle, Public motor in case of vehicle registration.",
            "rdfs:isDefinedBy": {
                "@id": "https://voc.iudx.org.in/"
            },
            "rdfs:label": "vehicleType"
        },
        {
            "@id": "https://voc.iudx.org.in/wardID",
            "@type": [
                "iudx:TextProperty"
            ],
            "iudx:domainIncludes": [
                {
                    "@id": "iudx:WmgmtBin"
                },
                {
                    "@id": "iudx:WmgmtVehicle"
                },
                {
                    "@id": "iudx:PointOfInterest"
                },
                {
                    "@id": "iudx:IssueReporting"
                }
            ],
            "iudx:rangeIncludes": [
                {
                    "@id": "iudx:Text"
                },
                {
                    "@id": "iudx:ValueDescriptor"
                }
            ],
            "rdfs:comment": "Ward ID of the entity corresponding to this observation.",
            "rdfs:isDefinedBy": {
                "@id": "https://voc.iudx.org.in/"
            },
            "rdfs:label": "wardID"
        },
        {
            "@id": "https://voc.iudx.org.in/wardName",
            "@type": [
                "iudx:TextProperty"
            ],
            "iudx:domainIncludes": [
                {
                    "@id": "iudx:WmgmtVehicle"
                },
                {
                    "@id": "iudx:PointOfInterest"
                }
            ],
            "iudx:rangeIncludes": [
                {
                    "@id": "iudx:Text"
                },
                {
                    "@id": "iudx:ValueDescriptor"
                }
            ],
            "rdfs:comment": "Ward name of the entity corresponding to this observation.",
            "rdfs:isDefinedBy": {
                "@id": "https://voc.iudx.org.in/"
            },
            "rdfs:label": "wardName"
        },
        {
            "@id": "https://voc.iudx.org.in/wasteBinInfo",
            "@type": [
                "iudx:StructuredProperty"
            ],
            "iudx:domainIncludes": [
                {
                    "@id": "iudx:WmgmtBin"
                }
            ],
            "iudx:rangeIncludes": [
                {
                    "@id": "iudx:WasteBinModel"
                }
            ],
            "rdfs:comment": "Describes the information of the waste bin device, sensor in consideration",
            "rdfs:isDefinedBy": {
                "@id": "https://voc.iudx.org.in/"
            },
            "rdfs:label": "wasteBinInfo"
        },
        {
            "@id": "https://voc.iudx.org.in/ZoneID",
            "@type": [
                "iudx:TextProperty"
            ],
            "iudx:domainIncludes": [
                {
                    "@id": "iudx:PointOfInterest"
                }
            ],
            "iudx:rangeIncludes": [
                {
                    "@id": "iudx:Text"
                },
                {
                    "@id": "iudx:ValueDescriptor"
                }
            ],
            "rdfs:comment": "Zone ID of the entity corresponding to this observation.",
            "rdfs:isDefinedBy": {
                "@id": "https://voc.iudx.org.in/"
            },
            "rdfs:label": "ZoneID"
        },
        {
            "@id": "https://voc.iudx.org.in/zoneName",
            "@type": [
                "iudx:TextProperty"
            ],
            "iudx:domainIncludes": [
                {
                    "@id": "iudx:WmgmtVehicle"
                },
                {
                    "@id": "iudx:PointOfInterest"
                }
            ],
            "iudx:rangeIncludes": [
                {
                    "@id": "iudx:Text"
                },
                {
                    "@id": "iudx:ValueDescriptor"
                }
            ],
            "rdfs:comment": "Zone name of the entity corresponding to this observation.",
            "rdfs:isDefinedBy": {
                "@id": "https://voc.iudx.org.in/"
            },
            "rdfs:label": "zoneName"
        },
        {
            "@id": "https://voc.iudx.org.in/department",
            "@type": [
                "iudx:TextProperty"
            ],
            "iudx:domainIncludes": [
                {
                    "@id": "iudx:EmployeeDetails"
                }
            ],
            "iudx:rangeIncludes": [
                {
                    "@id": "iudx:Text"
                },
                {
                    "@id": "iudx:ValueDescriptor"
                }
            ],
            "rdfs:comment": "Division or section of the organization corresponding to this observation. Eg. Health, Transport.",
            "rdfs:isDefinedBy": {
                "@id": "https://voc.iudx.org.in/"
            },
            "rdfs:label": "department",
            "skos:exactMatch": {
                "@id": "http://schema.org/department"
            }
        },
        {
            "@id": "https://voc.iudx.org.in/employeeDesignation",
            "@type": [
                "iudx:TextProperty"
            ],
            "iudx:domainIncludes": [
                {
                    "@id": "iudx:EmployeeDetails"
                }
            ],
            "iudx:rangeIncludes": [
                {
                    "@id": "iudx:Text"
                },
                {
                    "@id": "iudx:ValueDescriptor"
                }
            ],
            "rdfs:comment": "Title assigned to the employee corresponding to this observation. Eg. Sweeper, Driver, Helper, Supervisor, Safai Meth, Cleaner, Bhisti. etc.",
            "rdfs:isDefinedBy": {
                "@id": "https://voc.iudx.org.in/"
            },
            "rdfs:label": "employeeDesignation",
            "skos:exactMatch": {
                "@id": "http://schema.org/jobTitle"
            }
        },
        {
            "@id": "https://voc.iudx.org.in/employeeID",
            "@type": [
                "iudx:TextProperty"
            ],
            "iudx:domainIncludes": [
                {
                    "@id": "iudx:EmployeeDetails"
                }
            ],
            "iudx:rangeIncludes": [
                {
                    "@id": "iudx:Text"
                },
                {
                    "@id": "iudx:ValueDescriptor"
                }
            ],
            "rdfs:comment": "Unique ID of the employee corresponding to this observation",
            "rdfs:isDefinedBy": {
                "@id": "https://voc.iudx.org.in/"
            },
            "rdfs:label": "employeeID"
        },
        {
            "@id": "https://voc.iudx.org.in/employmentType",
            "@type": [
                "iudx:TextProperty"
            ],
            "iudx:domainIncludes": [
                {
                    "@id": "iudx:EmployeeDetails"
                }
            ],
            "iudx:rangeIncludes": [
                {
                    "@id": "iudx:Text"
                },
                {
                    "@id": "iudx:ValueDescriptor"
                }
            ],
            "rdfs:comment": "Type of employment. ENUM: [Contractual New, Contractual Old, Regular, Outsourcing]",
            "rdfs:isDefinedBy": {
                "@id": "https://voc.iudx.org.in/"
            },
            "rdfs:label": "employmentType",
            "skos:exactMatch": {
                "@id": "http://schema.org/employmentType"
            }
        },
        {
            "@id": "https://voc.iudx.org.in/employmentUnit",
            "@type": [
                "iudx:TextProperty"
            ],
            "iudx:domainIncludes": [
                {
                    "@id": "iudx:EmployeeDetails"
                }
            ],
            "iudx:rangeIncludes": [
                {
                    "@id": "iudx:Text"
                },
                {
                    "@id": "iudx:ValueDescriptor"
                }
            ],
            "rdfs:comment": "Unit and/or facility where the employee reports and/or in which the job is to be performed.\nENUM: [Sweeping, Drainage, Vehicle Driver, Vehicle Helper, Workshop, Door to Door, Supervisor, Office Work]",
            "rdfs:isDefinedBy": {
                "@id": "https://voc.iudx.org.in/"
            },
            "rdfs:label": "employmentUnit",
            "skos:exactMatch": {
                "@id": "http://schema.org/employmentUnit"
            }
        },
        {
            "@id": "https://voc.iudx.org.in/gender",
            "@type": [
                "iudx:TextProperty"
            ],
            "iudx:domainIncludes": [
                {
                    "@id": "iudx:EmployeeDetails"
                }
            ],
            "iudx:rangeIncludes": [
                {
                    "@id": "iudx:Text"
                },
                {
                    "@id": "iudx:ValueDescriptor"
                }
            ],
            "rdfs:comment": "Gender of the employee or person corresponding to this observation.",
            "rdfs:isDefinedBy": {
                "@id": "https://voc.iudx.org.in/"
            },
            "rdfs:label": "gender",
            "skos:exactMatch": {
                "@id": "http://schema.org/gender"
            }
        },
        {
            "@id": "https://voc.iudx.org.in/municipalityInfo",
            "@type": [
                "iudx:StructuredProperty"
            ],
            "iudx:domainIncludes": [
                {
                    "@id": "iudx:EmployeeDetails"
                }
            ],
            "iudx:rangeIncludes": [
                {
                    "@id": "iudx:MunicipalityDesc"
                }
            ],
            "rdfs:comment": "Municipality information corresponding to this observation.",
            "rdfs:isDefinedBy": {
                "@id": "https://voc.iudx.org.in/"
            },
            "rdfs:label": "municipalityInfo"
        },
        {
            "@id": "https://voc.iudx.org.in/serviceCompany",
            "@type": [
                "iudx:TextProperty"
            ],
            "iudx:domainIncludes": [
                {
                    "@id": "iudx:EmployeeDetails"
                }
            ],
            "iudx:rangeIncludes": [
                {
                    "@id": "iudx:Text"
                },
                {
                    "@id": "iudx:ValueDescriptor"
                }
            ],
            "rdfs:comment": "Service agency or company corresponding to this observation",
            "rdfs:isDefinedBy": {
                "@id": "https://voc.iudx.org.in/"
            },
            "rdfs:label": "serviceCompany"
        },
        {
            "@id": "https://voc.iudx.org.in/totalAbsent",
            "@type": [
                "iudx:QuantitativeProperty"
            ],
            "iudx:domainIncludes": [
                {
                    "@id": "iudx:EmployeeDetails"
                }
            ],
            "iudx:rangeIncludes": [
                {
                    "@id": "iudx:Number"
                },
                {
                    "@id": "iudx:ValueDescriptor"
                }
            ],
            "rdfs:comment": "Number of employees failed to report to work",
            "rdfs:isDefinedBy": {
                "@id": "https://voc.iudx.org.in/"
            },
            "rdfs:label": "totalAbsent"
        },
        {
            "@id": "https://voc.iudx.org.in/totalEmployee",
            "@type": [
                "iudx:QuantitativeProperty"
            ],
            "iudx:domainIncludes": [
                {
                    "@id": "iudx:EmployeeDetails"
                }
            ],
            "iudx:rangeIncludes": [
                {
                    "@id": "iudx:Number"
                },
                {
                    "@id": "iudx:ValueDescriptor"
                }
            ],
            "rdfs:comment": "Number of the employees in the organization",
            "rdfs:isDefinedBy": {
                "@id": "https://voc.iudx.org.in/"
            },
            "rdfs:label": "totalEmployee",
            "skos:exactMatch": {
                "@id": "http://schema.org/numberOfEmployees"
            }
        },
        {
            "@id": "https://voc.iudx.org.in/totalPresent",
            "@type": [
                "iudx:QuantitativeProperty"
            ],
            "iudx:domainIncludes": [
                {
                    "@id": "iudx:EmployeeDetails"
                }
            ],
            "iudx:rangeIncludes": [
                {
                    "@id": "iudx:Number"
                },
                {
                    "@id": "iudx:ValueDescriptor"
                }
            ],
            "rdfs:comment": "Number of employees reported to work",
            "rdfs:isDefinedBy": {
                "@id": "https://voc.iudx.org.in/"
            },
            "rdfs:label": "totalPresent"
        },
        {
            "@id": "https://voc.iudx.org.in/accessObject",
            "@type": [
                "iudx:Relationship"
            ],
            "iudx:domainIncludes": [
                {
                    "@id": "iudx:AccessObjectInfoValue"
                }
            ],
            "iudx:rangeIncludes": [
                {
                    "@id": "iudx:Text",
                    "@type": "@id"
                },
                {
                    "@id": "iudx:RelationshipValue"
                }
            ],
            "rdfs:comment": "Link to the access object. For example, an open API object.",
            "rdfs:isDefinedBy": {
                "@id": "https://voc.iudx.org.in/"
            },
            "rdfs:label": "accessObject"
        },
        {
            "@id": "https://voc.iudx.org.in/accessObjectInfo",
            "@type": [
                "iudx:StructuredProperty"
            ],
            "iudx:domainIncludes": [
                {
                    "@id": "iudx:ResourceGroup"
                }
            ],
            "iudx:rangeIncludes": [
                {
                    "@id": "iudx:AccessObjectInfoValue"
                }
            ],
            "rdfs:comment": "Link to the access object. For example, an open API object.",
            "rdfs:isDefinedBy": {
                "@id": "https://voc.iudx.org.in/"
            },
            "rdfs:label": "accessObjectInfo"
        },
        {
            "@id": "https://voc.iudx.org.in/accessObjectType",
            "@type": [
                "iudx:TextProperty"
            ],
            "iudx:domainIncludes": [
                {
                    "@id": "iudx:AccessObjectInfoValue"
                }
            ],
            "iudx:rangeIncludes": [
                {
                    "@id": "iudx:Text"
                }
            ],
            "rdfs:comment": "Type of access object. ENUM: [OpenAPI, AsyncAPI]",
            "rdfs:isDefinedBy": {
                "@id": "https://voc.iudx.org.in/"
            },
            "rdfs:label": "accessObjectType"
        },
        {
            "@id": "https://voc.iudx.org.in/accessPolicy",
            "@type": [
                "iudx:TextProperty"
            ],
            "iudx:domainIncludes": [
                {
                    "@id": "iudx:ResourceGroup"
                },
                {
                    "@id": "iudx:Resource"
                }
            ],
            "iudx:rangeIncludes": [
                {
                    "@id": "iudx:Text"
                }
            ],
            "rdfs:comment": "Defines the access policy for resources belonging to ResourceGroup or an individual Resource. In case of ResourceGroup item, it can take values: [OPEN, SECURE, MIXED]. OPEN implies all Resources in the group are open (and need no authorization token for data access). SECURE implies that all Resources are secured and will need authorization token for access. MIXED implies that some of Resource items may be open. In case of accessPolicy being set to MIXED in the resource group, the individual resource items will further qualify the access policy using this field. In case of Resource item, it will take values from: [OPEN, SECURE].",
            "rdfs:isDefinedBy": {
                "@id": "https://voc.iudx.org.in/"
            },
            "rdfs:label": "accessPolicy"
        },
        {
            "@id": "https://voc.iudx.org.in/additionalInfoURL",
            "@type": [
                "iudx:Relationship"
            ],
            "iudx:domainIncludes": [
                {
                    "@id": "iudx:AccessObjectInfoValue"
                },
                {
                    "@id": "iudx:Organization"
                },
                {
                    "@id": "iudx:PointOfInterest"
                }
            ],
            "iudx:rangeIncludes": [
                {
                    "@id": "iudx:Text",
                    "@type": "@id"
                },
                {
                    "@id": "iudx:RelationshipValue"
                }
            ],
            "rdfs:comment": "URL from which additional information of the subject can be obtained",
            "rdfs:isDefinedBy": {
                "@id": "https://voc.iudx.org.in/"
            },
            "rdfs:label": "additionalInfoURL"
        },
        {
            "@id": "https://voc.iudx.org.in/address",
            "@type": [
                "iudx:GeoProperty"
            ],
            "iudx:domainIncludes": [
                {
                    "@id": "iudx:Place"
                },
                {
                    "@id": "iudx:PointOfInterest"
                },
                {
                    "@id": "iudx:IssueReporting"
                },
                {
                    "@id": "iudx:Streetlight"
                },
                {
                    "@id": "iudx:BikeDockingStation"
                },
                {
                    "@id": "iudx:WaterDistributionNetwork"
                }
            ],
            "iudx:rangeIncludes": [
                {
                    "@id": "iudx:Text"
                },
                {
                    "@id": "iudx:ValueDescriptor"
                }
            ],
            "rdfs:comment": "Physical address of a place.",
            "rdfs:isDefinedBy": {
                "@id": "https://voc.iudx.org.in/"
            },
            "rdfs:label": "address",
            "skos:exactMatch": {
                "@id": "http://schema.org/address"
            }
        },
        {
            "@id": "https://voc.iudx.org.in/aggregationDuration",
            "@type": [
                "rdf:Property"
            ],
            "iudx:domainIncludes": [
                {
                    "@id": "iudx:ValueDescriptor"
                }
            ],
            "iudx:rangeIncludes": [
                {
                    "@id": "iudx:Number"
                },
                {
                    "@id": "iudx:ValueDescriptor"
                }
            ],
            "rdfs:comment": "Specifies the interval duration for computing statistical aggregations. Default duration interval unit is in Hours. Other units can be specified using ValueDescriptor Type.",
            "rdfs:isDefinedBy": {
                "@id": "https://voc.iudx.org.in/"
            },
            "rdfs:label": "aggregationDuration"
        },
        {
            "@id": "https://voc.iudx.org.in/areaServed",
            "@type": [
                "iudx:GeoProperty"
            ],
            "iudx:domainIncludes": [
                {
                    "@id": "iudx:ModelInfo"
                },
                {
                    "@id": "iudx:StreetLightFeeder"
                }
            ],
            "iudx:rangeIncludes": [
                {
                    "@id": "iudx:Text"
                }
            ],
            "rdfs:comment": "Area served by the entity or a service.",
            "rdfs:isDefinedBy": {
                "@id": "https://voc.iudx.org.in/"
            },
            "rdfs:label": "areaServed"
        },
        {
            "@id": "https://voc.iudx.org.in/authControlLevel",
            "@type": [
                "iudx:TextProperty"
            ],
            "iudx:domainIncludes": [
                {
                    "@id": "iudx:ResourceGroup"
                }
            ],
            "iudx:rangeIncludes": [
                {
                    "@id": "iudx:Text"
                }
            ],
            "rdfs:comment": "Authorizataion Control Level for resouces associated with a given resource-group.  Individual authorization control level indicates that access control is available per resource, i.e., authorization can be granted/not-granted on a per resource basis for the resources. Group authorization control level indicates that the authorization is available on group level only, i.e., authorization will be granted/not-granted for all the resources associated with the given resource group. ENUM: [GROUP, INDIVIDUAL]. Default value is set to GROUP. This field is applicable only for non-open data, i.e., when the accessPolicy field is set to value other than OPEN.",
            "rdfs:isDefinedBy": {
                "@id": "https://voc.iudx.org.in/"
            },
            "rdfs:label": "authControlLevel"
        },
        {
            "@id": "https://voc.iudx.org.in/authServerInfo",
            "@type": [
                "iudx:StructuredProperty"
            ],
            "iudx:domainIncludes": [
                {
                    "@id": "iudx:Resource"
                },
                {
                    "@id": "iudx:ResourceGroup",
                    "iudx:requiredProperty": true
                }
            ],
            "iudx:rangeIncludes": [
                {
                    "@id": "iudx:AuthServerInfoValue"
                }
            ],
            "rdfs:comment": "Information about the Authorization Server used for a given resource.",
            "rdfs:isDefinedBy": {
                "@id": "https://voc.iudx.org.in/"
            },
            "rdfs:label": "authServerInfo"
        },
        {
            "@id": "https://voc.iudx.org.in/authServerURL",
            "@type": [
                "iudx:Relationship"
            ],
            "iudx:domainIncludes": [
                {
                    "@id": "iudx:AuthServerInfoValue"
                }
            ],
            "iudx:rangeIncludes": [
                {
                    "@id": "iudx:Text",
                    "@type": "@id"
                },
                {
                    "@id": "iudx:RelationshipValue"
                }
            ],
            "rdfs:comment": "URL of the IUDX authorization server used for a given resource.",
            "rdfs:isDefinedBy": {
                "@id": "https://voc.iudx.org.in/"
            },
            "rdfs:label": "authServerURL"
        },
        {
            "@id": "https://voc.iudx.org.in/authType",
            "@type": [
                "iudx:TextProperty"
            ],
            "iudx:domainIncludes": [
                {
                    "@id": "iudx:AuthServerInfoValue"
                }
            ],
            "iudx:rangeIncludes": [
                {
                    "@id": "iudx:Text"
                }
            ],
            "rdfs:comment": "Identification of the auth scheme used for a given resource.  ENUM: [IUDXAUTH].",
            "rdfs:isDefinedBy": {
                "@id": "https://voc.iudx.org.in/"
            },
            "rdfs:label": "authType"
        },
        {
            "@id": "https://voc.iudx.org.in/avgOverTime",
            "@type": [
                "rdf:QuantitativeProperty"
            ],
            "iudx:domainIncludes": [
                {
                    "@id": "iudx:TimeSeriesAggregation"
                }
            ],
            "iudx:rangeIncludes": [
                {
                    "@id": "iudx:Number"
                },
                {
                    "@id": "iudx:ValueDescriptor"
                }
            ],
            "rdfs:comment": "Describes the average value of a time-series data over a specified duration in past. The duration is specified using another parameter in the value descriptor object related to this value",
            "rdfs:isDefinedBy": {
                "@id": "https://voc.iudx.org.in/"
            },
            "rdfs:label": "avgOverTime"
        },
        {
            "@id": "https://voc.iudx.org.in/brandName",
            "@type": [
                "iudx:TextProperty"
            ],
            "iudx:domainIncludes": [
                {
                    "@id": "iudx:ModelInfo"
                }
            ],
            "iudx:rangeIncludes": [
                {
                    "@id": "iudx:Text"
                }
            ],
            "rdfs:comment": "Name of the brand associated with an entity, e.g., sensor, device etc.",
            "rdfs:isDefinedBy": {
                "@id": "https://voc.iudx.org.in/"
            },
            "rdfs:label": "brandName",
            "skos:exactMatch": {
                "@id": "https://uri.fiware.org/ns/data-models#brandName"
            }
        },
        {
            "@id": "https://voc.iudx.org.in/coordinates",
            "@type": [
                "iudx:GeoProperty"
            ],
            "iudx:domainIncludes": [
                {
                    "@id": "iudx:Point"
                }
            ],
            "iudx:rangeIncludes": [
                {
                    "@container": "@list",
                    "@id": "iudx:Number"
                }
            ],
            "rdfs:comment": "Coordinates for the GeoJSON object",
            "rdfs:isDefinedBy": {
                "@id": "https://voc.iudx.org.in/"
            },
            "rdfs:label": "coordinates"
        },
        {
            "@id": "https://voc.iudx.org.in/dataDescriptor",
            "@type": [
                "iudx:Relationship"
            ],
            "iudx:domainIncludes": [
                {
                    "@id": "iudx:ResourceGroup"
                },
                {
                    "@id": "iudx:Resource"
                }
            ],
            "iudx:rangeIncludes": [
                {
                    "@id": "iudx:Text",
                    "@type": "@id"
                },
                {
                    "@id": "iudx:RelationshipValue"
                },
                {
                    "@id": "iudx:DataModel"
                }
            ],
            "rdfs:comment": "URI pointing to the data-descriptor entity",
            "rdfs:isDefinedBy": {
                "@id": "https://voc.iudx.org.in/"
            },
            "rdfs:label": "dataDescriptor"
        },
        {
            "@id": "https://voc.iudx.org.in/dataDescriptorLabel",
            "@type": [
                "iudx:TextProperty"
            ],
            "iudx:domainIncludes": [
                {
                    "@id": "iudx:DataDescriptor"
                }
            ],
            "iudx:rangeIncludes": [
                {
                    "@id": "iudx:Text"
                }
            ],
            "rdfs:comment": "Human readable label for an entity",
            "rdfs:isDefinedBy": {
                "@id": "https://voc.iudx.org.in/"
            },
            "rdfs:label": "dataDescriptorLabel"
        },
        {
            "@id": "https://voc.iudx.org.in/dataDescriptorName",
            "@type": [
                "iudx:TextProperty"
            ],
            "iudx:domainIncludes": [
                {
                    "@id": "iudx:DataDescriptor"
                }
            ],
            "iudx:rangeIncludes": [
                {
                    "@id": "iudx:Text"
                }
            ],
            "rdfs:comment": "Name of the entity.",
            "rdfs:isDefinedBy": {
                "@id": "https://voc.iudx.org.in/"
            },
            "rdfs:label": "dataDescriptorName",
            "skos:exactMatch": {
                "@id": "http://schema.org/name"
            }
        },
        {
            "@id": "https://voc.iudx.org.in/dataSample",
            "@type": [
                "iudx:TextProperty"
            ],
            "iudx:domainIncludes": [
                {
                    "@id": "iudx:ResourceGroup"
                },
                {
                    "@id": "iudx:Resource"
                }
            ],
            "iudx:rangeIncludes": [
                {
                    "@id": "iudx:Text"
                }
            ],
            "rdfs:comment": "Stringified sample object of the resource",
            "rdfs:isDefinedBy": {
                "@id": "https://voc.iudx.org.in/"
            },
            "rdfs:label": "dataSample"
        },
        {
            "@id": "https://voc.iudx.org.in/dataSampleFile",
            "@type": [
                "iudx:TextProperty"
            ],
            "iudx:domainIncludes": [
                {
                    "@id": "iudx:ResourceGroup"
                },
                {
                    "@id": "iudx:Resource"
                }
            ],
            "iudx:rangeIncludes": [
                {
                    "@id": "iudx:Text"
                }
            ],
            "rdfs:comment": "Sample file download link for the resource",
            "rdfs:isDefinedBy": {
                "@id": "https://voc.iudx.org.in/"
            },
            "rdfs:label": "dataSampleFile"
        },
        {
            "@id": "https://voc.iudx.org.in/dataSchema",
            "@type": [
                "iudx:TextProperty"
            ],
            "iudx:domainIncludes": [
                {
                    "@id": "iudx:ValueDescriptor"
                }
            ],
            "iudx:rangeIncludes": [
                {
                    "@id": "iudx:Text",
                    "@type": "@id"
                }
            ],
            "rdfs:comment": "Associated data schema. Specified as an URI (linking it to one of the known data type vocabulary, e.g., xsd)",
            "rdfs:isDefinedBy": {
                "@id": "https://voc.iudx.org.in/"
            },
            "rdfs:label": "dataSchema"
        },
        {
            "@id": "https://voc.iudx.org.in/date",
            "@type": [
                "iudx:TextProperty"
            ],
            "iudx:domainIncludes": [
                {
                    "@id": "iudx:RevenueCollection"
                },
                {
                    "@id": "iudx:EmployeeDetails"
                }
            ],
            "iudx:rangeIncludes": [
                {
                    "@id": "iudx:Text"
                },
                {
                    "@id": "iudx:ValueDescriptor"
                }
            ],
            "rdfs:comment": "Date corresponding to this observation and is described in YYYY-MM-DD format, for eg. '2020-11-01'.",
            "rdfs:isDefinedBy": {
                "@id": "https://voc.iudx.org.in/"
            },
            "rdfs:label": "date"
        },
        {
            "@id": "https://voc.iudx.org.in/description",
            "@type": [
                "iudx:TextProperty"
            ],
            "iudx:domainIncludes": [
                {
                    "@id": "iudx:Thing"
                }
            ],
            "iudx:rangeIncludes": [
                {
                    "@id": "iudx:Text"
                }
            ],
            "rdfs:comment": "Description for an IUDX thing.",
            "rdfs:isDefinedBy": {
                "@id": "https://voc.iudx.org.in/"
            },
            "rdfs:label": "description"
        },
        {
            "@id": "https://voc.iudx.org.in/domainIncludes",
            "@type": [
                "rdf:Property"
            ],
            "iudx:domainIncludes": [
                {
                    "@id": "rdf:Property"
                }
            ],
            "iudx:rangeIncludes": [
                {
                    "@id": "rdfs:Class"
                }
            ],
            "rdfs:comment": "Relates a property to a class that is (one of) the type(s) the property is expected to be used on.",
            "rdfs:isDefinedBy": {
                "@id": "https://voc.iudx.org.in/"
            },
            "rdfs:label": "domainIncludes"
        },
        {
            "@id": "https://voc.iudx.org.in/durationInHours",
            "@type": [
                "rdf:Property"
            ],
            "iudx:domainIncludes": [
                {
                    "@id": "iudx:ValueDescriptor"
                }
            ],
            "iudx:rangeIncludes": [
                {
                    "@id": "iudx:Number"
                }
            ],
            "rdfs:comment": "Specifies an interval duration in hours for computing statistical aggregations.",
            "rdfs:isDefinedBy": {
                "@id": "https://voc.iudx.org.in/"
            },
            "rdfs:label": "durationInHours"
        },
        {
            "@id": "https://voc.iudx.org.in/durationInMinutes",
            "@type": [
                "rdf:Property"
            ],
            "iudx:domainIncludes": [
                {
                    "@id": "iudx:ValueDescriptor"
                }
            ],
            "iudx:rangeIncludes": [
                {
                    "@id": "iudx:Number"
                }
            ],
            "rdfs:comment": "Specifies an interval duration in minutes for computing statistical aggregations.",
            "rdfs:isDefinedBy": {
                "@id": "https://voc.iudx.org.in/"
            },
            "rdfs:label": "durationInMinutes"
        },
        {
            "@id": "https://voc.iudx.org.in/functionParameters",
            "@type": [
                "iudx:TextProperty"
            ],
            "iudx:domainIncludes": [
                {
                    "@id": "iudx:FunctionDescription"
                }
            ],
            "iudx:rangeIncludes": [
                {
                    "@container": "@list",
                    "@id": "iudx:Text"
                }
            ],
            "rdfs:comment": "List of parameters associated with a function.",
            "rdfs:isDefinedBy": {
                "@id": "https://voc.iudx.org.in/"
            },
            "rdfs:label": "functionParameters"
        },
        {
            "@id": "https://voc.iudx.org.in/geoCovers",
            "@type": [
                "iudx:GeoProperty"
            ],
            "iudx:domainIncludes": [
                {
                    "@id": "iudx:Place"
                },
                {
                    "@id": "iudx:TransitManagement"
                }
            ],
            "iudx:rangeIncludes": [
                {
                    "@id": "iudx:GeoJSONGeometry"
                }
            ],
            "rdfs:comment": "Represents the coverage relationship between two geometries/places.",
            "rdfs:isDefinedBy": {
                "@id": "https://voc.iudx.org.in/"
            },
            "rdfs:label": "geoCovers"
        },
        {
            "@id": "https://voc.iudx.org.in/geoJSON",
            "@type": [
                "iudx:GeoProperty"
            ],
            "iudx:domainIncludes": [
                {
                    "@id": "iudx:Place"
                }
            ],
            "iudx:rangeIncludes": [
                {
                    "@id": "iudx:GeoJSONGeometry"
                }
            ],
            "rdfs:comment": "Geo-coordinates of a place specified in GeoJSON format.",
            "rdfs:isDefinedBy": {
                "@id": "https://voc.iudx.org.in/"
            },
            "rdfs:label": "geoJSON"
        },
        {
            "@id": "https://voc.iudx.org.in/geometry",
            "@type": [
                "iudx:GeoProperty"
            ],
            "iudx:domainIncludes": [
                {
                    "@id": "iudx:Feature"
                },
                {
                    "@id": "iudx:Place"
                }
            ],
            "iudx:rangeIncludes": [
                {
                    "@id": "iudx:GeoJSONGeometry"
                }
            ],
            "rdfs:comment": "Geometry property in a GeoJSON object",
            "rdfs:isDefinedBy": {
                "@id": "https://voc.iudx.org.in/"
            },
            "rdfs:label": "geometry"
        },
        {
            "@id": "https://voc.iudx.org.in/hasObject",
            "@type": [
                "iudx:TextProperty"
            ],
            "iudx:domainIncludes": [
                {
                    "@id": "iudx:RelationshipValue"
                }
            ],
            "iudx:rangeIncludes": [
                {
                    "@id": "iudx:Text",
                    "@type": "@id"
                },
                {
                    "@container": "@set",
                    "@id": "iudx:Text",
                    "@type": "@id"
                }
            ],
            "rdfs:comment": "Value associated with RelationshipValue class. Contains IRI(s) that specify the relationship object(s).",
            "rdfs:isDefinedBy": {
                "@id": "https://voc.iudx.org.in/"
            },
            "rdfs:label": "hasObject"
        },
        {
            "@id": "https://voc.iudx.org.in/id",
            "@type": [
                "iudx:TextProperty"
            ],
            "iudx:domainIncludes": [
                {
                    "@id": "iudx:IUDXEntity"
                }
            ],
            "iudx:rangeIncludes": [
                {
                    "@id": "iudx:Text"
                }
            ],
            "rdfs:comment": "ID of the entity.",
            "rdfs:isDefinedBy": {
                "@id": "https://voc.iudx.org.in/"
            },
            "rdfs:label": "id"
        },
        {
            "@id": "https://voc.iudx.org.in/instValue",
            "@type": [
                "rdf:QuantitativeProperty"
            ],
            "iudx:domainIncludes": [
                {
                    "@id": "iudx:TimeSeriesAggregation"
                }
            ],
            "iudx:rangeIncludes": [
                {
                    "@id": "iudx:Number"
                },
                {
                    "@id": "iudx:ValueDescriptor"
                }
            ],
            "rdfs:comment": "Describes the instantaneous value (associated with the current timestamp) of a time varying quantity.",
            "rdfs:isDefinedBy": {
                "@id": "https://voc.iudx.org.in/"
            },
            "rdfs:label": "instValue"
        },
        {
            "@id": "https://voc.iudx.org.in/isPartOf",
            "@type": [
                "rdf:Property"
            ],
            "iudx:domainIncludes": [
                {
                    "@id": "schema:CreativeWork"
                }
            ],
            "iudx:rangeIncludes": [
                {
                    "@id": "schema:CreativeWork"
                },
                {
                    "@id": "schema:URL"
                }
            ],
            "rdfs:comment": "Indicates an item or CreativeWork that this item, or CreativeWork (in some sense), is part of.",
            "rdfs:isDefinedBy": {
                "@id": "https://voc.iudx.org.in/"
            },
            "rdfs:label": "isPartOf"
        },
        {
            "@id": "https://voc.iudx.org.in/itemCreatedAt",
            "@type": [
                "iudx:TimeProperty"
            ],
            "iudx:domainIncludes": [
                {
                    "@id": "iudx:IUDXEntity"
                }
            ],
            "iudx:rangeIncludes": [
                {
                    "@id": "iudx:DateTime"
                }
            ],
            "rdfs:comment": "DateTime of creation of a catalogue item.",
            "rdfs:isDefinedBy": {
                "@id": "https://voc.iudx.org.in/"
            },
            "rdfs:label": "itemCreatedAt"
        },
        {
            "@id": "https://voc.iudx.org.in/itemDeprecatedAt",
            "@type": [
                "iudx:TimeProperty"
            ],
            "iudx:domainIncludes": [
                {
                    "@id": "iudx:IUDXEntity"
                }
            ],
            "iudx:rangeIncludes": [
                {
                    "@id": "iudx:DateTime"
                }
            ],
            "rdfs:comment": "DateTime of deprecation of a catalogue item.",
            "rdfs:isDefinedBy": {
                "@id": "https://voc.iudx.org.in/"
            },
            "rdfs:label": "itemDeprecatedAt"
        },
        {
            "@id": "https://voc.iudx.org.in/itemModifiedAt",
            "@type": [
                "iudx:TimeProperty"
            ],
            "iudx:domainIncludes": [
                {
                    "@id": "iudx:IUDXEntity"
                }
            ],
            "iudx:rangeIncludes": [
                {
                    "@id": "iudx:DateTime"
                }
            ],
            "rdfs:comment": "DateTime of modification of a catalogue item.",
            "rdfs:isDefinedBy": {
                "@id": "https://voc.iudx.org.in/"
            },
            "rdfs:label": "itemModifiedAt"
        },
        {
            "@id": "https://voc.iudx.org.in/itemStatus",
            "@type": [
                "iudx:TextProperty"
            ],
            "iudx:domainIncludes": [
                {
                    "@id": "iudx:IUDXEntity"
                }
            ],
            "iudx:rangeIncludes": [
                {
                    "@id": "iudx:Text"
                }
            ],
            "rdfs:comment": "Status of a catalouge item. ENUM: [ACTIVE, DEPRECATED].",
            "rdfs:isDefinedBy": {
                "@id": "https://voc.iudx.org.in/"
            },
            "rdfs:label": "itemStatus"
        },
        {
            "@id": "https://voc.iudx.org.in/iudxResourceAPIs",
            "@type": [
                "iudx:TextProperty"
            ],
            "iudx:domainIncludes": [
                {
                    "@id": "iudx:ResourceGroup",
                    "iudx:requiredProperty": true
                },
                {
                    "@id": "iudx:Resource"
                }
            ],
            "iudx:rangeIncludes": [
                {
                    "@container": "@set",
                    "@id": "iudx:Text"
                }
            ],
            "rdfs:comment": "The set of IUDX resource APIs supported by a given ResourceGroup. ENUM: [TEMPORAL, SPATIAL, ATTR, TEXT]",
            "rdfs:isDefinedBy": {
                "@id": "https://voc.iudx.org.in/"
            },
            "rdfs:label": "iudxResourceAPIs"
        },
        {
            "@id": "https://voc.iudx.org.in/label",
            "@type": [
                "iudx:TextProperty"
            ],
            "iudx:domainIncludes": [
                {
                    "@id": "iudx:IUDXEntity"
                }
            ],
            "iudx:rangeIncludes": [
                {
                    "@id": "iudx:Text"
                }
            ],
            "rdfs:comment": "Human readable label for an entity",
            "rdfs:isDefinedBy": {
                "@id": "https://voc.iudx.org.in/"
            },
            "rdfs:label": "label"
        },
        {
            "@id": "https://voc.iudx.org.in/landmark",
            "@type": [
                "iudx:GeoProperty"
            ],
            "iudx:domainIncludes": [
                {
                    "@id": "iudx:IssueReporting"
                }
            ],
            "iudx:rangeIncludes": [
                {
                    "@id": "iudx:Text"
                },
                {
                    "@id": "iudx:ValueDescriptor"
                }
            ],
            "rdfs:comment": "A physical distinguishing feature on land that marks a locality or a place.",
            "rdfs:isDefinedBy": {
                "@id": "https://voc.iudx.org.in/"
            },
            "rdfs:label": "landmark"
        },
        {
            "@id": "https://voc.iudx.org.in/latitude",
            "@type": [
                "iudx:GeoProperty"
            ],
            "iudx:domainIncludes": [
                {
                    "@id": "iudx:GeoCoordinates"
                },
                {
                    "@id": "iudx:Place"
                },
                {
                    "@id": "iudx:TransitManagement"
                },
                {
                    "@id": "iudx:WmgmtVehicle"
                }
            ],
            "iudx:rangeIncludes": [
                {
                    "@id": "iudx:Number"
                },
                {
                    "@id": "iudx:Text"
                }
            ],
            "rdfs:comment": "Latitude of a place. Specified in WGS 84 CRS (https://en.wikipedia.org/wiki/World_Geodetic_System)",
            "rdfs:isDefinedBy": {
                "@id": "https://voc.iudx.org.in/"
            },
            "rdfs:label": "latitude",
            "skos:exactMatch": {
                "@id": "http://schema.org/latitude"
            }
        },
        {
            "@id": "https://voc.iudx.org.in/location",
            "@type": [
                "iudx:GeoProperty"
            ],
            "iudx:domainIncludes": [
                {
                    "@id": "iudx:Resource"
                },
                {
                    "@id": "iudx:ResourceGroup"
                },
                {
                    "@id": "iudx:Provider"
                },
                {
                    "@id": "iudx:ResourceServer"
                },
                {
                    "@id": "iudx:Organization"
                },
                {
                    "@id": "iudx:EnvAQM"
                },
                {
                    "@id": "iudx:EnvFlood"
                },
                {
                    "@id": "iudx:StreetLightFeeder"
                },
                {
                    "@id": "iudx:WmgmtBin"
                },
                {
                    "@id": "iudx:WmgmtVehicle"
                },
                {
                    "@id": "iudx:TransitManagement"
                },
                {
                    "@id": "iudx:PointOfInterest"
                },
                {
                    "@id": "iudx:SafetiPin"
                },
                {
                    "@id": "iudx:IssueReporting"
                },
                {
                    "@id": "iudx:TrafficViolations"
                },
                {
                    "@id": "iudx:Streetlight"
                },
                {
                    "@id": "iudx:BikeDockingStation"
                },
                {
                    "@id": "iudx:WaterDistributionNetwork"
                },
                {
                    "@id": "iudx:Camera"
                },
                {
                    "@id": "iudx:WasteWaterMgmt"
                }
            ],
            "iudx:rangeIncludes": [
                {
                    "@id": "iudx:Point"
                },
                {
                    "@id": "iudx:GeoJSONGeometry"
                },
                {
                    "@id": "iudx:Place"
                },
                {
                    "@id": "iudx:Text"
                },
                {
                    "@id": "iudx:ValueDescriptor"
                }
            ],
            "rdfs:comment": "Location associated with a resource Item (a spatial point), a group of resource items (a spatial region) or even an observation in case of a mobile sensor.",
            "rdfs:isDefinedBy": {
                "@id": "https://voc.iudx.org.in/"
            },
            "rdfs:label": "location",
            "skos:exactMatch": {
                "@id": "http://schema.org/location"
            }
        },
        {
            "@id": "https://voc.iudx.org.in/longitude",
            "@type": [
                "iudx:GeoProperty"
            ],
            "iudx:domainIncludes": [
                {
                    "@id": "iudx:GeoCoordinates"
                },
                {
                    "@id": "iudx:Place"
                },
                {
                    "@id": "iudx:TransitManagement"
                },
                {
                    "@id": "iudx:WmgmtVehicle"
                }
            ],
            "iudx:rangeIncludes": [
                {
                    "@id": "iudx:Number"
                },
                {
                    "@id": "iudx:Text"
                }
            ],
            "rdfs:comment": "Longitude of a place. Specified in WGS 84 CRS (https://en.wikipedia.org/wiki/World_Geodetic_System)",
            "rdfs:isDefinedBy": {
                "@id": "https://voc.iudx.org.in/"
            },
            "rdfs:label": "longitude",
            "skos:exactMatch": {
                "@id": "http://schema.org/longitude"
            }
        },
        {
            "@id": "https://voc.iudx.org.in/manufacturerName",
            "@type": [
                "iudx:TextProperty"
            ],
            "iudx:domainIncludes": [
                {
                    "@id": "iudx:ModelInfo"
                }
            ],
            "iudx:rangeIncludes": [
                {
                    "@id": "iudx:Text"
                }
            ],
            "rdfs:comment": "Name of the manufacturer associated with an entity, e.g., sensor, device etc.",
            "rdfs:isDefinedBy": {
                "@id": "https://voc.iudx.org.in/"
            },
            "rdfs:label": "manufacturerName",
            "skos:exactMatch": {
                "@id": "https://uri.fiware.org/ns/data-models#manufacturerName"
            }
        },
        {
            "@id": "https://voc.iudx.org.in/maxOverTime",
            "@type": [
                "rdf:QuantitativeProperty"
            ],
            "iudx:domainIncludes": [
                {
                    "@id": "iudx:TimeSeriesAggregation"
                }
            ],
            "iudx:rangeIncludes": [
                {
                    "@id": "iudx:Number"
                },
                {
                    "@id": "iudx:ValueDescriptor"
                }
            ],
            "rdfs:comment": "Describes the maximum value of a time-series data over a specified duration in past. The duration is specified using another parameter in the value descriptor object related to this value",
            "rdfs:isDefinedBy": {
                "@id": "https://voc.iudx.org.in/"
            },
            "rdfs:label": "maxOverTime"
        },
        {
            "@id": "https://voc.iudx.org.in/maxValue",
            "@type": [
                "rdf:QuantitativeProperty"
            ],
            "iudx:domainIncludes": [
                {
                    "@id": "iudx:ValueDescriptor"
                }
            ],
            "iudx:rangeIncludes": [
                {
                    "@id": "iudx:Number"
                }
            ],
            "rdfs:comment": "The upper value of a quantity/property.",
            "rdfs:isDefinedBy": {
                "@id": "https://voc.iudx.org.in/"
            },
            "rdfs:label": "maxValue",
            "skos:exactMatch": {
                "@id": "http://schema.org/maxValue"
            }
        },
        {
            "@id": "https://voc.iudx.org.in/measAccuracy",
            "@type": [
                "iudx:QuantitativeProperty"
            ],
            "iudx:domainIncludes": [
                {
                    "@id": "iudx:ValueDescriptor"
                }
            ],
            "iudx:rangeIncludes": [
                {
                    "@id": "iudx:Text"
                },
                {
                    "@id": "iudx:ValueDescriptor"
                }
            ],
            "rdfs:comment": "Accuracy of a measurement. Maximum difference that can exist between the actual value and the measured value. It can be specified in relative as well as absolute terms.",
            "rdfs:isDefinedBy": {
                "@id": "https://voc.iudx.org.in/"
            },
            "rdfs:label": "measAccuracy"
        },
        {
            "@id": "https://voc.iudx.org.in/mediaURL",
            "@type": [
                "iudx:TextProperty"
            ],
            "iudx:domainIncludes": [
                {
                    "@id": "iudx:SafetiPin"
                },
                {
                    "@id": "iudx:IssueReporting"
                },
                {
                    "@id": "iudx:TrafficViolations"
                },
                {
                    "@id": "iudx:BikeDockingStation"
                },
                {
                    "@id": "iudx:Camera"
                }
            ],
            "iudx:rangeIncludes": [
                {
                    "@container": "@list",
                    "@id": "iudx:Text"
                },
                {
                    "@id": "iudx:ValueDescriptor"
                }
            ],
            "rdfs:comment": "URL providing further information of any image(s) or media of the complaint or place.",
            "rdfs:isDefinedBy": {
                "@id": "https://voc.iudx.org.in/"
            },
            "rdfs:label": "mediaURL",
            "skos:exactMatch": {
                "@id": "http://ontology.eil.utoronto.ca/open311.owl#media_url"
            }
        },
        {
            "@id": "https://voc.iudx.org.in/minOverTime",
            "@type": [
                "rdf:QuantitativeProperty"
            ],
            "iudx:domainIncludes": [
                {
                    "@id": "iudx:TimeSeriesAggregation"
                }
            ],
            "iudx:rangeIncludes": [
                {
                    "@id": "iudx:Number"
                },
                {
                    "@id": "iudx:ValueDescriptor"
                }
            ],
            "rdfs:comment": "Describes the minimum value of a time-series data over a specified duration in past. The duration is specified using another parameter in the value descriptor object related to this value",
            "rdfs:isDefinedBy": {
                "@id": "https://voc.iudx.org.in/"
            },
            "rdfs:label": "minOverTime"
        },
        {
            "@id": "https://voc.iudx.org.in/minValue",
            "@type": [
                "rdf:QuantitativeProperty"
            ],
            "iudx:domainIncludes": [
                {
                    "@id": "iudx:ValueDescriptor"
                }
            ],
            "iudx:rangeIncludes": [
                {
                    "@id": "iudx:Number"
                }
            ],
            "rdfs:comment": "The lower value of a quantity/property.",
            "rdfs:isDefinedBy": {
                "@id": "https://voc.iudx.org.in/"
            },
            "rdfs:label": "minValue",
            "skos:exactMatch": {
                "@id": "http://schema.org/minValue"
            }
        },
        {
            "@id": "https://voc.iudx.org.in/modelName",
            "@type": [
                "iudx:TextProperty"
            ],
            "iudx:domainIncludes": [
                {
                    "@id": "iudx:ModelInfo"
                }
            ],
            "iudx:rangeIncludes": [
                {
                    "@id": "iudx:Text"
                }
            ],
            "rdfs:comment": "Name of a specific model associated with an entity, e.g., sensor, device etc.",
            "rdfs:isDefinedBy": {
                "@id": "https://voc.iudx.org.in/"
            },
            "rdfs:label": "modelName",
            "skos:exactMatch": {
                "@id": "https://uri.fiware.org/ns/data-models#modelName"
            }
        },
        {
            "@id": "https://voc.iudx.org.in/modelURL",
            "@type": [
                "iudx:TextProperty"
            ],
            "iudx:domainIncludes": [
                {
                    "@id": "iudx:ModelInfo"
                }
            ],
            "iudx:rangeIncludes": [
                {
                    "@id": "iudx:Text"
                }
            ],
            "rdfs:comment": "URL providing further information of a specific model associated with an entity, e.g., sensor, device etc.",
            "rdfs:isDefinedBy": {
                "@id": "https://voc.iudx.org.in/"
            },
            "rdfs:label": "modelURL"
        },
        {
            "@id": "https://voc.iudx.org.in/month",
            "@type": [
                "iudx:TextProperty"
            ],
            "iudx:domainIncludes": [
                {
                    "@id": "iudx:RevenueCollection"
                }
            ],
            "iudx:rangeIncludes": [
                {
                    "@id": "iudx:Text"
                },
                {
                    "@id": "iudx:ValueDescriptor"
                }
            ],
            "rdfs:comment": "Month corresponding to this observation and is described in MM format, for eg. '05' for the month of May.",
            "rdfs:isDefinedBy": {
                "@id": "https://voc.iudx.org.in/"
            },
            "rdfs:label": "month"
        },
        {
            "@id": "https://voc.iudx.org.in/name",
            "@type": [
                "iudx:TextProperty"
            ],
            "iudx:domainIncludes": [
                {
                    "@id": "iudx:Place"
                },
                {
                    "@id": "iudx:Organization"
                },
                {
                    "@id": "iudx:IUDXEntity",
                    "iudx:requiredProperty": true
                },
                {
                    "@id": "iudx:PointOfInterest"
                }
            ],
            "iudx:rangeIncludes": [
                {
                    "@id": "iudx:Text"
                },
                {
                    "@id": "iudx:ValueDescriptor"
                }
            ],
            "rdfs:comment": "Name of the entity.",
            "rdfs:isDefinedBy": {
                "@id": "https://voc.iudx.org.in/"
            },
            "rdfs:label": "name",
            "skos:exactMatch": {
                "@id": "http://schema.org/name"
            }
        },
        {
            "@id": "https://voc.iudx.org.in/openDataFields",
            "@type": [
                "iudx:TextProperty"
            ],
            "iudx:domainIncludes": [
                {
                    "@id": "iudx:DataFieldListValue"
                }
            ],
            "iudx:rangeIncludes": [
                {
                    "@container": "@set",
                    "@id": "iudx:Text"
                }
            ],
            "rdfs:comment": "List of properties/fields/attributes contained in the data available from the resources associated with a given resource Group which are open, i.e., no authorization is required to access these fields for a given resource.",
            "rdfs:isDefinedBy": {
                "@id": "https://voc.iudx.org.in/"
            },
            "rdfs:label": "openDataFields"
        },
        {
            "@id": "https://voc.iudx.org.in/provider",
            "@type": [
                "iudx:Relationship"
            ],
            "iudx:domainIncludes": [
                {
                    "@id": "iudx:Resource"
                },
                {
                    "@id": "iudx:ResourceGroup",
                    "iudx:requiredProperty": true
                }
            ],
            "iudx:rangeIncludes": [
                {
                    "@id": "iudx:Text",
                    "@type": "@id"
                },
                {
                    "@id": "iudx:RelationshipValue"
                }
            ],
            "rdfs:comment": "IRI pointing to the provider entity associated with the given catalogue item",
            "rdfs:isDefinedBy": {
                "@id": "https://voc.iudx.org.in/"
            },
            "rdfs:label": "provider"
        },
        {
            "@id": "https://voc.iudx.org.in/providerOrg",
            "@type": [
                "iudx:StructuredProperty"
            ],
            "iudx:domainIncludes": [
                {
                    "@id": "iudx:Provider",
                    "iudx:requiredProperty": true
                }
            ],
            "iudx:rangeIncludes": [
                {
                    "@id": "iudx:Organization"
                }
            ],
            "rdfs:comment": "Information about the Provider Organization.",
            "rdfs:isDefinedBy": {
                "@id": "https://voc.iudx.org.in/"
            },
            "rdfs:label": "providerOrg"
        },
        {
            "@id": "https://voc.iudx.org.in/rangeIncludes",
            "@type": [
                "rdf:Property"
            ],
            "iudx:domainIncludes": [
                {
                    "@id": "rdf:Property"
                }
            ],
            "iudx:rangeIncludes": [
                {
                    "@id": "rdfs:Class"
                }
            ],
            "rdfs:comment": "Relates a property to a class that constitutes (one of) the expected type(s) for values of the property.",
            "rdfs:isDefinedBy": {
                "@id": "https://voc.iudx.org.in/"
            },
            "rdfs:label": "rangeIncludes",
            "skos:exactMatch": {
                "@id": "http://schema.org/rangeIncludes"
            }
        },
        {
            "@id": "https://voc.iudx.org.in/relatedEntity",
            "@type": [
                "iudx:Relationship"
            ],
            "iudx:domainIncludes": [
                {
                    "@id": "iudx:IUDXEntity"
                }
            ],
            "iudx:rangeIncludes": [
                {
                    "@id": "iudx:Text"
                },
                {
                    "@id": "iudx:RelationshipValue"
                }
            ],
            "rdfs:comment": "ID of the associated entity.",
            "rdfs:isDefinedBy": {
                "@id": "https://voc.iudx.org.in/"
            },
            "rdfs:label": "relatedEntity"
        },
        {
            "@id": "https://voc.iudx.org.in/relationType",
            "@type": [
                "iudx:TextProperty"
            ],
            "iudx:domainIncludes": [
                {
                    "@id": "iudx:RelationshipValue",
                    "iudx:requiredProperty": true
                }
            ],
            "iudx:rangeIncludes": [
                {
                    "@id": "iudx:Text"
                }
            ],
            "rdfs:comment": "Type of relation. ENUM: [REL_MESSAGESTREAM, REL_FILE].",
            "rdfs:isDefinedBy": {
                "@id": "https://voc.iudx.org.in/"
            },
            "rdfs:label": "relationType"
        },
        {
            "@id": "https://voc.iudx.org.in/requiredProperty",
            "@type": [
                "rdf:Property"
            ],
            "iudx:domainIncludes": [
                {
                    "@id": "rdf:Property"
                }
            ],
            "iudx:rangeIncludes": [
                {
                    "@id": "iudx:Boolean"
                }
            ],
            "rdfs:comment": "Boolean Value. Indicates if this property is required in the domain.",
            "rdfs:isDefinedBy": {
                "@id": "https://voc.iudx.org.in/"
            },
            "rdfs:label": "requiredProperties"
        },
        {
            "@id": "https://voc.iudx.org.in/resolution",
            "@type": [
                "iudx:QuantitativeProperty"
            ],
            "iudx:domainIncludes": [
                {
                    "@id": "iudx:ValueDescriptor"
                }
            ],
            "iudx:rangeIncludes": [
                {
                    "@id": "iudx:Number"
                },
                {
                    "@id": "iudx:ValueDescriptor"
                }
            ],
            "rdfs:comment": "Resolution of a measurement. That is, the smallest change in a quantity being measured that causes a perceptible change in the corresponding observation under specified conditions.",
            "rdfs:isDefinedBy": {
                "@id": "https://voc.iudx.org.in/"
            },
            "rdfs:label": "resolution"
        },
        {
            "@id": "https://voc.iudx.org.in/resourceGroup",
            "@type": [
                "iudx:Relationship"
            ],
            "iudx:domainIncludes": [
                {
                    "@id": "iudx:Resource",
                    "iudx:requiredProperty": true
                }
            ],
            "iudx:rangeIncludes": [
                {
                    "@id": "iudx:Text",
                    "@type": "@id"
                },
                {
                    "@id": "iudx:RelationshipValue"
                }
            ],
            "rdfs:comment": "IRI pointing to the resourceGroup entity associated with the resource.",
            "rdfs:isDefinedBy": {
                "@id": "https://voc.iudx.org.in/"
            },
            "rdfs:label": "resourceGroup"
        },
        {
            "@id": "https://voc.iudx.org.in/resourceServer",
            "@type": [
                "iudx:Relationship"
            ],
            "iudx:domainIncludes": [
                {
                    "@id": "iudx:Resource"
                },
                {
                    "@id": "iudx:ResourceGroup"
                }
            ],
            "iudx:rangeIncludes": [
                {
                    "@id": "iudx:Text",
                    "@type": "@id"
                },
                {
                    "@id": "iudx:RelationshipValue"
                }
            ],
            "rdfs:comment": "IRI pointing to the ResourceServer entity for a given Resource or ResourceGroup.",
            "rdfs:isDefinedBy": {
                "@id": "https://voc.iudx.org.in/"
            },
            "rdfs:label": "resourceServer"
        },
        {
            "@id": "https://voc.iudx.org.in/resourceServerFileAccessURL",
            "@type": [
                "iudx:Relationship"
            ],
            "iudx:domainIncludes": [
                {
                    "@id": "iudx:ResourceServer"
                }
            ],
            "iudx:rangeIncludes": [
                {
                    "@id": "iudx:Text",
                    "@type": "@id"
                }
            ],
            "rdfs:comment": "Resource Server URL for file access",
            "rdfs:isDefinedBy": {
                "@id": "https://voc.iudx.org.in/"
            },
            "rdfs:label": "resourceServerFileAccessURL"
        },
        {
            "@id": "https://voc.iudx.org.in/resourceServerHTTPAccessURL",
            "@type": [
                "iudx:Relationship"
            ],
            "iudx:domainIncludes": [
                {
                    "@id": "iudx:ResourceServer"
                }
            ],
            "iudx:rangeIncludes": [
                {
                    "@id": "iudx:Text",
                    "@type": "@id"
                }
            ],
            "rdfs:comment": "Resource Server URL for data access based on HTTP/REST APIs",
            "rdfs:isDefinedBy": {
                "@id": "https://voc.iudx.org.in/"
            },
            "rdfs:label": "resourceServerHTTPAccessURL"
        },
        {
            "@id": "https://voc.iudx.org.in/resourceServerOrg",
            "@type": [
                "iudx:StructuredProperty"
            ],
            "iudx:domainIncludes": [
                {
                    "@id": "iudx:ResourceServer"
                }
            ],
            "iudx:rangeIncludes": [
                {
                    "@id": "iudx:Organization"
                }
            ],
            "rdfs:comment": "Information about the organization operating the Resource Server.",
            "rdfs:isDefinedBy": {
                "@id": "https://voc.iudx.org.in/"
            },
            "rdfs:label": "resourceServerOrg"
        },
        {
            "@id": "https://voc.iudx.org.in/resourceServerStreamingAccessURL",
            "@type": [
                "iudx:Relationship"
            ],
            "iudx:domainIncludes": [
                {
                    "@id": "iudx:ResourceServer"
                }
            ],
            "iudx:rangeIncludes": [
                {
                    "@id": "iudx:Text",
                    "@type": "@id"
                }
            ],
            "rdfs:comment": "Resource Server URL for data access based on Streaming",
            "rdfs:isDefinedBy": {
                "@id": "https://voc.iudx.org.in/"
            },
            "rdfs:label": "resourceServerStreamingAccessURL"
        },
        {
            "@id": "https://voc.iudx.org.in/resourceType",
            "@type": [
                "iudx:TextProperty"
            ],
            "iudx:domainIncludes": [
                {
                    "@id": "iudx:ResourceGroup",
                    "iudx:requiredProperty": true
                },
                {
                    "@id": "iudx:Resource"
                }
            ],
            "iudx:rangeIncludes": [
                {
                    "@id": "iudx:Text"
                }
            ],
            "rdfs:comment": "Type of resource. ENUM: [MESSAGESTREAM, DATASET, FILE, GSLAYER, MEDIASTREAM].",
            "rdfs:isDefinedBy": {
                "@id": "https://voc.iudx.org.in/"
            },
            "rdfs:label": "resourceType"
        },
        {
            "@id": "https://voc.iudx.org.in/sameAs",
            "@type": [
                "iudx:TextProperty"
            ],
            "iudx:domainIncludes": [
                {
                    "@id": "iudx:ValueDescriptor"
                }
            ],
            "iudx:rangeIncludes": [
                {
                    "@id": "iudx:Text",
                    "@type": "@id"
                }
            ],
            "rdfs:comment": "URL reference to another thing/entity that identifies the given thing/entity. This may be used to provide references to another data models where a property is described or say a reference to Wiki pages for a given thing etc.",
            "rdfs:isDefinedBy": {
                "@id": "https://voc.iudx.org.in/"
            },
            "rdfs:label": "sameAs",
            "skos:exactMatch": {
                "@id": "http://schema.org/sameAs"
            }
        },
        {
            "@id": "https://voc.iudx.org.in/secureDataFields",
            "@type": [
                "iudx:TextProperty"
            ],
            "iudx:domainIncludes": [
                {
                    "@id": "iudx:DataFieldListValue"
                }
            ],
            "iudx:rangeIncludes": [
                {
                    "@container": "@set",
                    "@id": "iudx:Text"
                }
            ],
            "rdfs:comment": "List of properties/fields/attributes contained in the data available from the resources associated with a given resource Group which are secure, i.e., need authorization from the auth server to access these fields for a given resource.",
            "rdfs:isDefinedBy": {
                "@id": "https://voc.iudx.org.in/"
            },
            "rdfs:label": "secureDataFields"
        },
        {
            "@id": "https://voc.iudx.org.in/tags",
            "@type": [
                "iudx:TextProperty"
            ],
            "iudx:domainIncludes": [
                {
                    "@id": "iudx:Resource",
                    "iudx:requiredProperty": true
                },
                {
                    "@id": "iudx:ResourceGroup",
                    "iudx:requiredProperty": true
                }
            ],
            "iudx:rangeIncludes": [
                {
                    "@container": "@list",
                    "@id": "iudx:Text"
                }
            ],
            "rdfs:comment": "Comma separated discovery tags associated with an IUDXEntity (resource , resource Group)",
            "rdfs:isDefinedBy": {
                "@id": "https://voc.iudx.org.in/"
            },
            "rdfs:label": "tags"
        },
        {
            "@id": "https://voc.iudx.org.in/unitCode",
            "@type": [
                "iudx:TextProperty"
            ],
            "iudx:domainIncludes": [
                {
                    "@id": "iudx:ValueDescriptor"
                }
            ],
            "iudx:rangeIncludes": [
                {
                    "@id": "iudx:Text"
                },
                {
                    "@id": "iudx:Text",
                    "@type": "@id"
                }
            ],
            "rdfs:comment": "The unit of measurement given using the UN/CEFACT Common Code (3 characters) or a URL. Other codes/unit vocabularies may be used with a prefix",
            "rdfs:isDefinedBy": {
                "@id": "https://voc.iudx.org.in/"
            },
            "rdfs:label": "unitCode",
            "skos:exactMatch": {
                "@id": "http://schema.org/unitCode"
            }
        },
        {
            "@id": "https://voc.iudx.org.in/unitText",
            "@type": [
                "iudx:TextProperty"
            ],
            "iudx:domainIncludes": [
                {
                    "@id": "iudx:ValueDescriptor"
                }
            ],
            "iudx:rangeIncludes": [
                {
                    "@id": "iudx:Text"
                }
            ],
            "rdfs:comment": "Describes the unit of measurement. Useful if unitCode is not available.",
            "rdfs:isDefinedBy": {
                "@id": "https://voc.iudx.org.in/"
            },
            "rdfs:label": "unitText",
            "skos:exactMatch": {
                "@id": "http://schema.org/unitText"
            }
        },
        {
            "@id": "https://voc.iudx.org.in/value",
            "@type": [
                "rdf:Property"
            ],
            "iudx:domainIncludes": [
                {
                    "@id": "iudx:ValueDescriptor"
                }
            ],
            "iudx:rangeIncludes": [
                {
                    "@id": "iudx:Number"
                },
                {
                    "@id": "iudx:Text"
                },
                {
                    "@id": "iudx:Boolean"
                },
                {
                    "@id": "iudx:NumericArray"
                },
                {
                    "@id": "iudx:StructuredValue"
                }
            ],
            "rdfs:comment": "Value of the quantity being described in the ValueDescriptor object.",
            "rdfs:isDefinedBy": {
                "@id": "https://voc.iudx.org.in/"
            },
            "rdfs:label": "value"
        },
        {
            "@id": "https://voc.iudx.org.in/year",
            "@type": [
                "iudx:TextProperty"
            ],
            "iudx:domainIncludes": [
                {
                    "@id": "iudx:RevenueCollection"
                }
            ],
            "iudx:rangeIncludes": [
                {
                    "@id": "iudx:Text"
                },
                {
                    "@id": "iudx:ValueDescriptor"
                }
            ],
            "rdfs:comment": "Year corresponding to this observation and is described in YYYY format, for eg. '2020'.",
            "rdfs:isDefinedBy": {
                "@id": "https://voc.iudx.org.in/"
            },
            "rdfs:label": "year"
        }
    ]
}